remake larger model based on small model

OtbnModel.v
@@ -7,33 +7,35 @@ Require Import coqutil.Semantics.OmniSmallstepCombinators.
 Require Import coqutil.Map.Interface.
 Require Import coqutil.Tactics.Tactics.
 Require Import coqutil.Word.Interface.
+Require Import coqutil.Word.Properties.
+Require Import coqutil.Z.PushPullMod.
 Require Coq.Strings.HexString.
 Import ListNotations.
 Local Open Scope Z_scope.
 
+(*** Model of OTBN. ***)
+
+(* Size of DMEM. *)
+Definition DMEM_BYTES := 8192.
+
 Section Registers.
   (* General data registers, 32 bits each. *)
+  (* x0 is always wired to 0, x1 is the call stack. *)
   Inductive gpr : Type :=
-  | x0 | x1 | x2 | x3 | x4 | x5 | x6 | x7 | x8 | x9
-  | x10 | x11 | x12 | x13 | x14 | x15 | x16 | x17 | x18 | x19
-  | x20 | x21 | x22 | x23 | x24 | x25 | x26 | x27 | x28 | x29
-  | x30 | x31
-  .
+  | x0  | x1  | x2  | x3  | x4  | x5  | x6  | x7  | x8  | x9  | x10 | x11 | x12 | x13 | x14 | x15
+  | x16 | x17 | x18 | x19 | x20 | x21 | x22 | x23 | x24 | x25 | x26 | x27 | x28 | x29 | x30 | x31.
 
   (* Wide data registers, 256 bits each. *)
   Inductive wdr : Type :=
-  | w0 | w1 | w2 | w3 | w4 | w5 | w6 | w7 | w8 | w9
-  | w10 | w11 | w12 | w13 | w14 | w15 | w16 | w17 | w18 | w19
-  | w20 | w21 | w22 | w23 | w24 | w25 | w26 | w27 | w28 | w29
-  | w30 | w31
-  .
+  | w0  | w1  | w2  | w3  | w4  | w5  | w6  | w7  | w8  | w9  | w10 | w11 | w12 | w13 | w14 | w15
+  | w16 | w17 | w18 | w19 | w20 | w21 | w22 | w23 | w24 | w25 | w26 | w27 | w28 | w29 | w30 | w31.
 
-  (* Control and status registers, 32-bits each. *)
+  (* Control and status registers, 32 bits each. *)
   Inductive csr : Type :=
   | CSR_FG0
   | CSR_FG1
   | CSR_FLAGS
-      (* These registers are not used much in practice.
+      (* Omit these registers for now, they are ~never used in practice.
   | CSR_MOD0
   | CSR_MOD1
   | CSR_MOD2
@@ -42,205 +44,658 @@ Section Registers.
   | CSR_MOD5
   | CSR_MOD6
   | CSR_MOD7
+       *)
+  | CSR_RND_PREFETCH
   | CSR_RND
   | CSR_URND
-  | CSR_RND_PREFETCH
-       *)
   .
 
-  (* Wide special registers, 256 bits each. *)
+  (* Wide status registers, 256 bits each. *)
   Inductive wsr : Type :=
-  | MOD
-  | ACC
-  | RND
-  | URND
-  | KEY_S0_L
-  | KEY_S0_H
-  | KEY_S1_L
-  | KEY_S1_H
+  | WSR_MOD
+  | WSR_RND
+  | WSR_URND
+  | WSR_ACC
+  | WSR_KEY_S0_L
+  | WSR_KEY_S0_H
+  | WSR_KEY_S1_L
+  | WSR_KEY_S1_H
   .
 
-  (* Catchall type indicating any register. *)
+  (* Catchall type indicating any 32-bit register. *)
   Inductive reg :=
   | gpreg : gpr -> reg
   | csreg : csr -> reg
-  | wdreg : wdr -> reg
-  | wsreg : wsr -> reg
   .
+
+  (* Catchall type indicating any 256-bit register. *)
+  Inductive wreg :=
+  | wdreg : wdr -> wreg
+  | wsreg : wsr -> wreg
+  .
+
+  Inductive flag :=
+  | flagM : bool -> flag
+  | flagL : bool -> flag
+  | flagZ : bool -> flag
+  | flagC : bool -> flag.
 End Registers.
 
-Section Flags.
-  Inductive flag_group : Type :=
-  | FG0
-  | FG1
-  .
-
-  (* TODO: maybe make this a pair *)
-  Inductive flag : Type :=
-  | flagC : forall fg : flag_group, flag
-  | flagM : forall fg : flag_group, flag
-  | flagL : forall fg : flag_group, flag
-  | flagZ : forall fg : flag_group, flag
-  .
-End Flags.
-
 Section ISA.
-  (* Indicates one lib of a wdr; used for mulqacc instructions. *)
-  Inductive limb : Type :=
-  | limb0 : wdr -> limb
-  | limb1 : wdr -> limb
-  | limb2 : wdr -> limb
-  | limb3 : wdr -> limb
-  .
-
-  (* Immediate shift argument for arithmetic instructions. *)
-  Inductive shift : Type :=
-  | lshift : Z -> shift
-  | rshift : Z -> shift
-  .
-
-  (* Indirect register (may have increment bit set or not). *)
-  Inductive ind : Type :=
-  | ind_noinc : gpr -> ind
-  | ind_inc : gpr -> ind
-  .
-
   (* Straightline instructions (no control flow) *)
   Inductive sinsn : Type :=
   | Addi : gpr -> gpr -> Z -> sinsn
-  | Bn_mulqacc : forall (z : bool), limb -> limb -> Z -> sinsn
-  | Bn_mulqacc_wo : forall (z : bool), wdr -> limb -> limb -> Z -> sinsn
-  | Bn_mulqacc_so : forall (z : bool) (L : bool), wdr -> limb -> limb -> Z -> sinsn
-  | Bn_addm : wdr -> wdr -> wdr -> sinsn
-  | Bn_subm : wdr -> wdr -> wdr -> sinsn
-  | Bn_add : wdr -> wdr -> wdr -> shift -> flag_group -> sinsn
-  | Bn_addc : wdr -> wdr -> wdr -> shift -> flag_group -> sinsn
-  | Bn_sub : wdr -> wdr -> wdr -> shift -> flag_group -> sinsn
-  | Bn_subb : wdr -> wdr -> wdr -> shift -> flag_group -> sinsn
-  | Bn_rshi : wdr -> wdr -> wdr -> Z -> sinsn
-  | Bn_movr : ind -> ind -> sinsn
-  | Bn_lid : ind -> Z -> ind -> sinsn
+  | Add : gpr -> gpr -> gpr -> sinsn
+  | Lw : gpr -> gpr -> Z -> sinsn
+  | Sw : gpr -> gpr -> Z -> sinsn
+  | Csrrs : csr -> gpr -> sinsn
   .
 
   (* Control-flow instructions *)
-  Inductive cinsn {addr : Type} : Type :=
+  Inductive cinsn {label : Type} : Type :=
   (* TODO: technically ret is a special case of JALR, but only RET is used in practice *)
   | Ret : cinsn
   | Ecall : cinsn
-  | Jal : gpr -> addr -> cinsn
-  | Bne : gpr -> gpr -> addr -> cinsn
-  | Beq : gpr -> gpr -> addr -> cinsn
-  | Loop : gpr -> nat -> cinsn
-  | Loopi : nat -> nat -> cinsn
+  | Jal : gpr -> label -> cinsn
+  | Bne : gpr -> gpr -> label -> cinsn
+  | Beq : gpr -> gpr -> label -> cinsn
+  (* Note: loops here use an end instruction instead of an iteration
+     count to make codegen and processing easier. *)
+  | Loop : gpr -> cinsn
+  | Loopi : nat -> cinsn
+  | LoopEnd : cinsn
   .
 
-  Inductive insn {addr : Type} : Type :=
+  Inductive insn {label : Type} : Type :=
   | Straightline : sinsn -> insn
-  | Control : cinsn (addr:=addr) -> insn
+  | Control : cinsn (label:=label) -> insn
   .
-
 End ISA.
 
-(* Notations to interpret assembly code. *)
-Module OtbnNotations.
-  Coercion gpreg : gpr >-> reg.
-  Coercion wdreg : wdr >-> reg.
-  Coercion wsreg : wsr >-> reg.
-  Coercion ind_noinc : gpr >-> ind.
-  Coercion Straightline : sinsn >-> insn. 
-  Coercion Control : cinsn >-> insn. 
-  Declare Scope otbn_scope.
-  Delimit Scope otbn_scope with otbn.
+(* Boilerplate definitions for comparing registers. *)
+Section RegisterEquality.
+  Local Ltac derive_eqb r1 r2 :=
+    pose r1 as x1;
+    pose r2 as x2;
+    destruct r1, r2;
+    lazymatch goal with
+    | x1 := ?x, x2 := ?x |- _ => clear; exact true
+    | _ => clear; exact false
+    end.
+  
+  Definition gpr_eqb (r1 r2 : gpr) : bool.
+  Proof. derive_eqb r1 r2. Defined.
+  Definition csr_eqb (r1 r2 : csr) : bool.
+  Proof. derive_eqb r1 r2. Defined.
+  Definition reg_eqb (r1 r2 : reg) : bool :=
+    match r1, r2 with
+    | gpreg r1, gpreg r2 => gpr_eqb r1 r2
+    | csreg r1, csreg r2 => csr_eqb r1 r2
+    | _, _ => false
+    end.
 
-  (* special arguments *)
-  Notation "x '.0'" := (limb0 x) (at level 0) : otbn_scope.
-  Notation "x '.1'" := (limb1 x) (at level 0) : otbn_scope.
-  Notation "x '.2'" := (limb2 x) (at level 0) : otbn_scope.
-  Notation "x '.3'" := (limb3 x) (at level 0) : otbn_scope.
-  Notation "a '++'" := (ind_inc a) (at level 20) : otbn_scope.
+  Local Ltac prove_eqb_spec r1 r2 :=
+    destruct r1, r2; constructor; congruence.
+  Global Instance gpr_eqb_spec : forall r1 r2, BoolSpec (r1 = r2) (r1 <> r2) (gpr_eqb r1 r2).
+  Proof. prove_eqb_spec r1 r2. Qed.
+  Global Instance csr_eqb_spec : forall r1 r2, BoolSpec (r1 = r2) (r1 <> r2) (csr_eqb r1 r2).
+  Proof. prove_eqb_spec r1 r2. Qed.
+  Global Instance reg_eqb_spec : forall r1 r2, BoolSpec (r1 = r2) (r1 <> r2) (reg_eqb r1 r2).
+  Proof.
+    destruct r1, r2; cbn [reg_eqb];
+      repeat lazymatch goal with
+      | |- BoolSpec _ _ (?eqb ?x ?y) => destr (eqb x y)
+      | _ => constructor; congruence
+      end.
+  Qed.
+End RegisterEquality.
 
-  (* straightline instructions *)
-  Notation "'addi' d , a , imm" := (Addi d a imm : insn) (at level 40) : otbn_scope. 
-  Notation "'bn.mulqacc' a , b , imm" := (Bn_mulqacc false a b imm : insn) (at level 40) : otbn_scope.
-  Notation "'bn.mulqacc.z' a , b , imm" := (Bn_mulqacc true a b imm : insn) (at level 40) : otbn_scope.
-  Notation "'bn.mulqacc.wo' d , a , b , imm" := (Bn_mulqacc_wo false d a b imm : insn) (at level 40) : otbn_scope.
-  Notation "'bn.mulqacc.wo.z' d , a , b , imm" := (Bn_mulqacc_wo true d a b imm : insn) (at level 40) : otbn_scope.
-  Notation "'bn.mulqacc.so' d '.L' , a , b , imm" := (Bn_mulqacc_so false true d a b imm : insn) (at level 40) : otbn_scope.
-  Notation "'bn.mulqacc.so' d '.U' , a , b , imm" := (Bn_mulqacc_so false false d a b imm : insn) (at level 40) : otbn_scope.
-  Notation "'bn.mulqacc.so.z' d '.L' , a , b , imm" := (Bn_mulqacc_so true true d a b imm : insn) (at level 40) : otbn_scope.
-  Notation "'bn.mulqacc.so.z' d '.U' , a , b , imm" := (Bn_mulqacc_so true false d a b imm : insn) (at level 40) : otbn_scope.
-  Notation "'bn.addm' d , a , b " := (Bn_addm d a b : insn) (at level 40) : otbn_scope.
-  Notation "'bn.subm' d , a , b " := (Bn_subm d a b : insn) (at level 40) : otbn_scope.
-  Notation "'bn.add' d , a , b , fg" := (Bn_add d a b (lshift 0) fg : insn) (at level 40) : otbn_scope.
-  Notation "'bn.add' d , a , b '<<' s , fg" := (Bn_add d a b (lshift s) fg : insn) (at level 40) : otbn_scope.
-  Notation "'bn.add' d , a , b '>>' s , fg" := (Bn_add d a b (rshift s) fg : insn) (at level 40) : otbn_scope.
-  Notation "'bn.addc' d , a , b , fg" := (Bn_addc d a b (lshift 0) fg : insn) (at level 40) : otbn_scope.
-  Notation "'bn.addc' d , a , b '<<' s , fg" := (Bn_addc d a b (lshift s) fg : insn) (at level 40) : otbn_scope.
-  Notation "'bn.addc' d , a , b '>>' s , fg" := (Bn_addc d a b (rshift s) fg : insn) (at level 40) : otbn_scope.
-  Notation "'bn.sub' d , a , b , fg" := (Bn_sub d a b (lshift 0) fg : insn) (at level 40) : otbn_scope.
-  Notation "'bn.sub' d , a , b '<<' s , fg" := (Bn_sub d a b (lshift s) fg : insn) (at level 40) : otbn_scope.
-  Notation "'bn.sub' d , a , b '>>' s , fg" := (Bn_sub d a b (rshift s) fg : insn) (at level 40) : otbn_scope.
-  Notation "'bn.subb' d , a , b , fg" := (Bn_subb d a b (lshift 0) fg : insn) (at level 40) : otbn_scope.
-  Notation "'bn.subb' d , a , b '<<' s , fg" := (Bn_subb d a b (lshift s) fg : insn) (at level 40) : otbn_scope.
-  Notation "'bn.subb' d , a , b '>>' s , fg" := (Bn_subb d a b (rshift s) fg : insn) (at level 40) : otbn_scope.
-  Notation "'bn.movr' a , b" := (Bn_movr a b : insn) (at level 40) : otbn_scope.
+Section Stringify.
+  Context {word32 : word.word 32}.
+  Context {label : Type} {label_to_string : label -> string}.
+  Local Coercion label_to_string : label >-> string.
 
-  (* Load-store offset notations require special handling to parse the
-     parentheses as actual symbols. Only the most common offsets get
-     notations here, unfortunately; others may need to be written
-     without notation. *)
-  Notation "'bn.lid' a , 0( b )" := (Bn_lid a 0 b : insn) (at level 10) : otbn_scope.
-  Notation "'bn.lid' a , 32( b )" := (Bn_lid a 32 b : insn) (at level 10) : otbn_scope.
-  Notation "'bn.lid' a , 64( b )" := (Bn_lid a 64 b : insn) (at level 10) : otbn_scope.
-  Notation "'bn.lid' a , 96( b )" := (Bn_lid a 96 b : insn) (at level 10) : otbn_scope.
-  Notation "'bn.lid' a , 128( b )" := (Bn_lid a 128 b : insn) (at level 10) : otbn_scope.
-  Notation "'bn.lid' a , 160( b )" := (Bn_lid a 160 b : insn) (at level 10) : otbn_scope.
-  Notation "'bn.lid' a , 192( b )" := (Bn_lid a 192 b : insn) (at level 10) : otbn_scope.
-  Notation "'bn.lid' a , 224( b )" := (Bn_lid a 224 b : insn) (at level 10) : otbn_scope.
+  Definition gpr_to_string (r : gpr) : string :=
+    match r with
+    | x0 => "x0"
+    | x1 => "x1"
+    | x2 => "x2"
+    | x3 => "x3"
+    | x4 => "x4"
+    | x5 => "x5"
+    | x6 => "x6"
+    | x7 => "x7"
+    | x8 => "x8"
+    | x9 => "x9"
+    | x10 => "x10"
+    | x11 => "x11"
+    | x12 => "x12"
+    | x13 => "x13"
+    | x14 => "x14"
+    | x15 => "x15"
+    | x16 => "x16"
+    | x17 => "x17"
+    | x18 => "x18"
+    | x19 => "x19"
+    | x20 => "x20"
+    | x21 => "x21"
+    | x22 => "x22"
+    | x23 => "x23"
+    | x24 => "x24"
+    | x25 => "x25"
+    | x26 => "x26"
+    | x27 => "x27"
+    | x28 => "x28"
+    | x29 => "x29"
+    | x30 => "x30"
+    | x31 => "x31"
+    end.
+  Local Coercion gpr_to_string : gpr >-> string.
 
-  (* Control instructions. *)
-  Notation "'ret'" := (Ret : insn) (at level 40) : otbn_scope.
-  Notation "'ecall'" := (Ecall : insn) (at level 40) : otbn_scope.
-  Notation "'jal' a , addr" := (Jal a addr : insn) (at level 40) : otbn_scope.
-  Notation "'bne' a , b , addr" := (Bne a b addr : insn) (at level 40) : otbn_scope.
-  Notation "'beq' a , b , addr" := (Beq a b addr : insn) (at level 40) : otbn_scope.
-  Notation "'loop' a , len" := (Loop a len : insn) (at level 40) : otbn_scope.
-  Notation "'loopi' a , len" := (Loopi a len : insn) (at level 40) : otbn_scope.
+  Definition csr_to_string (r : csr) : string :=
+    match r with
+    | CSR_FG0 => "CSR_FG0"
+    | CSR_FG1 => "CSR_FG1"
+    | CSR_FLAGS => "CSR_FLAGS"
+    | CSR_RND_PREFETCH => "CSR_RND_PREFETCH"
+    | CSR_RND => "CSR_RND"
+    | CSR_URND => "CSR_URND"
+    end.
+  Local Coercion csr_to_string : csr >-> string.
 
-  (* Tests for instruction notations. *)
-  Check (addi x3, x0, 5)%otbn.
-  Check (addi x3, x0, -5)%otbn.
-  Check (bn.mulqacc w2.0, w3.3, 64)%otbn.
-  Check (bn.mulqacc.wo.z w4, w2.0, w3.3, 64)%otbn.
-  Check (bn.mulqacc.so w4.L, w2.0, w3.3, 64)%otbn.
-  Check (bn.addm w0, w1, w2)%otbn.
-  Check (bn.subm w0, w1, w2)%otbn.
-  Check (bn.add w0, w0, w0, FG0)%otbn.
-  Check (bn.add w20, w20, w20 << 128, FG0)%otbn.
-  Check (bn.add w20, w20, w20 >> 128, FG1)%otbn.
-  Check (bn.addc w0, w0, w0, FG0)%otbn.
-  Check (bn.addc w20, w20, w20 << 128, FG0)%otbn.
-  Check (bn.addc w20, w20, w20 >> 128, FG1)%otbn.
-  Check (bn.sub w0, w0, w0, FG0)%otbn.
-  Check (bn.sub w20, w20, w20 << 128, FG0)%otbn.
-  Check (bn.sub w20, w20, w20 >> 128, FG1)%otbn.
-  Check (bn.subb w0, w0, w0, FG0)%otbn.
-  Check (bn.subb w20, w20, w20 << 128, FG0)%otbn.
-  Check (bn.subb w20, w20, w20 >> 128, FG1)%otbn.
-  Check (bn.movr x20, x21)%otbn.
-  Check (bn.movr x20++, x21)%otbn.
-  Check (bn.movr x20, x21++)%otbn.
-  Check (bn.lid x20, 0(x21))%otbn.
-  Check (bn.lid x20, 32(x21++))%otbn.
-  Check (ret)%otbn.
-  Check (ecall)%otbn.
-  Check (bne x3, x4, 0xfde)%otbn.
-  Check (beq x3, x4, 0x400)%otbn.
-  Check (loop x2, 5)%otbn.
-  Check (loopi 2, 5)%otbn.
-End OtbnNotations.
+  Definition reg_to_string (r : reg) : string :=
+    match r with
+    | gpreg r => r
+    | csreg r => r
+    end.
 
-(*
+  Definition sinsn_to_string (i : sinsn) : string :=
+    match i with
+    | Addi rd rs imm =>
+        "addi " ++ rd ++ ", " ++ rs ++ ", " ++ HexString.of_Z imm
+    | Add rd rs1 rs2 =>
+        "add " ++ rd ++ ", " ++ rs1 ++ ", " ++ rs2
+    | Lw rd rs imm =>
+        "lw" ++ rd ++ ", (" ++ HexString.of_Z imm ++ ")" ++ rs
+    | Sw rs1 rs2 imm =>
+        "sw" ++ rs2 ++ ", (" ++ HexString.of_Z imm ++ ")" ++ rs1
+    | Csrrs rd rs =>
+        "csrrs " ++ rd ++ ", " ++ rs ++ ", "
+    end.
+
+  Definition cinsn_to_string (i : cinsn (label:=label)) : string :=
+    match i with
+    | Ret => "ret"
+    | Ecall => "ecall"
+    | Jal r dst => "jal " ++ r ++ ", " ++ dst
+    | Bne r1 r2 dst => "bne " ++ r1 ++ ", " ++ r2 ++ ", " ++ dst
+    | Beq r1 r2 dst => "beq " ++ r1 ++ ", " ++ r2 ++ ", " ++ dst
+    | Loop r => "loop " ++ r
+    | Loopi n => "loop " ++ HexString.of_nat n
+    | LoopEnd => "loopend"
+    end.
+
+  Definition insn_to_string (i : insn) : string :=
+    match i with
+    | Straightline i => sinsn_to_string i
+    | Control i => cinsn_to_string i
+    end.
+
+End Stringify.
+
+(* bitwise operation shorthand *)
+Local Infix "|'" := Z.lor (at level 40, only parsing) : Z_scope.
+Local Infix "&'" := Z.land (at level 40, only parsing) : Z_scope.
+Local Infix "<<" := Z.shiftl (at level 40, only parsing) : Z_scope.
+Local Infix ">>" := Z.shiftr (at level 40, only parsing) : Z_scope.
+Local Coercion Z.b2z : bool >-> Z.
+
+Section Semantics.
+  Context {word32 : word.word 32} {word256 : word.word 256}.
+  (* Parameterize over the representation of jump locations. *)
+  Context {label : Type}
+    {label_eqb : label -> label -> bool}
+    {label_eqb_spec :
+      forall d1 d2, BoolSpec (d1 = d2) (d1 <> d2) (label_eqb d1 d2)}.
+  Definition advance_pc (pc : label * nat) := (fst pc, S (snd pc)).
+  (* Parameterize over the map implementation. *)
+  Context {regfile : map.map reg word32}
+    {wregfile : map.map wreg word256}
+    {flagfile : map.map flag bool}
+    {mem : map.map word32 word32}
+    {fetch : label * nat -> option (insn (label:=label))}.
+
+  Definition is_valid_addi_imm (imm : Z) : bool :=
+    (-2048 <=? imm) && (imm <=? 2047).
+  Definition is_valid_mem_offset (imm : Z) : bool :=
+    (-2048 <=? imm) && (imm <=? 2047).
+  Definition is_valid_addr (addr : word32) : bool :=
+    word.eqb (word.of_Z 0) (word.and addr (word.of_Z 3))
+    && word.ltu addr (word.of_Z DMEM_BYTES).
+
+  Fixpoint repeat_advance_pc (pc : label * nat) (n : nat) : label * nat :=
+    match n with
+    | O => pc
+    | S n => advance_pc (repeat_advance_pc pc n)
+    end.
+
+  (* OTBN state definition *)
+  Local Notation call_stack := (list (label * nat)) (only parsing).
+  Local Notation loop_stack := (list (label * nat * nat)) (only parsing).
+  Inductive otbn_state : Type :=
+  | otbn_busy
+      (pc : label * nat)      
+      (regs : regfile)
+      (wregs : wregfile)
+      (flags : flagfile)
+      (dmem : mem)
+      (cstack : call_stack)
+      (lstack : loop_stack)
+  | otbn_error (pc : label * nat) (errs : list string)
+  | otbn_done (pc : label * nat) (dmem : mem)
+  .
+  
+  Definition get_pc (st : otbn_state) : label * nat :=
+    match st with
+    | otbn_busy pc _ _ _ _ _ _ => pc
+    | otbn_error pc _ => pc
+    | otbn_done pc _ => pc
+    end.
+
+  (* Code in this section can be used either for execution or for
+     omnisemantics-style proofs depending on the parameters. *) 
+  Section ExecOrProof.
+    Context
+      (* return type: option otbn_state for exec, Prop for proof *)
+      {T}
+        (* error case: None for exec, False for proof *)
+        (err : T)
+        (* construction of randomness: list fetch for exec, (forall v, P v) for proof *)
+        (random : (word32 -> T) -> T)
+        (* construction of pseudorandomness *)
+        (urandom : (word32 -> T) -> T)
+        (* construction for option types:
+             - for exec: match x with | Some x => P x | None => None end
+             - for proof: exists v, x = Some v /\ P v
+        *)
+        (option_bind : forall A, option A -> (A -> T) -> T).
+    Local Arguments option_bind {_}.
+
+    Definition read_gpr (regs : regfile) (r : gpr) (P : word32 -> T) : T :=
+      match r with
+      | x0 => P (word.of_Z 0) (* x0 always reads as 0 *)
+      | x1 =>
+          (* TODO: call stack reads are rare in practice; for now, don't model *)
+          err
+      | _ => option_bind (map.get regs (gpreg r)) P
+      end.
+
+    Definition read_flag_group (group : bool) (flags : flagfile) (P : word32 -> T) : T :=
+      option_bind
+        (map.get flags (flagM group))
+        (fun m =>
+           option_bind
+             (map.get flags (flagL group))
+             (fun l =>
+                option_bind
+                  (map.get flags (flagZ group))
+                  (fun z =>
+                     option_bind
+                       (map.get flags (flagC group))
+                       (fun c =>
+                          let value := Z.b2z c in
+                          let value := Z.lor value (Z.shiftl (Z.b2z z) 1) in
+                          let value := Z.lor value (Z.shiftl (Z.b2z l) 2) in
+                          let value := Z.lor value (Z.shiftl (Z.b2z m) 3) in
+                          P (word.of_Z value))))).
+
+    Definition read_csr
+      (regs : regfile)
+      (flags : flagfile)
+      (r : csr)
+      (P : word32 -> T) : T :=
+      match r with
+      | CSR_FG0 => read_flag_group false flags P
+      | CSR_FG1 => read_flag_group true flags P
+      | CSR_FLAGS =>
+          read_flag_group false flags
+            (fun fg0 =>
+               read_flag_group true flags
+                 (fun fg1 =>
+                    P (word.or fg0 (word.slu fg1 (word.of_Z 4)))))
+      | CSR_RND_PREFETCH => err (* cannot read *)
+      | CSR_RND => random P
+      | CSR_URND => urandom P
+      end.
+
+    Definition read_mem (dmem : mem) (addr : word32) (P : word32 -> T) : T :=
+      if is_valid_addr addr
+      then option_bind (map.get dmem addr) P
+      else err.      
+
+    Definition write_gpr (regs : regfile) (r : gpr) (v : word32) (P : regfile -> T) : T :=
+      match r with
+      | x0 => P regs
+      | x1 =>
+          (* TODO: this should push to the call stack, but is
+             practically never used. For now, don't model this behavior
+             and treat it as an error. *)
+          err
+      | _ => P (map.put regs (gpreg r) v)
+      end.
+
+    Definition extract_flag (v : word32) (f : flag) (P : bool -> T) : T :=
+      match f with
+      | flagC _ => P (word.eqb (word.of_Z 0) (word.and v (word.of_Z 1)))
+      | flagM _ => P (word.eqb (word.of_Z 0) (word.and v (word.of_Z 2)))
+      | flagL _ => P (word.eqb (word.of_Z 0) (word.and v (word.of_Z 4)))
+      | flagZ _ => P (word.eqb (word.of_Z 0) (word.and v (word.of_Z 8)))
+      end.
+
+    Definition write_flag_group
+      (group : bool)
+      (flags : flagfile)
+      (v : word32)
+      (P : flagfile -> T) : T :=
+      extract_flag v (flagC group)
+        (fun c =>
+           extract_flag v (flagM group)
+             (fun m =>
+                extract_flag v (flagL group)
+                  (fun l =>
+                     extract_flag v (flagZ group)
+                       (fun z =>
+                          let flags := map.put flags (flagC group) c in
+                          let flags := map.put flags (flagM group) m in
+                          let flags := map.put flags (flagL group) l in
+                          let flags := map.put flags (flagZ group) z in
+                          P flags)))).
+
+    Definition write_csr
+      (regs : regfile)
+      (flags : flagfile)
+      (r : csr)
+      (v : word32)
+      (P : regfile -> flagfile -> T) : T :=
+      match r with
+      | CSR_FG0 => write_flag_group false flags v (fun flags => P regs flags)
+      | CSR_FG1 => write_flag_group true flags v (fun flags => P regs flags)
+      | CSR_FLAGS =>
+          write_flag_group false flags v
+            (fun flags =>
+               write_flag_group true flags (word.sru v (word.of_Z 4))
+                 (fun flags => P regs flags))
+      | CSR_RND_PREFETCH => P regs flags (* no effect on this model *)
+      | CSR_RND => P regs flags (* writes ignored *)
+      | CSR_URND => P regs flags (* writes ignored *)
+      end.
+
+    Definition write_mem (dmem : mem) (addr v : word32) (P : mem -> T) : T :=
+      if is_valid_addr addr
+      then P (map.put dmem addr v)
+      else err.
+
+    Definition addi_spec (v : word32) (imm : Z) : word32 :=
+      if (0 <=? imm)
+      then word.add v (word.of_Z imm)
+      else word.sub v (word.of_Z imm).
+
+    Definition strt1
+      (regs : regfile) (wregs : wregfile) (flags : flagfile) (dmem : mem)
+      (i : sinsn) (post : regfile -> wregfile -> flagfile -> mem -> T) : T :=
+      match i with
+      | Addi d x imm =>
+          if is_valid_addi_imm imm
+          then
+            read_gpr regs x
+              (fun vx =>
+                 write_gpr regs d (addi_spec vx imm)
+                   (fun regs => post regs wregs flags dmem))
+          else err
+      | Add d x y =>
+          read_gpr regs x
+            (fun vx =>
+               read_gpr regs y
+                 (fun vy =>
+                    write_gpr regs d (word.add vx vy)
+                      (fun regs => post regs wregs flags dmem)))
+      | Lw d x imm =>
+          if is_valid_mem_offset imm
+          then read_gpr regs x
+                 (fun vx =>
+                    read_mem dmem (word.add vx (word.of_Z imm))
+                      (fun vm =>
+                         write_gpr regs d vm
+                           (fun regs => post regs wregs flags dmem)))
+          else err
+      | Sw x y imm =>
+          if is_valid_mem_offset imm
+          then read_gpr regs x
+                 (fun vx =>
+                    (read_gpr regs y
+                       (fun vy =>
+                          write_mem dmem (word.add vx (word.of_Z imm)) vy
+                            (fun dmem => post regs wregs flags dmem))))
+          else err
+      | Csrrs d x =>
+          read_gpr regs x
+            (fun vx =>
+               read_csr regs flags d
+                 (fun vd =>
+                    write_csr regs flags d (word.xor vd vx)
+                      (fun regs flags =>
+                         write_gpr regs x vd
+                           (fun regs => post regs wregs flags dmem))))
+      end.
+
+    (* Pop an address off the call stack and jump to that location. *)
+    Definition call_stack_pop (st : otbn_state) (post : otbn_state -> T) : T :=
+      match st with
+      | otbn_busy pc regs wregs flags dmem cstack lstack =>
+          option_bind (hd_error cstack)
+                      (fun dst => post (otbn_busy dst regs wregs flags dmem (tl cstack) lstack))
+      | _ => post st
+      end.
+
+    (* Push the next (one-advanced) PC onto the call stack. *)
+    Definition call_stack_push (st : otbn_state) (post : otbn_state -> T) : T :=
+      match st with
+      | otbn_busy pc regs wregs flags dmem cstack lstack =>
+          if (length cstack <? 8)%nat
+          then post (otbn_busy pc regs wregs flags dmem ((advance_pc pc) :: cstack) lstack)
+          else err
+      | _ => post st
+      end.
+    Definition program_exit (st : otbn_state) (post : otbn_state -> T) : T :=
+      match st with
+      | otbn_busy pc regs wregs flags dmem cstack lstack => post (otbn_done pc dmem)
+      | _ => post st
+      end.
+    Definition set_pc
+      (st : otbn_state) (pc : label * nat) (post : otbn_state -> T) : T :=
+      match st with
+      | otbn_busy _ regs wregs flags dmem cstack lstack =>
+          post (otbn_busy pc regs wregs flags dmem cstack lstack)
+      | _ => post st
+      end.
+    Definition update_state
+      (st : otbn_state)
+      (regs : regfile)
+      (wregs : wregfile)
+      (flags : flagfile)
+      (dmem : mem)
+      (post : otbn_state -> T) : T :=
+      match st with
+      | otbn_busy pc _ _ _ _ cstack lstack =>
+          post (otbn_busy pc regs wregs flags dmem cstack lstack)
+      | _ => post st
+      end.
+    Definition next_pc (st : otbn_state) (post : otbn_state -> T) : T :=
+      match st with
+      | otbn_busy pc regs wregs flags dmem cstack lstack =>
+          post (otbn_busy (advance_pc pc) regs wregs flags dmem cstack lstack)
+      | _ => post st
+      end.
+    Definition read_gpr_from_state (st : otbn_state) (r : gpr) (post : _ -> T) : T :=
+      match st with
+      | otbn_busy _ regs _ _ _ _ _ => read_gpr regs r post
+      | _ => err
+      end.
+
+    (* Begin a new loop. *)
+    Definition loop_start
+      (st : otbn_state) (iters : nat) (post : otbn_state -> T) : T :=
+      match iters with
+      | O => err (* iters cannot be zero *)
+      | S iters =>
+          match st with
+          | otbn_busy pc regs wregs flags dmem cstack lstack =>          
+              let start_pc := advance_pc pc in
+              if (length lstack <? 8)%nat
+              then post (otbn_busy
+                           start_pc regs wregs flags dmem cstack
+                           ((start_pc, iters) :: lstack))
+              else err
+          | _ => err
+          end
+      end.
+
+    (* Finish a loop iteration (and potentially the entire loop).
+       Expects that the current PC matches the loop-body end PC of the
+       first loop stack entry. *)
+    Definition loop_end (st : otbn_state) (post : otbn_state -> T) : T :=
+      match st with
+      | otbn_busy pc regs wregs flags dmem cstack lstack =>
+          option_bind (hd_error lstack)
+                      (fun start_iters =>
+                             match (snd start_iters) with
+                             | O => post (otbn_busy
+                                            (advance_pc pc) regs wregs flags dmem cstack
+                                            (tl lstack))
+                             | S iters =>
+                                 post (otbn_busy
+                                         (fst start_iters) regs wregs flags dmem cstack
+                                         ((fst start_iters, iters) :: tl lstack))
+                             end)
+      | _ => err
+      end.
+    
+  (* TODO: is it necessary to simulate some error conditions? There
+     should be a difference between "OTBN had an error", which
+     sometimes should in fact happen on some inputs, and "this program
+     is not valid" (e.g. out-of-bounds immediate value that cannot be
+     encoded). *)
+  Definition ctrl1
+    (st : otbn_state) (i : cinsn (label:=label))
+    (post : otbn_state -> T) : T :=
+    match i with
+    | Ret =>  call_stack_pop st post
+    | Ecall => program_exit st post
+    | Jal r dst =>
+        match r with
+        | x0 => set_pc st (dst, 0%nat) post
+        | x1 => call_stack_push st (fun st => set_pc st (dst, 0%nat) post)
+        | _ =>
+            (* technically it is possible to write the PC to other
+               registers but practically this is almost never done, so
+               for now we don't model it *)
+            err
+        end
+    | Bne r1 r2 dst =>
+        read_gpr_from_state st r1
+          (fun v1 =>
+             read_gpr_from_state st r2
+               (fun v2 =>
+                  if (word.eqb v1 v2)
+                  then next_pc st post
+                  else set_pc st (dst, 0%nat) post))
+    | Beq r1 r2 dst =>
+        read_gpr_from_state st r1
+          (fun v1 =>
+             read_gpr_from_state st r2
+               (fun v2 =>
+                  if (word.eqb v1 v2)
+                  then set_pc st (dst, 0%nat) post
+                  else next_pc st post))
+    | Loopi v => loop_start st v post
+    | Loop r => read_gpr_from_state st r
+                  (fun v => loop_start st (Z.to_nat (word.unsigned v)) post)
+    | LoopEnd => loop_end st post
+    end.
+  End ExecOrProof.
+  Definition prop_random (P : word32 -> Prop) : Prop := forall v, P v.
+  Definition prop_urandom (P : word32 -> Prop) : Prop := forall v, P v.
+  Definition prop_option_bind (A : Type) (x : option A) (P : A -> Prop) : Prop :=
+    exists v, x = Some v /\ P v.
+
+  (* Prop model for proofs *)
+  Definition run1 (st : otbn_state) (post : otbn_state -> Prop) : Prop :=
+    match st with
+    | otbn_busy pc regs wregs flags dmem cstack lstack =>
+        exists i,
+        fetch pc = Some i
+        /\ match i with
+           | Straightline i =>
+               strt1 False prop_random prop_urandom prop_option_bind
+                 regs wregs flags dmem i
+                 (fun regs wregs flags dmem =>
+                    update_state st regs wregs flags dmem
+                      (fun st => set_pc st (advance_pc pc) post))
+           | Control i => ctrl1 False prop_option_bind st i post
+           end
+    | _ => post st
+    end.
+
+  (* For now, we don't model RND in the executable model. It would
+     theoretically be possible by e.g. plugging in a "next random" at
+     every exec1. *)
+  Definition exec_random (P : word32 -> option otbn_state)
+    : option otbn_state := None.
+  Definition exec_urandom (P : word32 -> option otbn_state)
+    : option otbn_state := None.
+  Definition exec_option_bind
+    (A : Type) (x : option A) (P : A -> option otbn_state) : option otbn_state :=
+    match x with
+    | Some v => P v
+    | None => None
+    end.
+
+  (* Fully executable model. *)
+  Definition exec1 (st : otbn_state) : option otbn_state :=
+    match st with
+    | otbn_busy pc regs wregs flags dmem cstack lstack =>
+        match fetch pc with
+        | Some (Straightline i) =>
+            strt1 None exec_random exec_urandom exec_option_bind
+              regs wregs flags dmem i
+              (fun regs wregs flags dmem =>
+                 update_state st regs wregs flags dmem
+                   (fun st => set_pc st (advance_pc pc) Some))
+        | Some (Control i) => ctrl1 None exec_option_bind st i Some
+        | None => None
+        end
+    | _ => Some st
+    end.
+
+  Definition is_busy (st : otbn_state) : bool :=
+    match st with
+    | otbn_busy _ _ _ _ _ _ _ => true
+    | _ => false
+    end.
+  Fixpoint exec (st : otbn_state) (fuel : nat) : option otbn_state :=
+    match fuel with
+    | O => None
+    | S fuel =>
+        match exec1 st with
+        | Some st =>
+            if is_busy st
+            then exec st fuel
+            else Some st
+        | None => None
+        end        
+    end.
+End Semantics.
+
 Section ErrorMonad.
   (* returns either a value or an error message, helpful for debugging *)
   Definition maybe (A : Type) : Type := A + string.
@@ -270,6 +725,12 @@ Section ErrorMonad.
     | b :: l =>
         bind (f x b) (maybe_fold_left f l)
     end.
+  Fixpoint maybe_flat_map {A B} (f : A -> maybe (list B)) (l : list A) : maybe (list B) :=
+    match l with
+    | [] => inl []
+    | a :: l =>
+        bind (f a) (fun l1 => bind (maybe_flat_map f l) (fun l2 => inl (l1 ++ l2)))
+    end.
   Definition assertion (cond : bool) (msg : string) : maybe unit :=
     if cond then inl tt else inr msg.
 End ErrorMonad.
@@ -278,1214 +739,2668 @@ Module ErrorMonadNotations.
   Notation Ok := inl (only parsing).
   Notation "'Err' x" := (inr x%string) (at level 20, only parsing).
 End ErrorMonadNotations.
-Import ErrorMonadNotations.
- *)
 
-Section CpsMonad.
-  Definition bind {A B C} (x : (A -> C) -> C) (f : A -> (B -> C) -> C) : (B -> C) -> C :=
-    fun P => x (fun a => f a P).
-  Definition ret {A B} (a : A) (P : A -> B) : B := P a.
-End CpsMonad.
-Module CpsMonadNotations.
-  Notation "a <- b ; c" := (bind b (fun a => c)) (at level 100, right associativity).
-  Notation Ok := inl (only parsing).
-  Notation "'Err' x" := (inr x%string) (at level 20, only parsing).
-End CpsMonadNotations.
-Import CpsMonadNotations.
+Require Import coqutil.Map.SortedListZ.
+Require Import coqutil.Map.SortedListString.
+Local Coercion Straightline : sinsn >-> insn.
+Local Coercion Control : cinsn >-> insn.
 
-Module CpsMonadTest.
-  Local Definition add_cps (a b : nat) (P : nat -> Prop) : Prop :=
-    let ab := (a + b)%nat in
-    P ab.
+(* Contains a way to link programs. *)
+Section Build.
+  (* TODO: how should we now represent programs? All we need is fetch. *)
+  (* option: map from string -> list insn, so that all labels
+     that are jumped to need an entry. The list insns can
+     overlap. Execution should not pass the end. *)
+  (* Can this cause problems with cycles or too much redundancy? *)
+  (* option: list insns * map from string -> nat, return tail of list always *)
+  (* this is nice from a representation redundancy perspective *)
+  (* how about reasoning with objs? *)
+  (* different fetch, multiple copies of list insns * map from string -> nat to choose from *)
+  (* or maybe each obj needs to be considered separately? *)
+  Definition symbols : map.map string nat := SortedListString.map _.
+  Import ErrorMonadNotations.
 
-  Eval cbv beta iota delta [add_cps] in
-    (fun a b c d e =>
-       add_cps a b
-         (fun w => add_cps w c
-                     (fun x => add_cps x d
-                                 (fun y => add_cps y e
-                                             (fun z => z = y))))).
-  Eval cbv beta iota delta [add_cps] in
-    (fun a b c d e =>
-       (w <- add_cps a b ;
-        x <- add_cps w c ;
-        y <- add_cps x d ;
-        z <- add_cps y e ;
-        ret (z = y))).
+  (* Functions consist of a name, internal labels (map of string ->
+     offset within the function), and a list of instructions. *)
+  Definition function : Type := string * symbols * list (insn (label:=string)).
+  (* Programs are lists of instructions that link to each other with
+     offsets within the global program. This represents code
+     post-linking. *)
+  Definition program : Type := list (insn (label:=nat)).
 
-  Local Fixpoint mul_cps (a b : nat) : (nat -> Prop) -> Prop :=
-    match b with
-    | O => ret 0%nat
-    | S b =>
-        x <- mul_cps a b ;
-        add_cps x a
+  Definition add_symbol (syms : symbols) (label : string) (offset : nat)
+    : maybe symbols :=
+    match map.get syms label with
+    | Some _ => Err ("Symbol " ++ label ++ " appears more than once.")
+    | None => Ok (map.put syms label offset)
     end.
 
-  Goal (forall a, mul_cps a 5 (fun x => x = 5 * a))%nat.
-  Proof.
-    intros. cbv beta iota delta [mul_cps add_cps bind ret].
-    cbn. lia.
-  Qed.
-End CpsMonadTest.
+  Definition merge_symbols
+    (global_offset : nat) (global_syms fn_syms : symbols) : maybe symbols :=
+    map.fold
+      (fun global_syms label fn_offset =>
+         (global_syms <- global_syms ;
+          add_symbol global_syms label (global_offset + fn_offset)))
+      (Ok global_syms) fn_syms.
 
+  (* Returns the symbols plus the overall size of the program *)
+  Definition link_symbols_for_function
+    (syms_offset : symbols * nat) (fn : function) : maybe (symbols * nat) :=
+    let fn_name := fst (fst fn) in
+    let fn_syms := snd (fst fn) in
+    let fn_insns := snd fn in
+    (syms <- add_symbol (fst syms_offset) fn_name (snd syms_offset) ;
+     syms <- merge_symbols (snd syms_offset) syms fn_syms ;
+     Ok (syms, (snd syms_offset + length fn_insns)%nat)).
+  Definition link_symbols'
+    (start_syms : symbols)
+    (start_offset : nat)
+    (fns : list function)
+    : maybe (symbols * nat) :=
+    maybe_fold_left link_symbols_for_function fns (start_syms, start_offset).
+  Definition link_symbols (fns : list function) : maybe symbols :=
+    (syms_offset <- link_symbols' map.empty 0%nat fns ;
+     Ok (fst syms_offset)).
 
-(* Boilerplate definitions for comparing registers. *)
-Section RegisterEquality.
-  Local Ltac derive_eqb r1 r2 :=
-    pose r1 as x1;
-    pose r2 as x2;
-    destruct r1, r2;
-    lazymatch goal with
-    | x1 := ?x, x2 := ?x |- _ => clear; exact true
-    | _ => clear; exact false
-    end.
-  
-  Definition gpr_eqb (r1 r2 : gpr) : bool.
-  Proof. derive_eqb r1 r2. Defined.
-  Definition csr_eqb (r1 r2 : csr) : bool.
-  Proof. derive_eqb r1 r2. Defined.
-  Definition wdr_eqb (r1 r2 : wdr) : bool.
-  Proof. derive_eqb r1 r2. Defined.
-  Definition wsr_eqb (r1 r2 : wsr) : bool.
-  Proof. derive_eqb r1 r2. Defined.
-
-  Local Ltac prove_eqb_spec r1 r2 :=
-    destruct r1, r2; cbv [gpr_eqb]; constructor; congruence.
-  Lemma gpr_eqb_spec : forall r1 r2, BoolSpec (r1 = r2) (r1 <> r2) (gpr_eqb r1 r2).
-  Proof. prove_eqb_spec r1 r2. Qed.
-  Lemma csr_eqb_spec : forall r1 r2, BoolSpec (r1 = r2) (r1 <> r2) (csr_eqb r1 r2).
-  Proof. prove_eqb_spec r1 r2. Qed.
-  Lemma wdr_eqb_spec : forall r1 r2, BoolSpec (r1 = r2) (r1 <> r2) (wdr_eqb r1 r2).
-  Proof. prove_eqb_spec r1 r2. Qed.
-  Lemma wsr_eqb_spec : forall r1 r2, BoolSpec (r1 = r2) (r1 <> r2) (wsr_eqb r1 r2).
-  Proof. prove_eqb_spec r1 r2. Qed.
-End RegisterEquality.
-
-(* bitwise operation shorthand *)
-Local Infix "|'" := Z.lor (at level 40, only parsing) : Z_scope.
-Local Infix "&'" := Z.land (at level 40, only parsing) : Z_scope.
-Local Infix "<<" := Z.shiftl (at level 40, only parsing) : Z_scope.
-Local Infix ">>" := Z.shiftr (at level 40, only parsing) : Z_scope.
-Local Coercion Z.b2z : bool >-> Z.
-
-(* Executable model of OTBN. *)
-Section Exec.
-  (* Parameterize over the representation of code locations. *)
-  Context {addr : Type}
-    {error_addr : addr}
-    {advance_pc : addr -> addr}
-    {addr_eqb : addr -> addr -> bool}
-    {addr_eqb_spec : forall a1 a2, BoolSpec (a1 = a2) (a1 <> a2) (addr_eqb a1 a2)}.
-
-  (* error values for cases that should be unreachable *)
-  Context {error_Z : Z} {error_bool : bool}.
-
-  (* Parameterize over the map implementation. *)
-  Context {regfile : map.map reg Z}
-    {flagfile : map.map flag bool}
-    {mem : map.map Z Z}
-    {blockmap : map.map addr (list sinsn * option (cinsn (addr:=addr)))}.
-
-  (* Really, I want to talk about terminal states -- either a return
-     from the subroutine, the end of the program, or an error.
-
-     straightline needs/edits only regs, flags, dmem --> but can error
-     control needs/edits callstack, loopstack, pc, needs regs --> can also error 
-
-     need to process through, come out with a Prop in the end via cps style passing
-     the prop gives you rnd reasoning much easier
-   *)
-  (* mulqacc shifts must be positive multiples of 64 *)
-  Definition is_valid_mul_shift (s : Z) : Prop :=
-    s = 0 \/ s = 64 \/ s = 128 \/ s = 192.
-  (* rshi shifts must be in the range [0,255] *)
-  Definition is_valid_rshi_imm (s : Z) : Prop := 0 <= s < 256.
-  (* other shift immediates must be multiples of 8 and in the range [0,248] *)
-  Definition is_valid_arith_shift (s : shift) : Prop :=
-    let s := match s with
-             | lshift x => x
-             | rshift x => x
-             end in
-    (s mod 8 = 0) /\ 0 <= s < 256.
-  (* immediates for addi must be in the range [-2048, 2047] *)
-  Definition is_valid_addi_imm (imm : Z) : Prop :=
-    -2048 <= imm <= 2047.
-  (* offsets for loads and stores are in the range [-16384, 16352] in steps of 32 *)
-  Definition is_valid_mem_offset (offset : Z) : Prop :=
-    -16384 <= offset <= 16352.
-
-  (*
-  (* mulqacc shifts must be positive multiples of 64 *)
-  Definition to_valid_mul_shift (s : Z) : Z :=
-    Z.shiftl (Z.land (Z.shiftr (Z.abs s) 6) 3) 6.
-  (* rshi shifts must be in the range [0,255] *)
-  Definition to_valid_rshi_imm (s : Z) : Z := Z.land (Z.abs s) 255.
-  (* other shift immediates must be multiples of 8 and in the range [0,248] *)
-  Definition to_valid_arith_shift (s : shift) : Z :=
-    let s := match s with
-             | lshift x => x
-             | rshift x => x
-             end in
-    Z.shiftl (Z.land (Z.shiftr (Z.abs s) 3) 31) 3.
-  (* immediates for addi must be in the range [-2048, 2047] *)
-  (* TODO: this implementation cuts off the very lowest value, -2048 *)
-  Definition to_valid_addi_imm (imm : Z) : Z :=
-    if 0 <=? imm
-    then Z.land imm 2047
-    else - (Z.land (-imm) 2047).
-  (* offsets for loads and stores are in the range [-16384, 16352] in steps of 32 *)
-  (* TODO: this implementation cuts off the very lowest value, -16384 *)
-  Definition to_valid_mem_offset (offset : Z) : Z :=
-    if 0 <=? offset
-    then Z.shiftl (Z.land (Z.shiftr offset 5) 511) 5
-    else - Z.shiftl (Z.land (Z.shiftr (- offset) 5) 511) 5.
-   *)
-  Definition read_gpr (regs : regfile) (r : gpr) : option Z :=
-    match r with
-    | x0 => Some 0 (* x0 always reads as 0 *)
-    | x1 =>
-        (* TODO: call stack reads are rare in practice; for now, don't model *)
-        None
-    | _ => map.get regs (gpreg r)
-    end.
-
-  Definition read_wdr (regs : regfile) (r : wdr) : option Z :=
-    map.get regs (wdreg r).
-
-  Definition read_wsr (regs : regfile) (r : wsr) (P : Z -> Prop) : Prop :=
-    match r with
-    | RND => forall r, P r
-    | URND => forall u, P u
-    | _ => exists v, map.get regs (wsreg r) = Some v /\ P v
-    end.
-
-  Definition read_flag (flags : flagfile) (f : flag) : option bool :=
-    map.get flags f.
-
-  (* Assemble a group of flags into an integer value. *)
-  Definition read_flag_group (flags : flagfile) (fg : flag_group) (P : Z -> Prop) : Prop :=
-    exists c m l z,
-      read_flag flags (flagC fg) = Some c
-      /\ read_flag flags (flagM fg) = Some m
-      /\ read_flag flags (flagL fg) = Some l
-      /\ read_flag flags (flagZ fg) = Some z
-      /\ P (c |' (m << 1) |' (l << 2) |' (z << 3)).
-
-  Definition read_csr (flags : flagfile) (r : csr) (P : Z -> Prop) : Prop :=
-    match r with
-    | CSR_FG0 => read_flag_group flags FG0 P
-    | CSR_FG1 => read_flag_group flags FG1 P
-    | CSR_FLAGS =>
-        read_flag_group flags FG0
-          (fun fg0 => read_flag_group flags FG1
-                        (fun fg1 => P (fg0 |' (fg1 << 4))))
-    end.
-
-  Definition wdr_for_limb (l : limb) : wdr :=
-    match l with
-    | limb0 r => r
-    | limb1 r => r
-    | limb2 r => r
-    | limb3 r => r
-    end.
-  Definition get_limb (l : limb) (v : Z) :=
-    match l with
-    | limb0 r => (v          &' Z.ones 64)
-    | limb1 r => ((v >> 64 ) &' Z.ones 64)
-    | limb2 r => ((v >> 128) &' Z.ones 64)
-    | limb3 r => ((v >> 192) &' Z.ones 64)
-    end.
-
-  Definition cast32 (v : Z) : Z := v &' Z.ones 32.
-  Definition cast256 (v : Z) : Z := v &' Z.ones 256.
-
-  Definition write_gpr (regs : regfile) (r : gpr) (v : Z) : (regfile -> Prop) -> Prop :=
-    match r with
-    | x0 => ret regs
-    | x1 =>
-        (* TODO: this should push to the call stack, but is
-           practically never used. For now, don't model this behavior
-           and treat it as an error. *)
-        fun _ => False
-    | _ => ret (map.put regs (gpreg r) (cast32 v))
-    end.
-
-  Definition write_wdr (regs : regfile) (r : wdr) (v : Z) : regfile :=
-    map.put regs (wdreg r) (cast256 v).
-  Definition write_wsr (regs : regfile) (r : wsr) (v : Z) : regfile :=
-    match r with
-    | RND => regs (* writes to RND are ignored *)
-    | URND => regs (* writes to URND are ignored *)
-    | _ => map.put regs (wsreg r) (cast256 v)
-    end.
-
-  (* specifications for complex operations (may make proofs a little nicer) *)
-  Definition mulqacc_spec (acc x y s : Z) : Z :=
-    acc + (x * y) << s.
-  Definition addm_spec (x y m : Z) : Z :=
-    let r := x + y in
-    if r >? m then r - m else r.
-  Definition subm_spec (x y m : Z) : Z :=
-    let r := x - y in
-    if r <? 0 then r + m else r.
-  Definition rshi_spec (x y imm : Z) : Z :=
-    let xy := Z.lor (x << 256) y in
-    xy >> imm.
-
-  Definition run1
-    (regs : regfile) (flags : flagfile) (dmem : mem)
-    (i : sinsn) (post : regfile -> flagfile -> mem -> Prop) : Prop :=
+  Definition link_cinsn
+    (syms : map.rep (map:=symbols)) (i : cinsn (label:=string))
+    : maybe (cinsn (label:=nat)) :=
     match i with
-    | Addi d x imm =>
-        is_valid_addi_imm imm /\
-          (exists v,
-              read_gpr regs x = Some v
-              /\ write_gpr regs d (v + imm)
-                   (fun regs => post regs flags dmem))
-    | Bn_mulqacc z x y s =>
-        is_valid_mul_shift s
-        /\ let regs := if z then write_wsr regs ACC 0 else regs in
-           (exists vx vy,
-               read_wdr regs (wdr_for_limb x) = Some vx
-               /\ read_wdr regs (wdr_for_limb y) = Some vy
-               /\ read_wsr regs ACC
-                    (fun acc =>
-                       let x := get_limb x vx in
-                       let y := get_limb y vy in
-                       let r := mulqacc_spec acc x y s in
-                       let regs := write_wsr regs ACC r in
-                       post regs flags dmem))
-    | Bn_mulqacc_wo z d x y s =>
-        is_valid_mul_shift s
-        /\ let regs := if z then write_wsr regs ACC 0 else regs in
-           (exists vx vy,
-               read_wdr regs (wdr_for_limb x) = Some vx
-               /\ read_wdr regs (wdr_for_limb y) = Some vy
-               /\ read_wsr regs ACC
-                    (fun acc =>
-                       let x := get_limb x vx in
-                       let y := get_limb y vy in
-                       let r := mulqacc_spec acc x y s in
-                       let regs := write_wsr regs ACC r in
-                       let regs := write_wdr regs d r in
-                       post regs flags dmem))
-    | _ => False
+    | Ret => Ok Ret
+    | Ecall => Ok Ecall
+    | Jal r dst =>
+        (dst <- map_err (map.get syms dst) ("Label " ++ dst ++ " not found (jal)");
+         Ok (Jal r dst))
+    | Bne r1 r2 dst =>
+        (dst <- map_err (map.get syms dst) ("Label " ++ dst ++ " not found (bne)");
+         Ok (Bne r1 r2 dst))
+    | Beq r1 r2 dst =>
+        (dst <- map_err (map.get syms dst) ("Label " ++ dst ++ " not found (beq)");
+         Ok (Beq r1 r2 dst))
+    | Loop r => Ok (Loop r)
+    | Loopi imm => Ok (Loopi imm)
+    | LoopEnd => Ok LoopEnd
     end.
 
-  Goal (map.ok regfile ->
-        run1
-           (map.put map.empty (gpreg x2) 5)
-           map.empty map.empty
-           (Addi x3 x2 4)
-           (fun r f d =>
-              run1 r f d
-                (Addi x4 x3 (-4))
-                (fun r f d => read_gpr r x4 = Some 5))).
+  Definition link_insn
+    (syms : symbols) (i : insn (label:=string))
+    : maybe (insn (label:=nat)) :=
+    match i with
+    | Straightline i => Ok (Straightline i)
+    | Control i =>
+        (i <- link_cinsn syms i ;
+         Ok (Control i))
+    end.
+
+  Fixpoint link_insns
+    (syms : symbols) (insns : list (insn (label:=string)))
+    : maybe (list (insn (label:=nat))) :=
+    match insns with
+    | [] => Ok []
+    | i :: insns =>
+        (i <- link_insn syms i ;
+         insns <- link_insns syms insns ;
+         Ok (i :: insns))
+    end.
+
+  Definition link'
+    (syms : symbols) (prog : program) (fn : function) : maybe program :=
+    (fn_insns <- link_insns syms (snd fn) ;
+     Ok (prog ++ fn_insns)).
+
+  Definition link (fns : list function) : maybe program :=
+    (syms <- link_symbols fns ;
+     maybe_fold_left (link' syms) fns []).
+
+  Definition get_label_offset
+    (fn : function) (label : string) : option nat :=
+    let fn_name := fst (fst fn) in
+    let fn_syms := snd (fst fn) in
+    if (String.eqb label fn_name)
+    then Some 0%nat
+    else map.get fn_syms label.
+
+  (* Fetch from a function. *)
+  Definition fetch_fn
+    (fn : function) (pc : string * nat) : option insn :=
+    let label := fst pc in
+    let offset := snd pc in
+    let fn_insns := snd fn in
+    match get_label_offset fn label with
+    | None => None
+    | Some label_offset => nth_error fn_insns (label_offset + offset)
+    end.
+ 
+  (* Fetch from a collection of functions. *)
+  Definition fetch_ctx
+    (fns : list function) (pc : string * nat) : option insn :=
+    fold_left
+      (fun res fn =>
+         match res, fetch_fn fn pc with
+         | None, Some i => Some i
+         | _,_ => res
+         end)
+      fns None.
+
+  (* Fetch from a whole program. *)
+  Definition fetch
+    (prog : program) (pc : nat * nat) : option insn :=
+    let global_offset := fst pc in
+    let fn_offset := snd pc in
+    nth_error prog (global_offset + fn_offset).
+
+  Definition cinsn_equiv (syms : symbols)
+    (i1 : cinsn (label:=string))
+    (i2 : cinsn (label:=nat)) : Prop :=
+    match i1, i2 with
+    | Ret, Ret => True
+    | Ecall, Ecall => True
+    | Jal r1 dst1, Jal r2 dst2 =>
+        r1 = r2 /\ map.get syms dst1 = Some dst2
+    | Bne a1 b1 dst1, Bne a2 b2 dst2 =>
+        a1 = a2 /\ b1 = b2 /\ map.get syms dst1 = Some dst2
+    | Beq a1 b1 dst1, Beq a2 b2 dst2 =>
+        a1 = a2 /\ b1 = b2 /\ map.get syms dst1 = Some dst2
+    | Loop r1, Loop r2 => r1 = r2
+    | Loopi n1, Loopi n2 => n1 = n2
+    | LoopEnd, LoopEnd => True
+    | _, _ => False
+    end.
+    
+  (* States that a pre-link instruction and post-link instructions are
+     equivalent under a given symbol mapping. *)
+  Definition insn_equiv (syms : symbols)
+    (i1 : insn (label:=string))
+    (i2 : insn (label:=nat)) : Prop :=
+    match i1, i2 with
+    | Straightline i1, Straightline i2 => i1 = i2
+    | Control i1, Control i2 => cinsn_equiv syms i1 i2
+    | _, _ => False
+    end.
+
+  (* States that a particular (pre-link) function is linked into a
+     particular program at the given global offset. *)
+  Definition linked_at
+    (prog : program) (syms : symbols)
+    (fn : function) (global_offset : nat) : Prop :=
+    forall fn_offset : nat,
+      (fn_offset < length (snd fn))%nat ->
+      exists i1 i2,
+        fetch_fn fn (fst (fst fn), fn_offset) = Some i1
+        /\ fetch prog (global_offset, fn_offset) = Some i2
+        /\ insn_equiv syms i1 i2.
+
+End Build.
+
+Instance symbols_ok : map.ok symbols := (SortedListString.ok nat).
+
+Section BuildProofs.
+  Context {word32 : word.word 32} {regfile : map.map reg word32}.
+  Context {word256 : word.word 256} {wregfile : map.map wreg word256}.
+  Context {flagfile : map.map flag bool} {mem : map.map word32 word32}.
+  Import ErrorMonadNotations.
+
+  (* Returns the overall size of the program containing the functions
+     and starting at the given offset. *)
+  Definition program_size (start : nat) (fns : list function) : nat :=
+    fold_left
+      (fun offset fn =>
+         let fn_insns := snd fn in
+          (offset + length fn_insns)%nat)
+      fns start.
+
+  Ltac err_simpl_step :=
+    lazymatch goal with
+    | H : inl ?a = inl ?b |- _ => assert (a = b) by congruence; clear H; subst
+    | H : inl _ = inr _ |- _ => congruence
+    | H : inr _ = inl _ |- _ => congruence
+    | H : (?a, ?b) = (?c, ?d) |- _ =>
+        assert (a = c) by congruence;
+        assert (b = d) by congruence;
+        clear H; subst
+    | H : context [bind ?x] |- _ => destr x; cbn [bind] in H
+    | |- context [bind ?x] => destr x; cbn [bind]
+    | _ => progress cbn [bind] in *
+    end.
+  Ltac err_simpl := repeat err_simpl_step.
+
+  Lemma link_symbols'_step :
+    forall start_syms start_offset fn fns syms1 syms2 end_offset1 end_offset2,
+      link_symbols_for_function (start_syms, start_offset) fn = Ok (syms1, end_offset1) ->
+      link_symbols' syms1 end_offset1 fns = Ok (syms2, end_offset2) ->
+      link_symbols' start_syms start_offset (fn :: fns) = Ok (syms2, end_offset2).
+  Proof.
+    cbv [link_symbols']; intros; cbn [maybe_fold_left bind]; err_simpl; congruence.
+  Qed.
+
+  Lemma link_symbols'_offset :
+    forall fns start_syms start_offset syms end_offset,
+      link_symbols' start_syms start_offset fns = Ok (syms, end_offset) ->
+      end_offset = program_size start_offset fns.
+  Proof.
+    cbv [link_symbols' program_size]; induction fns; cbn [maybe_fold_left fold_left]; intros;
+      err_simpl; [ reflexivity | ].
+    destruct_products; cbn [fst snd] in *.
+    lazymatch goal with
+    | H : link_symbols_for_function _ _ = _ |- _ => cbv [link_symbols_for_function] in H
+    end.
+    err_simpl; cbn [fst snd] in *. eauto.
+  Qed.
+  
+  Lemma link_symbols'_inv :
+    forall start_syms start_offset fn fns syms2 end_offset2,
+      link_symbols' start_syms start_offset (fn :: fns) = Ok (syms2, end_offset2) ->
+      exists syms1 end_offset1,
+        link_symbols_for_function (start_syms, start_offset) fn = Ok (syms1, end_offset1)
+        /\ end_offset2 = program_size end_offset1 fns
+        /\ link_symbols' syms1 end_offset1 fns = Ok (syms2, end_offset2).
+  Proof.
+    cbv [link_symbols']; cbn [maybe_fold_left bind]; intros; err_simpl.
+    destruct_products; cbn [fst snd] in *.
+    repeat lazymatch goal with
+           | H : context [link_symbols_for_function ?a ?b]
+             |- context [link_symbols_for_function ?a ?b] =>
+               destruct (link_symbols_for_function a b) as [[? ?]|]; cbn [bind]
+           | |- exists _, _ => eexists
+           | |- _ /\ _ => split
+           | _ => solve [eauto using link_symbols'_offset]
+           end.    
+  Qed.
+
+  Lemma link_symbols_for_function_size :
+    forall fn start_syms start_offset syms size,
+      link_symbols_for_function (start_syms, start_offset) fn = Ok (syms, size) ->
+      size = (start_offset + length (snd fn))%nat.
+  Proof.
+    cbv [link_symbols_for_function]; intros; err_simpl; reflexivity.
+  Qed.
+
+  Lemma link_symbols'_size :
+    forall fns start_syms start_offset syms end_offset,
+      link_symbols' start_syms start_offset fns = Ok (syms, end_offset) ->
+      program_size start_offset fns = end_offset.
+  Proof.
+    cbv [program_size]; induction fns; intros;
+      [ cbn [link_symbols' maybe_fold_left] in *; err_simpl; reflexivity | ].
+    cbn [fold_left].
+    repeat lazymatch goal with
+           | H : link_symbols' _ _ (_ :: _) = Ok _ |- _ =>
+               eapply link_symbols'_inv in H
+           | H: link_symbols_for_function _ _ = Ok _ |- _ =>               
+               apply link_symbols_for_function_size in H; subst
+           | H : exists _, _ |- _ => destruct H
+           | H : _ /\ _ |- _ => destruct H
+           | _ => subst; solve [eauto]
+           end.
+  Qed.
+
+  Lemma add_symbol_no_overwrite start_syms label1 label_offset1 syms :
+    add_symbol start_syms label1 label_offset1 = Ok syms ->
+    (forall label2 label_offset2,
+        map.get start_syms label2 = Some label_offset2 ->
+        map.get syms label2 = Some label_offset2).
+  Proof.
+    cbv [add_symbol]; intros.
+    destr (map.get start_syms label1); [ congruence | ].
+    destr (string_dec label1 label2); subst; [ congruence | ].
+    err_simpl. rewrite map.get_put_diff by congruence.
+    auto.
+  Qed.
+
+  Lemma add_symbol_fail start_syms label label_offset1 label_offset2 :
+    map.get start_syms label = Some label_offset1 ->
+    exists msg,
+      add_symbol start_syms label label_offset2 = Err msg.
+  Proof.
+    cbv [add_symbol]; intros. destruct_one_match; try congruence.
+    eauto.
+  Qed.
+
+  Lemma merge_symbols_no_overwrite fn_syms global_offset global_syms :
+    forall syms,
+      merge_symbols global_offset global_syms fn_syms = Ok syms ->
+      (forall label label_offset,
+          map.get global_syms label = Some label_offset ->
+          map.get syms label = Some label_offset).
+  Proof.
+    cbv [merge_symbols].
+    lazymatch goal with
+    | |- forall syms,
+        map.fold _ _ _ = ?x -> ?Q =>
+        apply (map.fold_spec (fun _ m => forall syms, m = x -> Q))
+    end; intros; err_simpl; eauto using add_symbol_no_overwrite.
+  Qed.
+
+  Lemma link_symbols_for_function_no_overwrite :
+    forall fn start_syms start_offset syms label label_offset end_offset,
+      link_symbols_for_function (start_syms, start_offset) fn = Ok (syms, end_offset) ->
+      map.get start_syms label = Some label_offset ->
+      map.get syms label = Some label_offset.
+  Proof.
+    destruct fn as [[fn_name fn_syms] fn_insns].
+    cbv [link_symbols_for_function]; cbn [bind fst snd]; intros.
+    err_simpl. eauto using add_symbol_no_overwrite, merge_symbols_no_overwrite.
+  Qed.
+
+  Lemma link_symbols_for_function_name_fail :
+    forall fn start_syms start_offset name label_offset,
+      name = fst (fst fn) ->
+      map.get start_syms name = Some label_offset ->
+      exists msg,
+        link_symbols_for_function (start_syms, start_offset) fn = Err msg.
+  Proof.
+    destruct fn as [[fn_name fn_syms] fn_insns].
+    cbv [link_symbols_for_function]; cbn [bind fst snd]; intros.
+    subst. lazymatch goal with H : map.get _ _ = Some _ |- _ =>
+                                 eapply add_symbol_fail in H; destruct H end.
+    rewrite H. err_simpl. eauto.
+  Qed.
+
+  Lemma link_symbols'_no_overwrite :
+    forall fns start_syms start_offset syms label label_offset end_offset,
+      link_symbols' start_syms start_offset fns = Ok (syms, end_offset) ->
+      map.get start_syms label = Some label_offset ->
+      map.get syms label = Some label_offset.
+  Proof.
+    cbv [program_size]; induction fns; intros;
+      [ cbn [link_symbols' maybe_fold_left] in *; err_simpl; solve [auto] | ].
+    repeat lazymatch goal with
+           | H : link_symbols' _ _ (_ :: _) = Ok _ |- _ =>
+               eapply link_symbols'_inv in H
+           | H : exists _, _ |- _ => destruct H; subst
+           | H : _ /\ _ |- _ => destruct H; subst
+           | _ => solve [eauto using link_symbols_for_function_no_overwrite]
+           end.
+  Qed.
+
+  Lemma link_symbols'_name_fail fn name :
+    forall fns start_syms start_offset label_offset,
+      In fn fns ->
+      name = fst (fst fn) ->
+      map.get start_syms name = Some label_offset ->
+      exists msg,
+        link_symbols' start_syms start_offset fns = Err msg.
+  Proof.
+    cbv [program_size link_symbols']; induction fns; cbn [In]; intros;
+      repeat lazymatch goal with
+        | H : False |- _ => contradiction H
+        | H : _ \/ _ |- _ => destruct H
+        | H : map.get _ _ = Some _ |- context [link_symbols_for_function _ fn] =>
+            eapply link_symbols_for_function_name_fail in H; [ | reflexivity .. ];
+            destruct H as [? H]; rewrite H; err_simpl; solve [eauto]
+        | _ => progress (cbn [maybe_fold_left]; subst)
+        end; [ ].
+    err_simpl; eauto.
+    destruct_products; cbn [fst snd] in *.
+    eauto using link_symbols_for_function_no_overwrite.
+  Qed.
+
+  Lemma add_symbol_correct start_syms label label_offset syms :
+      add_symbol start_syms label label_offset = Ok syms ->
+      map.get syms label = Some label_offset.
+  Proof.
+    cbv [add_symbol]; destruct_one_match; intros; err_simpl; auto using map.get_put_same.
+  Qed.
+
+  Lemma merge_symbols_correct fn_syms global_offset global_syms :
+    forall syms,
+      merge_symbols global_offset global_syms fn_syms = Ok syms ->
+      (forall label label_offset,
+          map.get fn_syms label = Some label_offset ->
+          map.get syms label = Some (global_offset + label_offset)%nat).
+  Proof.
+    cbv [merge_symbols].
+    apply map.fold_spec.
+    { intros. rewrite map.get_empty in *. congruence. }
+    { intros. err_simpl.
+      repeat lazymatch goal with
+             | H : map.get (map.put _ ?x _) ?y = Some _ |- _ =>
+                 destr (String.eqb x y);
+                 [ rewrite map.get_put_same in H
+                 | rewrite map.get_put_diff in H by congruence ]
+             | H : Some _ = Some _ |- _ => inversion H; clear H; subst
+             end;
+        eauto using add_symbol_correct, add_symbol_no_overwrite. }
+  Qed.
+
+  Lemma get_label_offset_name fn name :
+    name = fst (fst fn) ->
+    get_label_offset fn name = Some 0%nat.
+  Proof.
+    intros; subst. cbv [get_label_offset].
+    destruct_one_match; congruence.
+  Qed.
+
+  Lemma link_symbols_for_function_correct
+    fn start_syms start_offset syms end_offset dst fn_offset :
+      link_symbols_for_function (start_syms, start_offset) fn = Ok (syms, end_offset) ->
+      get_label_offset fn dst = Some fn_offset ->
+      map.get syms dst = Some (start_offset + fn_offset)%nat.
+  Proof.
+    destruct fn as [[fn_name fn_syms] fn_insns].
+    cbv [link_symbols_for_function get_label_offset].
+    cbn [bind fst snd]; intros; err_simpl.
+    destruct_one_match_hyp; [ | solve [eauto using merge_symbols_correct] ].
+    lazymatch goal with
+    | H : Some _ = Some _ |- _ => inversion H; clear H; subst
+    end.
+    rewrite Nat.add_0_r.
+    eauto using add_symbol_correct, merge_symbols_no_overwrite.
+  Qed.
+
+  Lemma link_symbols_for_function_name fn start_syms start_offset syms end_offset :
+      link_symbols_for_function (start_syms, start_offset) fn = Ok (syms, end_offset) ->
+      map.get syms (fst (fst fn)) = Some start_offset.
+  Proof.
+    intros. replace start_offset with (start_offset + 0)%nat by lia.
+    eapply link_symbols_for_function_correct; eauto; [ ].
+    apply get_label_offset_name; reflexivity.
+  Qed.
+
+  Lemma link_symbols'_correct :
+    forall fns1 fns2 fn start_syms start_offset syms end_offset fn_offset dst,
+    link_symbols' start_syms start_offset (fns1 ++ fn :: fns2) = inl (syms, end_offset) ->
+    get_label_offset fn dst = Some fn_offset ->
+    map.get syms dst = Some (program_size start_offset fns1 + fn_offset)%nat.
+  Proof.
+    cbv [program_size]; induction fns1; intros.
+    { rewrite ?app_nil_l in *. cbn [link_symbols' maybe_fold_left] in *.
+      err_simpl. destruct_products.
+      eauto using link_symbols'_no_overwrite, link_symbols_for_function_correct. }
+    { rewrite <-?app_comm_cons in *. cbn [fold_left].
+      repeat lazymatch goal with
+             | H : link_symbols' _ _ (_ :: _) = Ok _ |- _ =>
+                 eapply link_symbols'_inv in H
+             | H: link_symbols_for_function _ _ = Ok _ |- _ =>               
+                 apply link_symbols_for_function_size in H; subst
+             | H : exists _, _ |- _ => destruct H
+             | H : _ /\ _ |- _ => destruct H
+             | _ => subst; solve [eauto]                                 
+             end. }
+  Qed.
+
+  Lemma link_symbols'_name :
+    forall fns1 fns2 fn start_syms start_offset syms end_offset,
+      link_symbols' start_syms start_offset (fns1 ++ fn :: fns2) = Ok (syms, end_offset) ->
+      map.get syms (fst (fst fn)) = Some (program_size start_offset fns1).
+  Proof.
+    intros.
+    replace (program_size start_offset fns1)
+      with (program_size start_offset fns1 + 0)%nat by lia.
+    eapply link_symbols'_correct; eauto using get_label_offset_name.
+  Qed.
+
+  Lemma link_cinsn_correct syms i1 i2 : 
+    link_cinsn syms i1 = Ok i2 ->
+    cinsn_equiv syms i1 i2.
+  Proof.
+    cbv [link_cinsn cinsn_equiv]; intros.
+    destruct_one_match; err_simpl; ssplit; auto;
+      lazymatch goal with
+      | H : map_err (map.get ?m ?k) _ = Ok _ |- _ =>
+          destr (map.get m k); cbn [map_err] in H; err_simpl
+      end; reflexivity.
+  Qed.
+
+  Lemma link_insn_correct syms i1 i2 : 
+    link_insn syms i1 = Ok i2 ->
+    insn_equiv syms i1 i2.
+  Proof.
+    cbv [link_insn insn_equiv]; intros.
+    destruct_one_match; err_simpl; eauto using link_cinsn_correct.
+  Qed.
+
+  Lemma link_insns_correct :
+    forall syms fn_insns prog,
+      link_insns syms fn_insns = Ok prog ->
+      forall (fn_offset : nat),
+        (fn_offset < length fn_insns)%nat ->
+        exists i1 i2,
+          nth_error fn_insns fn_offset = Some i1
+          /\ nth_error prog fn_offset = Some i2
+          /\ insn_equiv syms i1 i2.
+  Proof.
+    induction fn_insns; intros; cbn [link_insns length] in *; err_simpl; [ lia | ].
+    destr fn_offset; cbn [nth_error].
+    { do 2 eexists; ssplit; try reflexivity; eauto using link_insn_correct. }
+    { apply IHfn_insns; auto; lia. }
+  Qed.
+
+  Lemma fetch_fn_name offset (fn : function) :
+    fetch_fn fn (fst (fst fn), offset) = nth_error (snd fn) offset.
+  Proof.
+    cbv [fetch_fn get_label_offset]. cbn [fst snd].
+    rewrite String.eqb_refl, Nat.add_0_l. reflexivity.
+  Qed.
+  
+  Lemma fetch_fn_sym fn label offset label_offset :
+    label <> fst (fst fn) ->
+    map.get (snd (fst fn)) label = Some label_offset ->
+    fetch_fn fn (label, offset) = nth_error (snd fn) (label_offset + offset).
+  Proof.
+    destruct fn as [[fn_name fn_syms] fn_insns].
+    cbv [fetch_fn get_label_offset]; cbn [fst snd]; intros.
+    destr (label =? fn_name)%string; [ congruence | ].
+    destruct_one_match; congruence.
+  Qed.
+
+  Lemma linked_at_cons i prog syms fn offset :
+    linked_at prog syms fn offset ->
+    linked_at (i :: prog) syms fn (S offset).
+  Proof.
+    cbv [linked_at]; cbn [fst snd]. intro Hlink; intros.
+    specialize (Hlink _ ltac:(eassumption)). destruct_products.
+    eauto.
+  Qed.
+
+  Lemma link'_correct :
+    forall start_prog fn prog syms offset,
+      link' syms start_prog fn = Ok prog ->
+      offset = length start_prog ->
+      linked_at prog syms fn offset.
+  Proof.
+    cbv [link']; induction start_prog; intros; subst.
+    { err_simpl. rewrite app_nil_l in *. cbn [length].
+      cbv [linked_at]; intros.
+      lazymatch goal with H : link_insns _ _ = _ |- _ =>
+                            eapply link_insns_correct in H; eauto end.
+      destruct_products. cbn [fst snd].
+      rewrite fetch_fn_name. cbv [fetch]; cbn [fst snd].
+      eauto. }
+    { err_simpl. rewrite <-app_comm_cons. cbn [length].
+      apply linked_at_cons. apply IHstart_prog; auto; err_simpl.
+      reflexivity. }
+  Qed.
+
+  Lemma link'_no_unlink :
+    forall fn1 fn2 syms offset start_prog prog,
+      link' syms start_prog fn2 = Ok prog ->
+      linked_at start_prog syms fn1 offset ->
+      linked_at prog syms fn1 offset.
+  Proof.
+    cbv [link']; intros. err_simpl. cbv [linked_at]; intros.
+    lazymatch goal with H : linked_at _ _ _ _ |- _ =>
+                          specialize (H _ ltac:(eassumption))
+    end.
+    destruct_products. do 2 eexists; ssplit; eauto; [ ].
+    cbv [fetch] in *; cbn [fst snd] in *.
+    lazymatch goal with
+    | H : nth_error ?l1 ?i = Some _ |- _ =>
+        assert (i < length l1)%nat by eauto using List.nth_error_Some_bound_index
+    end.
+    rewrite nth_error_app1 by lia. auto.
+  Qed.
+
+  Lemma fold_link'_no_unlink :
+    forall fns fn syms offset start_prog prog,
+      maybe_fold_left (link' syms) fns start_prog = Ok prog ->
+      linked_at start_prog syms fn offset ->
+      linked_at prog syms fn offset.
+  Proof.
+    induction fns; cbn [maybe_fold_left]; intros; err_simpl;
+      eauto using link'_no_unlink.
+  Qed.
+
+  Lemma link_insns_length :
+    forall syms insns prog,
+    link_insns syms insns = Ok prog ->
+    length prog = length insns.
+  Proof.
+    induction insns; cbn [link_insns length]; intros; err_simpl; [ reflexivity | ].
+    cbn [length]. rewrite IHinsns; eauto.
+  Qed.
+
+  Lemma link'_length syms start_prog fn prog:
+    link' syms start_prog fn = Ok prog ->
+    length prog = (length start_prog + length (snd fn))%nat.
+  Proof.
+    cbv [link']. destruct fn as [[fn_name fn_syms] fn_insns]. cbn [fst snd].
+    intros; err_simpl. rewrite app_length.
+    lazymatch goal with H : link_insns _ _ = _ |- _ => apply link_insns_length in H end.
+    lia.
+  Qed.
+
+  Lemma link_correct'' :
+    forall fns1 fn fns2 start_syms start_offset start_prog syms prog end_offset,
+      maybe_fold_left (link' syms) (fns1 ++ fn :: fns2) start_prog = inl prog ->
+      link_symbols' start_syms start_offset (fns1 ++ fn :: fns2) = inl (syms, end_offset) ->
+      start_offset = length start_prog ->
+      linked_at prog syms fn (program_size start_offset fns1).
+  Proof.
+    cbv [program_size]. induction fns1; intros; subst.
+    { rewrite app_nil_l in *. cbn [maybe_fold_left fold_left fst snd] in *.
+      err_simpl. eauto using link'_correct, fold_link'_no_unlink. }
+    { rewrite <-?app_comm_cons in *. cbn [fold_left maybe_fold_left] in *.
+      err_simpl.
+      repeat lazymatch goal with
+             | H : link_symbols' _ _ (_ :: _) = Ok _ |- _ =>
+                 eapply link_symbols'_inv in H
+             | H: link_symbols_for_function _ _ = Ok _ |- _ =>               
+                 apply link_symbols_for_function_size in H; subst
+             | H : exists _, _ |- _ => destruct H
+             | H : _ /\ _ |- _ => destruct H
+             | _ => progress subst                           
+             end.
+      eapply IHfns1; eauto; [ ].
+      cbv [function] in *; destruct_products; cbn [fst snd] in *.
+      lazymatch goal with H : link' _ _ _ = _ |- _ => apply link'_length in H end.
+      cbn [fst snd] in *. lia. }
+  Qed.
+
+  Lemma link_correct' fns1 fns2 fn prog syms :
+      link (fns1 ++ fn :: fns2) = Ok prog ->
+      link_symbols (fns1 ++ fn :: fns2) = Ok syms ->
+      linked_at prog syms fn (program_size 0%nat fns1).
+  Proof.
+    cbv [link link_symbols]; intros. err_simpl.
+    destruct_products; cbn [fst snd] in *.
+    eauto using link_correct''.    
+  Qed.
+
+  Lemma link_correct :
+    forall fns fn prog syms,
+      (* If the function is in the input list of functions `fns`... *)
+      In fn fns ->
+      (* ...and `prog` is the result of a successful `link`... *)
+      link fns = Ok prog ->
+      (* ..and `syms` is the symbol table for `fns`... *)
+      link_symbols fns = Ok syms ->
+      (* ...then there exists an `offset` and an index `idx`... *)
+      exists offset idx,
+        (* ...such that `fn` is in the list at index `idx`...  *)
+        nth_error fns idx = Some fn
+        (* ...and `offset` is the size of the program before `fn`... *)
+        /\ offset = program_size 0%nat (firstn idx fns)
+        (* ...and `fn` is linked at `offset`. *)
+        /\ linked_at prog syms fn offset.
+  Proof.
+    intros.
+    lazymatch goal with H : In _ _ |- _ =>
+                          apply in_split in H; destruct H as [fns1 [fns2 ?]]
+    end.
+    subst. eexists; exists (length fns1); ssplit; [ | reflexivity | ].
+    { rewrite nth_error_app2, Nat.sub_diag by lia. reflexivity. }
+    { rewrite List.firstn_app_l by lia. eauto using link_correct'. }
+  Qed.
+
+  (* Convenience shorthand for defining function specs. *)
+  Definition returns
+    {label : Type} {fetch:label * nat -> option insn}
+    (start : label) regs wregs flags dmem cstack lstack
+    (spec : regfile -> wregfile -> flagfile -> mem -> Prop) : Prop :=
+    forall ret_pc,
+      hd_error cstack = Some ret_pc ->
+      eventually
+        (run1 (fetch:=fetch))
+        (fun st =>
+           match st with
+           | otbn_busy pc regs' wregs' flags' dmem' cstack' lstack' =>
+               pc = ret_pc
+               /\ spec regs' wregs' flags' dmem'
+               /\ cstack' = tl cstack
+               /\ lstack' = lstack
+           | _ => False
+           end)
+        (otbn_busy (start, 0%nat) regs wregs flags dmem cstack lstack).
+  Definition exits
+    {label : Type} {fetch: label * nat -> option insn}
+    (start : label) regs wregs flags dmem cstack lstack
+    (spec : mem -> Prop) (err_spec : _ -> Prop)
+    : Prop :=
+    eventually
+      (run1 (fetch:=fetch))
+      (fun st =>
+         match st with
+         | otbn_done pc dmem => spec dmem
+         | otbn_error pc errs => err_spec errs
+         | _ => False
+         end)
+      (otbn_busy (start, 0%nat) regs wregs flags dmem cstack lstack).
+
+  Definition pcs_related (syms : symbols) (pc1 : string * nat) (pc2 : nat * nat) : Prop :=
+    map.get syms (fst pc1) = Some (fst pc2) /\ snd pc1 = snd pc2.
+  Definition loop_stack_entries_related (syms : symbols) (e1 : _ * nat) (e2 : _ * nat) : Prop :=
+    pcs_related syms (fst e1) (fst e2) /\ snd e1 = snd e2.
+  Definition states_related (syms : symbols)
+    (st1 : otbn_state (label:=string)) (st2 : otbn_state (label:=nat)) : Prop :=
+    match st1, st2 with
+    | otbn_busy pc1 regs1 wregs1 flags1 dmem1 cstack1 lstack1,
+      otbn_busy pc2 regs2 wregs2 flags2 dmem2 cstack2 lstack2 =>
+        pcs_related syms pc1 pc2
+        /\ regs1 = regs2
+        /\ wregs1 = wregs2
+        /\ flags1 = flags2
+        /\ dmem1 = dmem2
+        /\ Forall2 (pcs_related syms) cstack1 cstack2
+        /\ Forall2 (loop_stack_entries_related syms) lstack1 lstack2
+    | otbn_done pc1 dmem1, otbn_done pc2 dmem2 =>
+        pcs_related syms pc1 pc2
+        /\ dmem1 = dmem2
+    | otbn_error pc1 errs1, otbn_error pc2 errs2 =>
+        pcs_related syms pc1 pc2
+        /\ errs1 = errs2
+    | _, _ => False
+    end.
+
+  Lemma fetch_ctx_done :
+    forall fns dst i,
+      fold_left (fun res fn =>
+                   match res, fetch_fn fn dst with
+                   | None, Some i => Some i
+                   | _, _ => res
+                   end) fns (Some i) = Some i.
+  Proof.
+    induction fns; cbn [fold_left]; [ reflexivity | ].
+    intros. apply IHfns.
+  Qed.
+
+  Lemma fetch_fn_Some fn pc i :
+      fetch_fn fn pc = Some i ->
+      exists offset,
+        get_label_offset fn (fst pc) = Some offset
+        /\ nth_error (snd fn) (offset + snd pc) = Some i.
+  Proof.
+    cbv [fetch_fn]. destruct_one_match; [ | congruence ].
+    intros. eexists; ssplit; [ reflexivity .. | ].
+    assumption.
+  Qed.
+
+  Lemma fetch_ctx_Some :
+    forall fns pc i,
+      fetch_ctx fns pc = Some i ->    
+      exists fn,
+        fetch_fn fn pc = Some i
+        /\ In fn fns.
+  Proof.
+    cbv [fetch_ctx].
+    induction fns as [|fn fns]; cbn [fold_left]; [ congruence | ].
+    intros. destruct_one_match_hyp.
+    { rewrite fetch_ctx_done in *.
+      lazymatch goal with H : Some _ = Some _ |- _ => inversion H; clear H; subst end.
+      eexists; ssplit; eauto using in_eq. }
+    { repeat lazymatch goal with
+             | H : _ /\ _ |- _ => destruct H
+             | H : exists _, _ |- _ => destruct H
+             | H : fold_left _ _ None = Some _ |- _ => apply IHfns in H
+             end.
+      eexists; ssplit; eauto using in_cons. }
+  Qed.
+
+  Lemma link_symbols_correct fns fn syms fn_offset dst n :
+    link_symbols fns = inl syms ->
+    nth_error fns n = Some fn ->
+    get_label_offset fn dst = Some fn_offset ->
+    map.get syms dst = Some (program_size 0 (firstn n fns) + fn_offset)%nat.
+  Proof.
+    cbv [link_symbols]. intros. err_simpl. destruct_products.
+    Search nth_error app.
+    repeat lazymatch goal with
+           | H : nth_error _ _ = Some _ |- _ =>
+               apply nth_error_split in H
+           | H : _ /\ _ |- _ => destruct H
+           | H : exists _, _ |- _ => destruct H
+           end.
+    subst. rewrite List.firstn_app_l by reflexivity. cbn [fst snd].
+    eauto using link_symbols'_correct.
+  Qed.
+
+  Lemma link_fetch syms prog fns pc1 pc2 i1 :
+    link fns = Ok prog ->
+    link_symbols fns = Ok syms ->
+    pcs_related syms pc1 pc2 ->
+    fetch_ctx fns pc1 = Some i1 ->
+    exists i2,
+      fetch prog pc2 = Some i2
+      /\ insn_equiv syms i1 i2.
+  Proof.
+    cbv [pcs_related]; intros.
+    repeat lazymatch goal with
+           | H : _ /\ _ |- _ => destruct H
+           | H : exists _, _ |- _ => destruct H
+           | H : fetch_ctx _ _ = Some _ |- _ => apply fetch_ctx_Some in H
+           end.
+    pose proof (link_correct _ _ _ _ ltac:(eassumption) ltac:(eassumption) ltac:(eassumption)).
+    repeat lazymatch goal with
+           | H : _ /\ _ |- _ => destruct H; subst
+           | H : exists _, _ |- _ => destruct H
+           | H : fetch_fn ?fn (fst (fst ?fn), _) = Some _ |- _ => rewrite fetch_fn_name in H
+    
+           | H : fetch_fn _ _ = Some _ |- _ => apply fetch_fn_Some in H
+           | H : @nth_error insn _ ?n = Some _, H' : linked_at _ _ _ _ |- _ =>
+               specialize (H' n ltac:(eauto using List.nth_error_Some_bound_index))
+           end.
+
+    lazymatch goal with
+    | H : nth_error ?l ?i = Some ?x, H' : nth_error ?l ?i = Some ?y |- _ =>
+        assert (x = y) by congruence; subst
+    end.
+ 
+    pose proof (link_symbols_correct
+                  _ _ _ _ _ _
+                  ltac:(eassumption) ltac:(eassumption) ltac:(eassumption)).
+    lazymatch goal with
+    | H : map.get ?m ?k = Some ?x, H' : map.get ?m ?k = Some ?y |- _ =>
+        assert (x = y) by congruence; subst
+    end.
+
+    lazymatch goal with
+    | H : fetch prog _ = Some ?i |- _ => exists i
+    end.
+    ssplit; [ | assumption .. ].
+    destruct_products.
+    cbv [fetch] in *. cbn [fst snd] in *. subst.
+    lazymatch goal with
+    | H : _ = Some ?x |- _ = Some ?x => rewrite <-H
+    end.
+    repeat (f_equal; try lia).
+  Qed.
+
+  Lemma read_gpr_weaken regs r P Q :
+    read_gpr False prop_option_bind regs r P ->
+    (forall regs, P regs -> Q regs) ->
+    read_gpr False prop_option_bind regs r Q.
+  Proof.
+    cbv [read_gpr prop_option_bind]; intros; destruct_one_match;
+      repeat lazymatch goal with
+        | H : exists _, _ |- _ => destruct H
+        | H : _ /\ _ |- _ => destruct H
+        | H : False |- _ => contradiction H
+        | |- exists _, _ => eexists; ssplit; [ eassumption | ]
+        | |- Q _ => solve [eauto]
+        end.
+  Qed.
+
+  Lemma read_csr_weaken regs flags r P Q :
+    read_csr False prop_random prop_urandom prop_option_bind regs flags r P ->
+    (forall regs, P regs -> Q regs) ->
+    read_csr False prop_random prop_urandom prop_option_bind regs flags r Q.
+  Proof.
+    cbv [read_csr read_flag_group prop_random prop_urandom prop_option_bind]; intros.
+    destruct r;
+      repeat lazymatch goal with
+        | H : exists _, _ |- _ => destruct H
+        | H : _ /\ _ |- _ => destruct H
+        | H : False |- _ => contradiction H
+        | |- exists _, _ => eexists; ssplit; [ eassumption | ]
+        | _ => solve [eauto]
+        end.
+  Qed.
+
+  Lemma read_mem_weaken dmem addr P Q :
+    read_mem False prop_option_bind dmem addr P ->
+    (forall dmem, P dmem -> Q dmem) ->
+    read_mem False prop_option_bind dmem addr Q.
+  Proof.
+    cbv [read_mem prop_option_bind]; intros.
+    destruct_one_match;
+      repeat lazymatch goal with
+        | H : exists _, _ |- _ => destruct H
+        | H : _ /\ _ |- _ => destruct H
+        | H : False |- _ => contradiction H
+        | |- exists _, _ => eexists; ssplit; [ eassumption | ]
+        | _ => solve [eauto]
+        end.
+  Qed.
+
+  Lemma write_gpr_weaken regs r v P Q :
+    write_gpr False regs r v P ->
+    (forall regs, P regs -> Q regs) ->
+    write_gpr False regs r v Q.
+  Proof.
+    cbv [write_gpr]; intros; destruct_one_match;
+      repeat lazymatch goal with
+        | H : exists _, _ |- _ => destruct H
+        | H : _ /\ _ |- _ => destruct H
+        | H : False |- _ => contradiction H
+        | |- exists _, _ => eexists; ssplit; [ eassumption | ]
+        | |- Q _ => solve [eauto]
+        end.
+  Qed.
+
+  Lemma write_csr_weaken regs flags r v P Q :
+    write_csr (T:=Prop) regs flags r v P ->
+    (forall regs flags, P regs flags -> Q regs flags) ->
+    write_csr (T:=Prop) regs flags r v Q.
+  Proof.
+    cbv [write_csr write_flag_group extract_flag]; intros; destruct_one_match; eauto.
+  Qed.
+
+  Lemma write_mem_weaken dmem addr v P Q :
+    write_mem False dmem addr v P ->
+    (forall dmem, P dmem -> Q dmem) ->
+    write_mem False dmem addr v Q.
+  Proof.
+    cbv [write_mem]; intros; destruct_one_match; eauto.
+  Qed.
+
+  Lemma strt1_weaken regs wregs flags dmem i P Q :
+    strt1 False prop_random prop_urandom prop_option_bind
+      regs wregs flags dmem i P ->
+    (forall regs wregs flags dmem, P regs wregs flags dmem -> Q regs wregs flags dmem) ->
+    strt1 False prop_random prop_urandom prop_option_bind
+      regs wregs flags dmem i Q.
+  Proof.
+    cbv [strt1]; intros; repeat destruct_one_match;
+      repeat lazymatch goal with
+        | H : exists _, _ |- _ => destruct H
+        | H : _ /\ _ |- _ => destruct H
+        | H : False |- _ => contradiction H
+        | |- exists _, _ => eexists; ssplit; [ eassumption | ]
+        | |- read_gpr _ _ _ _ _ =>
+            eapply read_gpr_weaken; [ eassumption | ]; cbv beta; intros
+        | |- read_csr _ _ _ _ _ _ _ _ =>
+            eapply read_csr_weaken; [ eassumption | ]; cbv beta; intros
+        | |- read_mem _ _ _ _ _ =>
+            eapply read_mem_weaken; [ eassumption | ]; cbv beta; intros
+        | |- write_gpr _ _ _ _ _ =>
+            eapply write_gpr_weaken; [ eassumption | ]; cbv beta; intros
+        | |- write_csr _ _ _ _ _ =>
+            eapply write_csr_weaken; [ eassumption | ]; cbv beta; intros
+        | |- write_mem _ _ _ _ _ =>
+            eapply write_mem_weaken; [ eassumption | ]; cbv beta; intros
+        | |- Q _ _ _ _ => solve [eauto]
+        end.
+  Qed.
+
+  Ltac related_states_hammer :=
+    cbn [states_related] in *;
+      repeat lazymatch goal with
+        | H : False |- _ => contradiction H
+        | H : exists _, _ |- _ => destruct H
+        | H : _ /\ _ |- _ => destruct H; subst
+        | H : forall st1' st2', _ st1' st2' -> _ st1' -> ?spec2 st2' |- ?spec2 _ =>
+            eapply H; [ | eassumption ]
+        | H : Forall2 _ (_ :: _) _ |- _ =>
+            inversion H; clear H; subst; cbn [hd_error tl] in *
+        | H : context [match ?x with _ => _ end] |- _ => destruct_one_match_hyp
+        | |- context [match ?x with _ => _ end] => destruct_one_match
+        | H : hd_error ?l = Some _ |- _ =>
+            destruct l; cbn [hd_error tl] in *                                               
+        | H : Some _ = Some _ |- _ => inversion H; clear H; subst
+        | H : None = Some _ |- _ => exfalso; congruence
+        | |- pcs_related _ _ _ =>
+            progress cbv [advance_pc pcs_related] in *; cbn [fst snd]; ssplit; eauto
+        | |- loop_stack_entries_related _ _ _ =>
+            progress cbv [loop_stack_entries_related] in *; ssplit
+        | |- states_related _ _ _ =>
+            progress cbv [states_related]; try contradiction; ssplit; eauto
+        | H: Forall2 _ ?l1 ?l2,
+            H0 : (length ?l1 < ?n)%nat, H1 : (?n <= length ?l2)%nat |- _ =>
+            pose proof (Forall2_length H); lia
+        | |- Forall2 _ (_ :: _) (_ :: _) => constructor
+        | |- read_gpr _ _ _ _ _ =>
+            eapply read_gpr_weaken; [ eassumption | ]; cbv beta; intros
+        | |- read_csr _ _ _ _ _ _ _ _ =>
+            eapply read_csr_weaken; [ eassumption | ]; cbv beta; intros
+        | |- write_gpr _ _ _ _ _ =>
+            eapply write_gpr_weaken; [ eassumption | ]; cbv beta; intros
+        | |- write_csr _ _ _ _ _ =>
+            eapply write_csr_weaken; [ eassumption | ]; cbv beta; intros
+        | |- exists _, _ =>
+            eexists; ssplit; first [ eassumption
+                                   | reflexivity
+                                   | solve [related_states_hammer] ]
+        | _ => first [ progress (cbv [call_stack_pop call_stack_push
+                                        loop_start loop_end loop_stack_entries_related
+                                        read_gpr_from_state next_pc
+                                        set_pc update_state program_exit] in *;
+                                 cbn [fst snd] in *; subst )
+                     | congruence
+                     | solve [eauto] ]
+        end.
+
+  Lemma ctrl1_weaken syms i1 i2 st1 st2 spec1 spec2 :
+    ctrl1 (label:=string) False prop_option_bind st1 i1 spec1 ->
+    states_related syms st1 st2 ->
+    cinsn_equiv syms i1 i2 ->
+    (forall st1' st2', states_related syms st1' st2' -> spec1 st1' -> spec2 st2') ->
+    ctrl1 (label:=nat) False prop_option_bind st2 i2 spec2.
+  Proof.
+    cbv [ctrl1 cinsn_equiv prop_option_bind]; intros.
+    destruct st1, st2; related_states_hammer.
+  Qed.
+
+  (* prove that run1 on related states produces a related state *)
+  Lemma link_run1 fns prog syms st1 st2 spec1 spec2 :
+      link fns = Ok prog ->
+      link_symbols fns = Ok syms ->
+      states_related syms st1 st2 ->
+      (forall st1' st2',
+          states_related syms st1' st2' ->
+          spec1 st1' ->
+          spec2 st2') ->
+      run1 (fetch:=fetch_ctx fns) st1 spec1 ->
+      run1 (fetch:=fetch prog) st2 spec2.
   Proof.
     cbv [run1].
+    destruct st1, st2; cbn [states_related]; try contradiction; intros;
+      repeat lazymatch goal with
+        | H : exists _, _ |- _ => destruct H
+        | H : _ /\ _ |- _ => destruct H
+        | H : fetch_ctx _ _ = Some _ |- _ => eapply link_fetch in H; [ | eassumption .. ]
+        | H : forall st1' st2',
+            states_related _ st1' st2' ->
+              spec1 st1' ->
+              spec2 st2' |- spec2 _ =>
+            eapply H; eauto; cbv [states_related]; ssplit; solve [eauto]
+        | _ => progress subst
+        end; [ ].
+    eexists; ssplit; [ eauto | ].
+    cbv [insn_equiv] in *.
+    destruct_one_match; destruct_one_match_hyp; subst; try contradiction; [ | ].
+    { (* straightline case *)
+      eapply strt1_weaken; [ eassumption | ].
+      cbv beta; intros.
+      related_states_hammer. }
+    { (* ctrl1 case *)
+      eapply ctrl1_weaken; try eassumption; [ ].
+      related_states_hammer. ssplit; related_states_hammer. }
+  Qed.
+
+  Lemma link_eventually_run1 fns prog syms st1 st2 spec1 spec2 :
+      link fns = Ok prog ->
+      link_symbols fns = Ok syms ->
+      (forall st1' st2',
+          states_related syms st1' st2' ->
+          spec1 st1' ->
+          spec2 st2') ->
+      states_related syms st1 st2 ->
+      eventually (run1 (fetch:=fetch_ctx fns)) spec1 st1 ->
+      eventually (run1 (fetch:=fetch prog)) spec2 st2.
+  Proof.
+    intros. generalize dependent st2.
+    let H := lazymatch goal with H : eventually _ _ _ |- _ => H end in
+    induction H; intros; [ solve [eauto using eventually_done] | ].    
+    eapply eventually_step; [ | solve [eauto] ].
+    eapply link_run1; eauto.      
+  Qed.
+
+  Lemma link_symbols_name fns1 fns2 fn name syms :
+    link_symbols (fns1 ++ fn :: fns2) = Ok syms ->
+    name = fst (fst fn) ->
+    map.get syms name = Some (program_size 0%nat fns1).
+  Proof.
+    cbv [link_symbols]; err_simpl; intros; subst; [ | congruence ].
+    destruct_products; cbn [fst snd] in *.
+    lazymatch goal with H : inl _ = inl _ |- _ => inversion H; clear H; subst end.
+    eauto using link_symbols'_name.
+  Qed.
+
+  (* Theorem that connects run1 with a ctx to run1 with a program *)
+  Lemma link_exits' :
+    forall fns prog syms start_fn start_name n start_pc regs wregs flags dmem spec err_spec,
+      (* ...if `prog` is the result of a successful `link fns`... *)
+      link fns = Ok prog ->
+      (* ..and `syms` is the symbol table for `fns`... *)
+      link_symbols fns = Ok syms ->
+      (* ...and `start_fn` is in the list... *)
+      nth_error fns n = Some start_fn ->
+      (* ...and `start_pc` is the global offset... *)
+      start_pc = program_size 0%nat (firstn n fns) ->
+      (* ...and `start_name is the name of the starting function... *)
+      start_name = fst (fst start_fn) ->
+      (* ...and the pre-link version satisfies the spec... *)
+      exits (fetch:=fetch_ctx fns) start_name regs wregs flags dmem [] [] spec err_spec ->
+      (* ...the program satisfies the spec. *)
+      exits (fetch:=fetch prog) start_pc regs wregs flags dmem [] [] spec err_spec.
+  Proof.
+    cbv [exits]; intros.
+    assert (In start_fn fns) by (eauto using nth_error_In).
+    pose proof (link_correct _ _ _ _ ltac:(eassumption) ltac:(eassumption) ltac:(eassumption)).
+    repeat lazymatch goal with
+           | H : exists _, _ |- _ => destruct H
+           | H : _ /\ _ |- _ => destruct H
+           | H : nth_error _ _ = Some _ |- _ => apply nth_error_split in H
+           | _ => progress subst
+           end.
+    eapply link_eventually_run1; eauto; [ | ].
+    { cbv beta; intros.
+      cbv [states_related] in *.
+      related_states_hammer. }
+    { cbv beta; intros.
+      cbv [states_related]; ssplit; related_states_hammer.
+      eapply link_symbols_name; [ | reflexivity .. ].
+      rewrite List.firstn_app_l by lia.
+      eauto. }
+  Qed.
+
+  (* like `find` except returns the index of the match *)
+  Definition find_index {A} (f : A -> bool) (l : list A) : option nat :=    
+    find (fun idx =>
+            match nth_error l idx with
+            | Some a => f a
+            | None => false
+            end)
+      (seq 0 (length l)).
+
+  Definition find_global_offset (fns : list function) (name : string) : option nat :=
+    match find_index (fun fn => String.eqb name (fst (fst fn))) fns with
+    | Some idx => Some (program_size 0%nat (firstn idx fns))
+    | None => None
+    end.
+
+  Lemma find_app :
+    forall {A} (f : A -> bool) l1 l2,
+      find f (l1 ++ l2) = match find f l1 with
+                          | Some x => Some x
+                          | None => find f l2
+                          end.
+  Proof.
+    induction l1; intros; [ reflexivity | ].
+    cbn [app find]. destruct_one_match; eauto.
+  Qed.
+
+  Lemma find_map :
+    forall {A B} (f : B -> bool) (g : A -> B) l,
+      find f (List.map g l) = option_map g (find (fun a => f (g a)) l).
+  Proof.
+    cbv [option_map].
+    induction l; cbn [find List.map]; intros; [ congruence | ].
+    destruct_one_match_hyp; destruct_one_match;
+      repeat lazymatch goal with
+        | H : Some _ = Some _ |- _ => inversion H; clear H; subst
+        | _ => first [ solve [eauto] | congruence ]
+        end.
+  Qed.
+
+  Lemma find_map_inv :
+    forall {A B} (f : B -> bool) (g : A -> B) l b,
+      find f (List.map g l) = Some b ->
+      exists a,
+        find (fun a => f (g a)) l = Some a
+        /\ g a = b.
+  Proof.
+    induction l; cbn [find List.map]; intros; [ congruence | ].
+    destruct_one_match_hyp;
+      repeat lazymatch goal with
+        | H : exists _, _ |- _ => destruct H
+        | H : _ /\ _ |- _ => destruct H
+        | H : Some _ = Some _ |- _ => inversion H; clear H; subst
+        | H : find _ (List.map _ _) = Some _ |- _ => apply IHl in H
+        | _ => solve [eauto]
+        end.
+  Qed.
+
+  Lemma program_size_add :
+    forall fns start,
+      fold_left
+        (fun offset (fn : function) => (offset + length (snd fn))%nat)
+        fns start = (fold_left
+                       (fun offset (fn : function) => (offset + length (snd fn))%nat)
+                       fns 0 + start)%nat.
+  Proof.
+    induction fns; cbn [fold_left]; intros; [ lia | ].
+    rewrite !(IHfns (_ + _)%nat). lia.
+  Qed.
+
+  Lemma program_size_equiv :
+    forall fns1 fns2 fns3 fns4 a b start,
+      program_size start fns1 = program_size start fns2 ->
+      fns1 ++ a :: fns3 = fns2 ++ b :: fns4 ->
+      (0 < length (snd a))%nat ->
+      (0 < length (snd b))%nat ->
+      a = b.
+  Proof.
+    cbv [program_size].
+    induction fns1; destruct fns2; cbn [app fold_left]; intros; subst;
+      repeat lazymatch goal with
+        | H : _ :: _ = _ :: _ |- _ => inversion H; clear H; subst
+        | H : ?start = fold_left _ _ (?start + _)%nat |- _ =>
+            rewrite program_size_add in H; lia
+        | H : fold_left _ _ (?start + _)%nat = ?start |- _ =>
+            rewrite program_size_add in H; lia
+        | |- ?x = ?x => reflexivity
+        | _ => solve [eauto]
+        end.    
+  Qed.
+
+  Lemma link_symbols'_app :
+    forall fns1 fns2 start_syms start_offset end_offset syms,
+      link_symbols' start_syms start_offset (fns1 ++ fns2) = Ok (syms, end_offset) ->
+      exists syms1 end_offset1,
+        link_symbols' start_syms start_offset fns1 = Ok (syms1, end_offset1)
+        /\ link_symbols' syms1 end_offset1 fns2 = Ok (syms, end_offset).
+  Proof.
+    induction fns1; cbn [app]; intros; [ do 2 eexists; ssplit; [ reflexivity | eauto ] | ].
+    repeat lazymatch goal with
+           | H : _ /\ _ |- _ => destruct H
+           | H : exists _, _ |- _ => destruct H
+           | H : link_symbols' _ _ (_ :: _) = Ok _ |- _ =>
+               apply link_symbols'_inv in H
+           | H : link_symbols' _ _ (_ ++ _) = Ok _ |- _ =>
+               apply IHfns1 in H
+           | _ => progress subst
+           end.    
+    erewrite link_symbols'_step by eauto.
+    eauto.
+  Qed.
+
+  Lemma link_symbols'_no_dup' :
+    forall fns start_syms start_offset end_offset syms fn1 fn2 n1 n2,
+      link_symbols' start_syms start_offset fns = Ok (syms, end_offset) ->
+      nth_error fns n1 = Some fn1 ->
+      nth_error fns n2 = Some fn2 ->
+      (n1 < n2)%nat ->
+      fst (fst fn1) <> fst (fst fn2).
+  Proof.
+    intros. intro; subst.
+    repeat lazymatch goal with 
+           | H : _ /\ _ |- _ => destruct H
+           | H : exists _, _ |- _ => destruct H
+           | H : nth_error (_ ++ _) _ = _ |- _ => rewrite nth_error_app2 in H by lia
+           | H : nth_error (_ :: _) _ = Some _ |- _ =>
+               rewrite nth_error_cons in H; destruct_one_match_hyp; [ lia | ]
+           | H : nth_error _ n1 = Some _ |- _ =>
+               apply List.nth_error_split in H
+           | H : nth_error _ ?n = Some _, H' : _ = S ?n |- _ =>
+               apply List.nth_error_split in H
+           | H : link_symbols' _ _ (_ ++ _) = Ok _ |- _ =>
+               apply link_symbols'_app in H
+           | H : link_symbols' _ _ (_ :: _) = Ok _ |- _ =>
+               apply link_symbols'_inv in H
+           | _ => progress (cbn [fst snd] in *; subst)
+           end.
+    repeat lazymatch goal with
+           | H : _ /\ _ |- _ => destruct H
+           | H : exists _, _ |- _ => destruct H
+           | H : link_symbols_for_function _ fn1 = _ |- _ =>
+               apply link_symbols_for_function_name in H
+           | H : link_symbols_for_function (?syms, ?off) fn2 = _,
+               H' : map.get ?syms _ = Some _ |- _ =>
+               eapply link_symbols_for_function_name_fail with (fn:=fn2) (start_offset:=off) in H';
+               [ | solve [eauto] ]
+           | H : link_symbols' ?syms _ _ = _, H' : map.get ?syms _ = Some _ |- _ =>
+               eapply link_symbols'_no_overwrite in H; [ | solve [eauto] .. ]
+           | _ => progress (cbn [fst snd] in *; subst)
+           end.
+    congruence.
+  Qed.
+
+  Lemma link_symbols'_no_dup :
+    forall fns start_syms start_offset end_offset syms fn1 fn2,
+      link_symbols' start_syms start_offset fns = Ok (syms, end_offset) ->
+      In fn1 fns ->
+      In fn2 fns ->
+      fst (fst fn1) = fst (fst fn2) ->
+      fn1 = fn2.      
+  Proof.
     intros.
-    ssplit; [ cbv [is_valid_addi_imm]; lia | ].
-    eexists; ssplit; [ | ].
-    { cbv [read_gpr].
-      repeat progress (rewrite ?map.get_put_diff, ?map.get_put_same by congruence).
+    repeat lazymatch goal with
+           | H : _ /\ _ |- _ => destruct H
+           | H : exists _, _ |- _ => destruct H
+           | H : In _ _ |- _ => apply In_nth_error in H
+           end.
+    lazymatch goal with
+    | H1 : nth_error fns ?n1 = Some fn1,
+        H2 : nth_error fns ?n2 = Some fn2 |- _ =>
+        destr (n1 <? n2)%nat;
+        [ | destr (n2 <? n1)%nat;
+            [ | assert (n1 = n2) by lia; subst ] ]
+    end; lazymatch goal with
+         | H : (_ < _)%nat |- _ => eapply link_symbols'_no_dup' in H; eauto; congruence
+         | _ => congruence
+         end.
+  Qed.
+
+  Lemma link_symbols_no_dup :
+    forall fns syms fn1 fn2,
+      link_symbols fns = Ok syms ->
+      In fn1 fns ->
+      In fn2 fns ->
+      fst (fst fn1) = fst (fst fn2) ->
+      fn1 = fn2.      
+  Proof.
+    cbv [link_symbols].
+    intros. err_simpl. destruct_products.
+    eapply link_symbols'_no_dup; eauto.    
+  Qed.
+
+  Lemma find_ext {A} (f g : A -> bool) l (Hext : forall a, f a = g a) :
+    find f l = find g l.
+  Proof.
+    induction l; cbn [find]; intros; [ reflexivity | ].
+    rewrite Hext, IHl; reflexivity.
+  Qed.
+
+  Lemma find_index_cons {A} (f : A -> bool) l a :
+      find_index f (a :: l) = if f a then Some 0%nat else option_map S (find_index f l).
+  Proof.
+    cbv [find_index]. cbn [length].
+    rewrite <-cons_seq, <-seq_shift.
+    cbn [find nth_error]. destruct_one_match; [ reflexivity | ].    
+    rewrite find_map; reflexivity.
+  Qed.
+
+  Lemma find_index_Some :
+    forall {A} (f : A -> bool) l i,
+      find_index f l = Some i ->
+      exists a,
+        nth_error l i = Some a
+        /\ f a = true.
+  Proof.
+    induction l; intros.
+    { cbn [find_index length nth_error seq find] in *. congruence. }
+    { rewrite find_index_cons in *. cbv [option_map] in *.
+      repeat lazymatch goal with
+             | H : Some _ = Some _ |- _ => inversion H; clear H; subst
+             | H : None = Some _ |- _ => congruence
+             | H : context [match ?x with _ => _ end] |- _ => destruct_one_match_hyp
+             | _ => first [ progress (cbn [nth_error] in *; subst)
+                          | solve [eauto] ]
+             end. }    
+  Qed.
+
+  Lemma find_global_offset_correct' :
+    forall fns syms fn name offset,
+      In fn fns ->
+      link_symbols fns = Ok syms ->
+      find_global_offset fns name = Some offset ->
+      name = fst (fst fn) ->
+      exists n,
+        nth_error fns n = Some fn
+        /\ offset = program_size 0%nat (firstn n fns).
+  Proof.
+    cbv [find_global_offset]. intros.
+    repeat lazymatch goal with
+           | H : exists _, _ |- _ => destruct H
+           | H : _ /\ _ |- _ => destruct H
+           | H : Some _ = Some _ |- _ => inversion H; clear H; subst
+           | H : None = Some _ |- _ => congruence
+           | H : find_index _ _ = Some _ |- _ => apply find_index_Some in H
+           | H : String.eqb _ _ = true |- _ => apply String.eqb_eq in H
+           | H : nth_error _ _ = Some ?fn, H' : fst (fst _) = fst (fst ?fn) |- _ =>
+               eapply link_symbols_no_dup in H'; eauto using nth_error_In; subst; eauto
+           | _ => first [ progress subst | destruct_one_match_hyp ]
+           end.
+  Qed.
+
+  Lemma find_global_offset_correct :
+    forall fns syms name offset,
+      link_symbols fns = Ok syms ->
+      find_global_offset fns name = Some offset ->
+      exists fn n,
+        nth_error fns n = Some fn
+        /\ name = fst (fst fn)
+        /\ In fn fns
+        /\ offset = program_size 0%nat (firstn n fns).
+  Proof.
+    cbv [find_global_offset]. intros.
+    repeat lazymatch goal with
+           | H : exists _, _ |- _ => destruct H
+           | H : _ /\ _ |- _ => destruct H
+           | H : Some _ = Some _ |- _ => inversion H; clear H; subst
+           | H : None = Some _ |- _ => congruence
+           | H : find_index _ _ = Some _ |- _ => apply find_index_Some in H
+           | H : String.eqb _ _ = true |- _ => apply String.eqb_eq in H
+           | _ => first [ progress subst | destruct_one_match_hyp ]
+           end.
+    do 2 eexists; ssplit; eauto using nth_error_In.    
+  Qed.
+
+  (* Theorem that connects run1 with a ctx to run1 with a program *)
+  Lemma link_exits :
+    forall fns prog syms start_name start_pc regs wregs flags dmem spec err_spec,
+      (* ...if `prog` is the result of a successful `link fns`... *)
+      link fns = Ok prog ->
+      (* ..and `syms` is the symbol table for `fns`... *)
+      link_symbols fns = Ok syms ->
+      (* ...and `start_pc` is the global offset of `start_name`... *)
+      find_global_offset fns start_name = Some start_pc ->
+      (* ...and the pre-link version satisfies the spec... *)
+      exits (fetch:=fetch_ctx fns) start_name regs wregs flags dmem [] [] spec err_spec ->
+      (* ...the program satisfies the spec. *)
+      exits (fetch:=fetch prog) start_pc regs wregs flags dmem [] [] spec err_spec.
+  Proof.
+    cbv [exits]; intros.
+    lazymatch goal with H : find_global_offset _ _ = Some _ |- _ =>
+                          eapply find_global_offset_correct in H; [ | solve [eauto] ] end.
+    repeat lazymatch goal with
+           | H : exists _, _ |- _ => destruct H
+           | H : _ /\ _ |- _ => destruct H
+           | _ => progress subst
+           end.
+    pose proof (link_correct _ _ _ _ ltac:(eassumption) ltac:(eassumption) ltac:(eassumption)).
+    repeat lazymatch goal with
+           | H : exists _, _ |- _ => destruct H
+           | H : _ /\ _ |- _ => destruct H
+           end.
+    eapply link_eventually_run1; eauto; [ | ].
+    { cbv beta; intros.
+      cbv [states_related] in *.
+      related_states_hammer. }
+    { cbv beta; intros.
+      cbv [states_related]; ssplit; related_states_hammer.
+      repeat lazymatch goal with
+             | H : exists _, _ |- _ => destruct H
+             | H : _ /\ _ |- _ => destruct H
+             | H : nth_error _ _ = Some ?fn |- map.get syms (fst (fst ?fn)) = _ =>
+                 apply nth_error_split in H
+             | _ => progress subst
+             end.
+      erewrite link_symbols_name by eauto.
+      rewrite List.firstn_app_l by lia.
       reflexivity. }
-    cbv [write_gpr ret].
-    ssplit; [ cbv [is_valid_addi_imm]; lia | ].
-    eexists; ssplit; [ | ].
-    { cbv [read_gpr].
-      repeat progress (rewrite ?map.get_put_diff, ?map.get_put_same by congruence).
-      reflexivity. }
-    cbv [read_gpr].
-    repeat progress (rewrite ?map.get_put_diff, ?map.get_put_same by congruence).
-    reflexivity.
+  Qed.
+End BuildProofs.
+
+Module map.
+  Section __.
+    Context {K V : Type} {map : map.map K V} {map_ok : map.ok map}.
+    Context {key_eqb : K -> K -> bool}
+      {key_eqb_spec : forall k1 k2, BoolSpec (k1 = k2) (k1 <> k2) (key_eqb k1 k2)}.
+
+    Lemma only_differ_trans (m1 m2 m3 : map.rep (map:=map)) (s1 s2 s3 : PropSet.set K) :
+      map.only_differ m1 s1 m2 ->
+      map.only_differ m2 s2 m3 ->
+      PropSet.subset (PropSet.union s1 s2) s3 ->
+      map.only_differ m1 s3 m3.
+    Proof using Type.
+      intros. intro k.
+      repeat lazymatch goal with
+             | H : _ /\ _ |- _ => destruct H
+             | H : _ \/ _ |- _ => destruct H
+             | H : map.only_differ _ _ _ |- _ => specialize (H k)
+             | H : PropSet.elem_of _ ?s,
+                 H' : PropSet.subset (PropSet.union _ ?s) ?s'
+               |- PropSet.elem_of _ ?s' \/ _ =>
+                 left; apply H'; apply PropSet.in_union_r; assumption
+             | H : PropSet.elem_of _ ?s,
+                 H' : PropSet.subset (PropSet.union ?s _) ?s'
+               |- PropSet.elem_of _ ?s' \/ _ =>
+                 left; apply H'; apply PropSet.in_union_l; assumption
+             | H : ?a = ?b, H' : ?b = ?c |- _ \/ ?a = ?c => right; congruence
+             end.
+    Qed.
+
+    Lemma only_differ_put (m : map.rep (map:=map)) k v s :
+      PropSet.subset (PropSet.singleton_set k) s ->
+      map.only_differ m s (map.put m k v).
+    Proof using map_ok key_eqb_spec.
+      intros. cbv [map.only_differ PropSet.elem_of PropSet.subset PropSet.singleton_set] in *.
+      intro k'. destr (key_eqb k k'); [ left; solve [auto] | right ].
+      rewrite map.get_put_diff; congruence.
+    Qed.
+
+    Lemma only_differ_subset (m1 m2 : map.rep (map:=map)) s1 s2 :
+      PropSet.subset s1 s2 ->
+      map.only_differ m1 s1 m2 ->
+      map.only_differ m1 s2 m2.
+    Proof using Type.
+      clear key_eqb key_eqb_spec.
+      intros. cbv [map.only_differ PropSet.elem_of PropSet.subset] in *.
+      intro k.
+      repeat lazymatch goal with
+             | H : _ /\ _ |- _ => destruct H
+             | H : _ \/ _ |- _ => destruct H
+             | H : forall x : K, _ |- _ => specialize (H k)
+             | _ => tauto
+             end.
+    Qed.
+
+    Lemma only_differ_same (m : map.rep (map:=map)) s :
+      map.only_differ m s m.
+    Proof using Type. right; reflexivity. Qed.
+  End __.
+End map.
+
+Ltac solve_map_step t :=
+  first [ rewrite map.get_put_diff by t
+        | rewrite map.get_put_same by t                       
+        | reflexivity
+        | eassumption
+        | lazymatch goal with
+          | H : map.get ?m ?k = _ |- context [map.get ?m ?k] =>
+              rewrite H end
+        | lazymatch goal with m := _ : map.rep |- _ =>
+                                lazymatch goal with |- context [m] => subst m end end
+    ].
+Ltac solve_map := repeat (solve_map_step ltac:(congruence)).
+
+(* Helper lemmas for proving things about programs. *)
+Section Helpers.
+  Context {word32 : word.word 32} {word32_ok : word.ok word32}.
+  Context {word256 : word.word 256} {word256_ok : word.ok word256}.
+  Context {regfile : map.map reg word32} {regfile_ok : map.ok regfile}.
+  Context {wregfile : map.map wreg word256} {wregfile_ok : map.ok wregfile}.
+  Context {flagfile : map.map flag bool} {flagfile_ok : map.ok flagfile}.
+  Context {mem : map.map word32 word32} {mem_ok : map.ok mem}.
+
+  Definition gpr_has_value (regs : regfile) (r : gpr) (v : word32) : Prop :=
+    read_gpr False prop_option_bind regs r (eq v).
+
+  Lemma fetch_weaken_run1
+    {label : Type}
+    {fetch1 : label * nat -> option insn}
+    {fetch2 : label * nat -> option insn} :
+    forall st P,
+      run1 (fetch:=fetch1) st P ->
+      (forall dst i, fetch1 dst = Some i -> fetch2 dst = Some i) ->
+      run1 (fetch:=fetch2) st P.
+  Proof.
+    induction st; cbn [run1]; intros; auto; [ ].
+    repeat lazymatch goal with
+           | H : exists _, _ |- _ => destruct H
+           | H : _ /\ _ |- _ => destruct H
+           end.
+    eauto.
+  Qed.
+
+  Lemma fetch_weaken
+    {label : Type}
+    {fetch1 : label * nat -> option insn}
+    {fetch2 : label * nat -> option insn} :
+    forall st P,
+      eventually (run1 (fetch:=fetch1)) P st ->
+      (forall dst i, fetch1 dst = Some i -> fetch2 dst = Some i) ->
+      eventually (run1 (fetch:=fetch2)) P st.
+  Proof.
+    induction 1; intros; [ auto using eventually_done | ].
+    eapply eventually_step; eauto using fetch_weaken_run1.
+  Qed.
+
+  Definition function_symbols_disjoint (fn1 fn2 : function) : Prop :=
+    let name1 := fst (fst fn1) in
+    let name2 := fst (fst fn2) in
+    let syms1 := snd (fst fn1) in
+    let syms2 := snd (fst fn2) in
+    map.disjoint syms1 syms2
+    /\ map.get syms1 name2 = None
+    /\ map.get syms2 name1 = None
+    /\ name1 <> name2.    
+
+  Lemma fetch_fn_disjoint fn1 fn2 dst i :
+    fetch_fn fn1 dst = Some i ->
+    function_symbols_disjoint fn1 fn2 ->
+    fetch_fn fn2 dst = None.
+  Proof.
+    cbv [function_symbols_disjoint].
+    destruct fn1 as [[name1 syms1] insns1].
+    destruct fn2 as [[name2 syms2] insns2].
+    destruct dst as [dst offset].
+    cbv [fetch_fn get_label_offset]. cbn [fst snd].
+    repeat lazymatch goal with
+           | |- context [String.eqb ?x ?y] => destr (String.eqb x y); subst; try congruence
+           | |- context [match _ with _ => _ end] => destruct_one_match; try congruence
+           | H0 : map.disjoint ?m1 ?m2,
+               H1 : map.get ?m1 ?k = Some _,
+                 H2 : map.get ?m2 ?k = Some _ |- _ =>
+               exfalso; eapply H0; eauto
+           | H : _ /\ _ |- _ => destruct H
+           | H : ?x <> ?x |- _ => congruence
+           | H : Some _ = None |- _ => congruence
+           | _ => progress intros
+           end.
+  Qed.
+
+  Lemma fetch_ctx_singleton_iff fn dst i :
+    fetch_ctx [fn] dst = Some i <-> fetch_fn fn dst = Some i.
+  Proof.
+    cbn [fetch_ctx fold_left]. destruct_one_match; split; congruence.
+  Qed.
+
+  Lemma fetch_ctx_weaken_cons_eq fns fn dst i :
+      fetch_ctx [fn] dst = Some i ->
+      fetch_ctx (fn :: fns) dst = Some i.
+  Proof.
+    cbn [fetch_ctx fold_left]; intro Hfn.
+    rewrite Hfn. eauto using fetch_ctx_done.
+  Qed.
+
+  (* TODO: rework this lemma so it's easier -- not just fetch_fn =
+     None, but fn is disjoint from the symbol table *)
+  Lemma fetch_ctx_weaken_cons_ne fns fn dst :
+    fetch_fn fn dst = None ->
+    fetch_ctx (fn :: fns) dst = fetch_ctx fns dst.
+  Proof.
+    cbn [fetch_ctx fetch_fn fold_left]; intro Hfn.
+    rewrite Hfn. eauto.
+  Qed.
+
+  Lemma eventually_jump
+    {label : Type}
+    {fetch1 : label * nat -> option insn}
+    {fetch2 : label * nat -> option insn} :
+    forall dst pc (regs : regfile) wregs flags dmem cstack lstack spec post,
+      fetch2 pc = Some (Control (Jal x1 dst)) ->
+      (length cstack < 8)%nat ->
+      returns (fetch:=fetch1) dst regs wregs flags dmem (advance_pc pc :: cstack) lstack spec ->
+      (forall dst i, fetch1 dst = Some i -> fetch2 dst = Some i) ->
+      (forall regs wregs flags dmem,
+          spec regs wregs flags dmem ->
+          eventually (run1 (fetch:=fetch2))
+            post (otbn_busy (advance_pc pc) regs wregs flags dmem cstack lstack)) ->
+      eventually (run1 (fetch:=fetch2)) post
+        (otbn_busy pc regs wregs flags dmem cstack lstack).
+  Proof.
+    cbv [returns]; intros.
+    cbn [hd_error] in *.
+    eapply eventually_step.
+    { cbv [run1]; intros. eexists; split; [ eassumption | ].
+      cbv iota. cbn [ctrl1 call_stack_push set_pc].
+      destruct_one_match; try lia; apply eq_refl. }
+    intros; subst.
+    eapply eventually_trans;
+      [ eapply fetch_weaken; eauto | intro st; destruct st; try contradiction ].
+    intros; repeat lazymatch goal with H : _ /\ _ |- _ => destruct H end. subst.
+    cbn [tl]. eauto.
   Qed.
     
+  Lemma eventually_invariant {label : Type} {fetch : label * nat -> option insn} :
+    forall (invariant : nat -> otbn_state -> Prop) iters post st,
+      invariant iters st ->
+      (forall i st,
+          (0 <= i < iters)%nat ->
+          invariant (S i) st ->
+          eventually (run1 (fetch:=fetch)) (fun st => invariant i st \/ post st) st) ->
+      (forall st, invariant 0%nat st -> eventually (run1 (fetch:=fetch)) post st) ->
+      eventually (run1 (fetch:=fetch)) post st.
+  Proof.
+    induction iters; intros; [ solve [eauto] | ].
+    apply (eventually_trans _ (fun st => invariant iters st \/ post st));
+      repeat match goal with
+        | H : _ \/ _ |- _ => destruct H
+        | H : context [invariant] |- _ => apply H; auto; lia
+        | _ => eapply IHiters; eauto; [ ]
+        | _ => progress intros
+        | _ => eauto using eventually_done
+        end.
+  Qed.
+
+  Definition get_lstack {label : Type} (st : otbn_state)
+    : option (list (label * nat * nat)) :=
+    match st with
+    | otbn_busy _ _ _ _ _ _ lstack => Some lstack
+    | _ => None
+    end.
+
+  (* Loop invariant helper lemma. Note: `invariant i` should hold on
+     the state the loop has when it reaches the end of the loop body
+     in the `i`th iteration from last, so e.g. `invariant 0` should
+     hold at the very end of the loop. *)
+  Lemma loop_invariant
+    {label : Type} {fetch : label * nat -> option insn} :
+    forall (invariant : nat -> regfile -> wregfile -> flagfile -> mem -> Prop)
+           (end_pc : label * nat)
+           iters pc r v (regs : regfile) wregs flags dmem cstack lstack post,
+      fetch pc = Some (Control (Loop r)) ->
+      fetch end_pc = Some (Control LoopEnd) ->
+      gpr_has_value regs r v ->
+      Z.of_nat iters = word.unsigned v ->
+      (length lstack < 8)%nat ->
+      iters <> 0%nat ->
+      invariant iters regs wregs flags dmem ->
+      (* invariant step condition; if `invariant` holds at start, we reach end *)
+      (forall i regs wregs flags dmem,
+          (0 <= i <= iters)%nat ->
+          invariant (S i) regs wregs flags dmem ->
+          eventually (run1 (fetch:=fetch))
+          (fun st => (exists regs wregs flags dmem,
+                         invariant i regs wregs flags dmem
+                         /\ st = match i with
+                                 | S i => otbn_busy (advance_pc pc) regs wregs flags dmem cstack
+                                            ((advance_pc pc, i) :: lstack)
+                                 | O => otbn_busy (advance_pc end_pc)
+                                          regs wregs flags dmem cstack lstack
+                                 end)
+                     \/ post st)
+          (otbn_busy (advance_pc pc) regs wregs flags dmem cstack
+             ((advance_pc pc, i) :: lstack))) ->
+      (forall regs wregs flags dmem,
+          invariant 0%nat regs wregs flags dmem ->
+          eventually (run1 (fetch:=fetch)) post
+            (otbn_busy (advance_pc end_pc) regs wregs flags dmem cstack lstack)) ->
+      eventually (run1 (fetch:=fetch)) post (otbn_busy pc regs wregs flags dmem cstack lstack).
+  Proof.
+    cbv [loop_start]; intros.
+    repeat match goal with H : _ /\ _ |- _ => destruct H end.
+    destruct iters; [ lia | ].    
+    eapply eventually_step.
+    { cbn [run1]. eexists; ssplit; [ eassumption | ].
+      cbv iota. cbn [ctrl1 read_gpr_from_state].
+      eapply read_gpr_weaken; [ eassumption | ].
+      intros; cbv [loop_start]. ssplit; [ lia .. | ].
+      subst.
+      lazymatch goal with H : Z.of_nat _ = word.unsigned ?v |- context [word.unsigned ?v] =>
+                            rewrite <-H end.
+      rewrite Nat2Z.id.
+      destruct_one_match; try lia; eapply eq_refl. }
+    intros; subst.
+    eapply eventually_invariant
+      with (iters := S iters)
+           (invariant :=
+              fun i st =>
+                (exists regs wregs flags dmem,
+                    invariant i regs wregs flags dmem
+                    /\ st = match i with
+                            | S i => otbn_busy (advance_pc pc) regs wregs flags dmem cstack
+                                       ((advance_pc pc, i) :: lstack)
+                            | O => otbn_busy (advance_pc end_pc) regs wregs flags dmem cstack lstack
+                            end)).
+    { intros. subst. eexists; ssplit; eauto. }
+    { intros. subst.
+      repeat match goal with
+             | H : _ /\ _ |- _ => destruct H
+             | H : exists _, _ |- _ => destruct H
+             | H : Some _ = Some _ |- _ => inversion H; clear H; subst
+             | H : context [eventually run1 (fun st => _ \/ post st)] |- _ =>
+                 apply H; eauto; lia
+             | _ => progress subst
+             end. }
+    { intros. subst.
+      repeat match goal with
+             | H : _ /\ _ |- _ => destruct H
+             | H : exists _, _ |- _ => destruct H
+             | H : Some _ = Some _ |- _ => inversion H; clear H; subst
+             | _ => progress subst
+             end.
+      eauto. }
+  Qed.
+
+  Lemma eventually_beq {label : Type} {fetch : label * nat -> option insn}:
+    forall pc dst r1 r2 regs wregs flags dmem cstack lstack v1 v2 post,
+      fetch pc = Some (Control (Beq r1 r2 dst)) ->
+      gpr_has_value regs r1 v1 ->
+      gpr_has_value regs r2 v2 ->
+      (* branch case *)
+      (v1 = v2 ->
+       eventually (run1 (fetch:=fetch)) post
+         (otbn_busy (dst, 0%nat) regs wregs flags dmem cstack lstack)) ->
+      (* no-branch case *)
+      (v1 <> v2 ->
+       eventually (run1 (fetch:=fetch)) post
+         (otbn_busy (advance_pc pc) regs wregs flags dmem cstack lstack)) ->
+      eventually (run1 (fetch:=fetch)) post
+        (otbn_busy pc regs wregs flags dmem cstack lstack).
+  Proof.
+    intros.
+    destr (word.eqb v1 v2).
+    { eapply eventually_step.
+      { cbv [run1]. eexists; ssplit; [ eassumption .. | ]. cbv [ctrl1 read_gpr_from_state].
+        repeat (eapply read_gpr_weaken; [ eassumption .. | ]; intros; subst).
+        rewrite word.eqb_eq by reflexivity.
+        cbv [set_pc]. apply eq_refl. }
+      intros; subst. eauto. }
+    { eapply eventually_step.
+      { cbv [run1]. eexists; ssplit; [ eassumption .. | ]. cbv [ctrl1 read_gpr_from_state].
+        repeat (eapply read_gpr_weaken; [ eassumption .. | ]; intros; subst).
+        destruct_one_match; try congruence; [ ]. apply eq_refl. }
+      intros; subst. eauto. }
+  Qed.
+
+  Lemma eventually_bne {label : Type} {fetch : label * nat -> option insn}:
+    forall pc dst r1 r2 regs wregs flags dmem cstack lstack v1 v2 post,
+      fetch pc = Some (Control (Bne r1 r2 dst)) -> 
+      gpr_has_value regs r1 v1 ->
+      gpr_has_value regs r2 v2 ->
+      (* branch case *)
+      (v1 <> v2 ->
+       eventually (run1 (fetch:=fetch)) post
+         (otbn_busy (dst, 0%nat) regs wregs flags dmem cstack lstack)) ->
+      (* no-branch case *)
+      (v1 = v2 ->
+       eventually (run1 (fetch:=fetch)) post
+         (otbn_busy (advance_pc pc) regs wregs flags dmem cstack lstack)) ->
+      eventually (run1 (fetch:=fetch)) post
+        (otbn_busy pc regs wregs flags dmem cstack lstack).
+  Proof.
+    intros.
+    destr (word.eqb v1 v2).
+    { eapply eventually_step.
+      { cbv [run1]. eexists; ssplit; [ eassumption .. | ]. cbv [ctrl1 read_gpr_from_state].
+        repeat (eapply read_gpr_weaken; [ eassumption .. | ]; intros; subst).
+        destruct_one_match; try congruence; [ ]. apply eq_refl. }
+      intros; subst. eauto. }
+    { eapply eventually_step.
+      { cbv [run1]. eexists; ssplit; [ eassumption .. | ]. cbv [ctrl1 read_gpr_from_state].
+        repeat (eapply read_gpr_weaken; [ eassumption .. | ]; intros; subst).
+        destruct_one_match; try congruence; [ ]. apply eq_refl. }
+      intros; subst. eauto. }
+  Qed.
+
+  Lemma eventually_loop_end {label : Type} {fetch : label * nat -> option insn}:
+    forall pc regs wregs flags dmem cstack lstack loop_start iters post,
+      fetch pc = Some (Control LoopEnd) ->
+      (match iters with
+       | O => eventually (run1 (fetch:=fetch)) post
+                (otbn_busy (advance_pc pc) regs wregs flags dmem cstack lstack)
+       | S iters => eventually (run1 (fetch:=fetch)) post
+                      (otbn_busy loop_start regs wregs flags dmem cstack
+                         ((loop_start, iters) :: lstack))
+       end) ->
+      eventually (run1 (fetch:=fetch)) post
+        (otbn_busy pc regs wregs flags dmem cstack ((loop_start, iters) :: lstack)).
+  Proof.
+    intros. destruct iters.
+    { eapply eventually_step.
+      { cbv [run1]. eexists; ssplit; [ eassumption .. | ]. cbn [loop_end hd_error tl ctrl1].
+        do 2 eexists; ssplit; [ reflexivity .. | ].
+        cbv iota. apply eq_refl. }
+      intros; subst. eassumption. }
+    { eapply eventually_step.
+      { cbv [run1]. eexists; ssplit; [ eassumption .. | ]. cbn [loop_end hd_error tl ctrl1].
+        do 2 eexists; ssplit; [ reflexivity .. | ].
+        cbv iota. apply eq_refl. }
+      intros; subst. eassumption. }
+  Qed.
+
+  Lemma eventually_ret {label : Type} {fetch : label * nat -> option insn}:
+    forall pc regs wregs flags dmem cstack lstack ret_pc post,
+      fetch pc = Some (Control Ret) ->
+      hd_error cstack = Some ret_pc ->
+      post (otbn_busy ret_pc regs wregs flags dmem (tl cstack) lstack) ->
+      eventually (run1 (fetch:=fetch)) post
+        (otbn_busy pc regs wregs flags dmem cstack lstack).
+  Proof.
+    intros. eapply eventually_step.
+    { cbv [run1]. eexists; ssplit; [ eassumption .. | ].
+      cbn [ctrl1 call_stack_pop]. eexists; ssplit; [ eassumption .. | ].
+      apply eq_refl. }
+    intros; subst. eauto using eventually_done.
+  Qed.
+
+  Lemma eventually_ecall {label : Type} {fetch : label * nat -> option insn}:
+    forall pc regs wregs flags dmem cstack lstack post,
+      fetch pc = Some (Control Ecall) ->
+      post (otbn_done pc dmem) ->
+      eventually (run1 (fetch:=fetch)) post
+        (otbn_busy pc regs wregs flags dmem cstack lstack).
+  Proof.
+    intros. eapply eventually_step.
+    { cbv [run1]. eexists; ssplit; [ eassumption .. | ].
+      cbn [ctrl1 program_exit]. eassumption. }
+    intros; subst. eauto using eventually_done.
+  Qed.
+
+  (* TODO: maybe strt1 should return a function args -> result? need
+     more detail here, need to express new map *)
+  Lemma eventually_straightline
+    {label : Type} {fetch : label * nat -> option insn}:
+    forall pc regs wregs flags dmem cstack lstack i post,
+      fetch pc = Some (Straightline i) ->
+      strt1 False prop_random prop_urandom prop_option_bind regs wregs flags dmem i
+        (fun regs wregs flags dmem =>
+           eventually (run1 (fetch:=fetch)) post
+             (otbn_busy (advance_pc pc) regs wregs flags dmem cstack lstack)) ->
+      eventually (run1 (fetch:=fetch)) post (otbn_busy pc regs wregs flags dmem cstack lstack).
+  Proof.
+    intros. eapply eventually_step.
+    { cbv [run1]. eexists; ssplit; [ eassumption .. | ].
+      cbv iota. cbv [update_state set_pc]. eassumption. }
+    intros; subst. eauto.
+  Qed.
+
+  Definition clobbers (l : list reg) (regs regs' : regfile) : Prop :=
+    map.only_differ regs (PropSet.of_list l) regs'.
+
+  Lemma clobbers_step_in l k v r1 r2 :
+    clobbers l r1 r2 ->
+    In k l ->
+    clobbers l r1 (map.put r2 k v).
+  Proof.
+    cbv [clobbers PropSet.of_list]; intros.
+    intro k'; cbv [map.only_differ PropSet.elem_of] in *.
+    lazymatch goal with H : forall k : reg, _ |- _ => specialize (H k') end.
+    destr (reg_eqb k k'); rewrite ?map.get_put_diff, ?map.get_put_same by congruence.
+    all:tauto.
+  Qed.
+
+  Lemma clobbers_step l k v r1 r2 :
+    clobbers l r1 r2 ->
+    clobbers (k :: l) r1 (map.put r2 k v).
+  Proof.
+    cbv [clobbers PropSet.of_list]; intros.
+    intro k'; cbv [map.only_differ PropSet.elem_of] in *. cbn [In].
+    lazymatch goal with H : forall k : reg, _ |- _ => specialize (H k') end.
+    destr (reg_eqb k k'); rewrite ?map.get_put_diff, ?map.get_put_same by congruence.
+    all:tauto.
+  Qed.
+
+  Lemma clobbers_not_in l (r1 r2 : regfile) x v :
+    clobbers l r1 r2 ->
+    map.get r1 x = Some v ->
+    ~ (In x l) ->
+    map.get r2 x = Some v.
+  Proof.
+    cbv [clobbers map.only_differ PropSet.of_list PropSet.elem_of]; intros.
+    lazymatch goal with H : forall x : reg, _ \/ _ |- _ =>
+                          destruct (H ltac:(eassumption)) end.
+    all:try tauto; congruence.
+  Qed.
+
+  Lemma clobbers_trans :
+    forall l1 l2 (r1 r2 r3 : regfile),
+      clobbers l1 r1 r2 ->
+      clobbers l2 r2 r3 ->
+      clobbers (l1 ++ l2) r1 r3.
+  Proof.
+    cbv [clobbers]; intros.
+    eapply map.only_differ_trans; eauto; [ ].
+    rewrite PropSet.of_list_app_eq. reflexivity.
+  Qed.
+
+  Lemma clobbers_trans_dedup l1 l2 l3 (r1 r2 r3 : regfile) :
+      clobbers l1 r1 r2 ->
+      clobbers l2 r2 r3 ->
+      l3 = List.dedup reg_eqb (l1 ++ l2) ->
+      clobbers l3 r1 r3.
+  Proof.
+    intros; subst.
+    eapply map.only_differ_subset;
+      [ | eapply map.only_differ_trans; eauto; reflexivity ].
+    cbv [PropSet.of_list PropSet.subset PropSet.union PropSet.elem_of].
+    intros. rewrite <-List.dedup_preserves_In.
+    auto using in_or_app.
+  Qed.
+
+  Lemma clobbers_incl l1 l2 (r1 r2 : regfile) :
+    clobbers l1 r1 r2 ->
+    incl l1 l2 ->
+    clobbers l2 r1 r2.
+  Proof.
+    cbv [incl clobbers map.only_differ PropSet.elem_of PropSet.of_list].
+    intros; subst. repeat lazymatch goal with H : forall x : reg, _ |- _ =>
+                                                specialize (H ltac:(eassumption)) end.
+    intuition idtac.
+  Qed.
+
+  Lemma is_valid_addr_0 : is_valid_addr (word.of_Z 0) = true.
+  Proof.
+    cbv [is_valid_addr]. apply Bool.andb_true_iff. ssplit.
+    { apply word.eqb_eq, word.unsigned_inj.
+      rewrite word.unsigned_and, !word.unsigned_of_Z_nowrap by lia.
+      cbv [Z.land word.wrap]. rewrite Z.mod_small; lia. }
+    { cbv [DMEM_BYTES].
+      rewrite word.unsigned_ltu, !word.unsigned_of_Z_nowrap by lia.
+      lia. }
+  Qed.
+
+  Lemma is_valid_addr_add addr offset :
+    is_valid_addr addr = true ->
+    offset mod 4 = 0 ->
+    0 <= offset ->
+    0 <= word.unsigned addr + offset < DMEM_BYTES ->
+    is_valid_addr (word.add addr (word.of_Z offset)) = true.
+  Proof.
+    cbv [is_valid_addr DMEM_BYTES]. rewrite !Bool.andb_true_iff. intros.
+    repeat lazymatch goal with
+           | H : _ /\ _ |- _ => destruct H
+           | H : word.eqb ?x ?y = true |- _ =>
+               rewrite word.unsigned_eqb in H
+           | H : (_ =? _)%Z = true |- _ => apply Z.eqb_eq in H
+           | H : word.ltu ?x ?y = true |- _ =>
+               destruct (word.ltu_spec x y); [ | congruence ]; clear H;
+               rewrite ?word.unsigned_of_Z_nowrap in * by lia
+           end.
+    pose proof (word.unsigned_range addr).
+    ssplit.
+    { apply word.eqb_eq, word.unsigned_inj.
+      rewrite word.unsigned_and, word.unsigned_add, !word.unsigned_of_Z_nowrap in * by lia.
+      cbv [word.wrap] in *. rewrite (Z.mod_small (_ + _)) by lia.
+      rewrite !(Z.land_ones _ 2) in * by lia. change (2 ^ 2) with 4 in *.
+      repeat lazymatch goal with
+             | H : context [(?x mod 4) mod _] |- _ =>
+                 rewrite (Z.mod_small (x mod 4) _) in H;
+                 [ | pose proof (Z.mod_pos_bound x 4 ltac:(lia)); lia ]
+             | |- context [(?x mod 4) mod _] =>
+                 rewrite (Z.mod_small (x mod 4) _);
+                 [ | pose proof (Z.mod_pos_bound x 4 ltac:(lia)); lia ]
+             end.
+      rewrite Z.add_mod by lia.
+      repeat lazymatch goal with
+             | H : ?x = 0 |- context[?x] => rewrite H
+             | H : 0 = ?x |- context[?x] => rewrite <-H
+             end.
+      rewrite Z.mod_0_l by lia.
+      reflexivity. }
+    { rewrite word.unsigned_ltu, word.unsigned_add, !word.unsigned_of_Z_nowrap by lia.
+      apply Z.ltb_lt.
+      cbv [word.wrap]. rewrite Z.mod_small by lia.
+      lia. }
+  Qed.
+
+  Definition start_state : otbn_state :=
+    otbn_busy (0%nat, 0%nat) map.empty map.empty map.empty map.empty [] [].
+End Helpers.
+
+Ltac zsimplify_step :=
+  lazymatch goal with
+  | |- context [_ + 0] => rewrite Z.add_0_r
+  | |- context [0 + _] => rewrite Z.add_0_l
+  | |- context [_ - 0] => rewrite Z.sub_0_r
+  | |- context [?x - ?x] => rewrite Z.sub_diag
+  | |- context [_ * 0] => rewrite Z.mul_0_r
+  | |- context [0 * _] => rewrite Z.mul_0_l
+  | |- context [_ * 1] => rewrite Z.mul_1_r
+  | |- context [1 * _] => rewrite Z.mul_1_l
+  | |- context [0 mod _] => rewrite Z.mod_0_l by lia
+  | |- context [Z.of_nat (Z.to_nat _)] => rewrite Z2Nat.id by lia
+  | |- context [Z.to_nat (Z.of_nat _)] => rewrite Nat2Z.id by lia
+  | |- context [Z.of_nat 0] => change (Z.of_nat 0) with 0
+  | |- context [Z.of_nat 1] => change (Z.of_nat 1) with 1
+  | _ => progress Z.push_pull_mod
+  end.
+Ltac zsimplify := repeat zsimplify_step.
+
+Ltac solve_is_valid_addr :=
+  lazymatch goal with
+  | H : is_valid_addr ?a = true |- is_valid_addr ?a = true => exact H
+  | |- is_valid_addr (word.of_Z 0) = true => apply is_valid_addr_0
+  | |- is_valid_addr (word.add ?a (word.of_Z ?offset)) = true =>
+      assert (is_valid_addr a = true) by solve_is_valid_addr; apply is_valid_addr_add;
+      eauto; cbv[DMEM_BYTES] in *; rewrite ?word.unsigned_of_Z_nowrap by lia; lia
+  end.
   
-    | Bn_mulqacc_wo z d x y s =>
-        let st := if z then write_wsr st ACC 0 else st in
-        (_ <- assertion (valid_mul_shift s) "Invalid shift for bn.mulqacc.wo" ;
-         x <- read_limb st x ;
-         y <- read_limb st y ;
-         acc <- read_wsr st ACC ;
-         let r := mulqacc_spec acc x y s in
-         Ok (write_wdr (write_wsr st ACC r) d r))
-    | Bn_mulqacc_so z L d x y s =>
-        let st := if z then write_wsr st ACC 0 else st in
-        (_ <- assertion (valid_mul_shift s) "Invalid shift for bn.mulqacc.so" ;
-         x <- read_limb st x ;
-         y <- read_limb st y ;
-         old <- read_wdr st d ;
-         acc <- read_wsr st ACC ;
-         let r := mulqacc_spec acc x y s in
-         let accL := r &' (Z.ones 128) in
-         let accH := r >> 128 in
-         let dL := old &' (Z.ones 128) in
-         let dH := old >> 128 in
-         let d' := if L
-                   then (accL |' (dH << 128))
-                   else (dL |' (accL << 128)) in
-         Ok (write_wdr (write_wsr st ACC r) d d'))
-    | Bn_addm d x y =>
-         (x <- read_wdr st x ;
-          y <- read_wdr st y ;
-          m <- read_wsr st MOD ;          
-          Ok (write_wdr st d (addm_spec x y m)))
-    | Bn_subm d x y =>
-         (x <- read_wdr st x ;
-          y <- read_wdr st y ;
-          m <- read_wsr st MOD ;
-          Ok (write_wdr st d (subm_spec x y m)))
-    | Bn_add d x y s fg =>
-        (_ <- assertion (valid_arith_shift s) "Invalid shift for bn.add" ;
-         x <- read_wdr st x ;
-         y <- read_wdr st y ;
-         let r := x + y in
-         let st := set_mlz st fg r in
-         let st := flagfile_set st (flagC fg) (2^256 <=? r) in
-         Ok (write_wdr st d r))
-    | Bn_addc d x y s fg =>
-        (_ <- assertion (valid_arith_shift s) "Invalid shift for bn.addc" ;
-         c <- read_flag st (flagC fg);
-         x <- read_wdr st x ;
-         y <- read_wdr st y ;
-         let r := x + y + c in
-         let st := set_mlz st fg r in
-         let st := flagfile_set st (flagC fg) (2^256 <=? r) in
-         Ok (write_wdr st d r))
-    | Bn_sub d x y s fg =>
-        (_ <- assertion (valid_arith_shift s) "Invalid shift for bn.sub" ;
-         x <- read_wdr st x ;
-         y <- read_wdr st y ;
-         let r := x - y in
-         let st := set_mlz st fg r in
-         let st := flagfile_set st (flagC fg) (r <? 0) in
-         Ok (write_wdr st d r))
-    | Bn_subb d x y s fg =>
-        (_ <- assertion (valid_arith_shift s) "Invalid shift for bn.subb" ;
-         b <- read_flag st (flagC fg);
-         x <- read_wdr st x ;
-         y <- read_wdr st y ;
-         let r := x - y - b in
-         let st := set_mlz st fg r in
-         let st := flagfile_set st (flagC fg) (r <? 0) in
-         Ok (write_wdr st d r))
-    | Bn_rshi d x y imm =>
-        (_ <- assertion (valid_rshi_imm imm) "Invalid immediate for bn.rshi" ;
-         x <- read_wdr st x ;
-         y <- read_wdr st y ;
-         let r := rshi_spec x y imm in
-         Ok (write_wdr st d r))
-    | Bn_movr x y =>
-        let xinc := has_inc x in
-        let yinc := has_inc y in
-        let xr := ind_to_gpr x in
-        let yr := ind_to_gpr y in
-        (_ <- assertion (negb(xinc && yinc)) "Cannot increment both indirect registers (bn.movr)";
-         src_ptr <- read_gpr st yr ;
-         src <- index_to_wdr (src_ptr &' 32) ;
-         addr_ptr <- read_gpr st xr ;
-         addr <- index_to_wdr (addr_ptr &' 32) ;
-         v <- read_wdr st src ;
-         st <- (if xinc
-                then write_gpr st xr (src_ptr + 1)
-                else if yinc
-                     then write_gpr st yr (addr_ptr + 1)
-                     else Ok st) ;
-         Ok (write_wdr st addr v))
-    | Bn_lid x offset y =>
-        let xinc := has_inc x in
-        let yinc := has_inc y in
-        let xr := ind_to_gpr x in
-        let yr := ind_to_gpr y in
-        (_ <- assertion (negb(xinc && yinc)) "Cannot increment both indirect registers (bn.lid)";
-         _ <- assertion (valid_mem_offset offset) "Invalid offset for bn.lid";
-         src_ptr <- read_gpr st yr ;
-         src <- index_to_wdr (src_ptr &' 32) ;
-         addr_ptr <- read_gpr st xr ;
-         addr <- index_to_wdr (addr_ptr &' 32) ;
-         v <- read_wdr st src ;
-         st <- (if xinc
-                then write_gpr st xr (src_ptr + 1)
-                else if yinc
-                     then write_gpr st yr (addr_ptr + 1)
-                     else Ok st) ;
-         Ok (write_wdr st addr v))
 
-  Inductive OtbnState : Type :=
-  | OtbnBusy :
-    forall (regs : regfile) (flags : flagfile) (dmem : mem)
-           (callstack : list addr) (loopstack : list (addr * addr * nat)),
-      OtbnState
-  | OtbnErr : forall (err_code : Z) (msg : string), OtbnState
-  | OtbnDone : forall (dmem : mem), OtbnState
-  | OtbnReturn :
-    forall (regs : regfile) (flags : flagfile) (dmem : mem),
-      OtbnState
-  .
+Ltac simplify_side_condition_step :=
+  match goal with
+  | |- exists _, _ => eexists
+  | |- _ /\ _ => split
+  | |- context [if is_valid_addi_imm ?v then _ else _] =>
+        replace (is_valid_addi_imm v) with true by (cbv [is_valid_addi_imm]; lia)
+  | |- context [if is_valid_mem_offset ?v then _ else _] =>
+        replace (is_valid_mem_offset v) with true by (cbv [is_valid_mem_offset]; lia)
+  | |- context [if is_valid_addr ?a then _ else _] =>
+        replace (is_valid_addr a) with true by (symmetry; solve_is_valid_addr)
+  | |- context [(_ + 0)%nat] => rewrite Nat.add_0_r
+  | |- context [fetch_fn (?s, _, _) (?s, _)] => rewrite fetch_fn_name by auto
+  | |- match fetch_fn ?fn ?pc with _ => _ end = Some _ => reflexivity
+  | |- context [fetch_fn _ _] =>
+      erewrite fetch_fn_sym by
+      (cbn [fst snd]; first [ congruence | solve_map ])
+  | |- map.get _ _ = Some _ => solve_map
+  | H : map.get ?m ?k = Some _ |- context [match map.get ?m ?k with _ => _ end] =>
+      rewrite H
+  | |- context [match map.get _ _ with _ => _ end] => solve_map
+  | |- context [advance_pc (?dst, ?off)] =>
+      change (advance_pc (dst, off)) with (dst, S off)
+  | |- (_ < _) => lia
+  | |- (_ <= _) => lia                                   
+  | |- (_ < _)%nat => lia
+  | |- (_ <= _)%nat => lia
+  | |- Some _ = Some _ => reflexivity
+  | _ => first [ progress
+                   cbn [run1 strt1 read_gpr write_gpr ctrl1
+                          read_gpr_from_state read_mem
+                          set_pc update_state call_stack_pop call_stack_push
+                          length hd_error tl skipn nth_error fold_left
+                          fetch fetch_ctx Nat.add fst snd
+                          repeat_advance_pc advance_pc]
+               | progress cbv [prop_random prop_option_bind
+                                 gpr_has_value write_mem]
+               | eassumption ]
+  end.
+Ltac simplify_side_condition := repeat simplify_side_condition_step.
 
-  Definition exec (st : OtbnState) (P : OtbnState -> Prop) : Prop :=
-    exec_cps st (fun x =>
-                   match x with
-                   | Err _ => False
-                   | Ok x => P x
-                   end).
-
-  (* State information for the processor. *)
-  Record OtbnState : Type :=
-    {
-      (* Register file. *)
-      regs : regfile;
-      (* Flag states. *)
-      flags : flagfile;
-      (* Data memory *)
-      dmem : mem;
-      (* Call stack: holds the IMEM address of the last calls. *)
-      callstack : list addr;
-      (* Loop stack: holds the IMEM start/end addresses and counter for active loops. *)
-      loopstack : list (addr * addr * nat);
-      (* Instruction counter. *)
-      insn_counter : nat;
-      (* Program counter. *)
-      pc : addr;
-      (* Errors. *)
-      errs : 
-    }.
-
-  (* Called when OTBN encounters an error or ecall. *)
-  Definition wipe (st : OtbnState) : OtbnState :=
-    {| regs := map.empty;
-      flags := map.empty;
-      dmem := st.(dmem);
-      callstack := [];
-      loopstack := [];
-      insn_counter := st.(insn_counter);
-      pc := st.(pc);
-    |}.
-
-  Definition reg_get (st : OtbnState) (r : reg) : Z :=
-    match map.get st.(regs) r with
-    | Some v => v
-    | None => error_Z
+(* Run the linker to compute the fully linked version of a program *)
+Ltac link_program fns :=
+  let val := eval vm_compute in (link fns) in
+    lazymatch val with
+    | inl ?x => exact x
+    | inr ?e => fail e
     end.
 
-  Definition read_gpr (st : OtbnState) (r : gpr) : Z :=
-    match r with
-    | x0 => 0 (* x0 always reads as 0 *)
-    | x1 =>
-        (* TODO: call stack reads are rare in practice; for now, don't model *)
-        error_Z
-    | _ => reg_get st (gpreg r)
-    end.
-
-  Definition read_wdr (st : OtbnState) (r : wdr) : Z := reg_get st (wdreg r).
-
-  Definition read_wsr (st : OtbnState) (r : wsr) : Z :=
-    match r with
-    | RND => rnd st.(insn_counter)
-    | URND => urnd st.(insn_counter)
-    | _ => reg_get st (wsreg r)
-    end.
-
-  Definition read_flag (st : OtbnState) (f : flag) : bool :=
-    match map.get st.(flags) f with
-    | Some v => v
-    | None => error_bool
-    end.
-
-  (* Assemble a group of flags into an integer value. *)
-  Definition read_flag_group (st : OtbnState) (fg : flag_group) : Z :=
-    let c := read_flag st (flagC fg) in
-    let m := read_flag st (flagM fg) in
-    let l := read_flag st (flagL fg) in
-    let z := read_flag st (flagZ fg) in
-    c |' (m << 1) |' (l << 2) |' (z << 3).
-
-  Definition read_csr (st : OtbnState) (r : csr) : Z :=
-    match r with
-    | CSR_FG0 => read_flag_group st FG0
-    | CSR_FG1 => read_flag_group st FG1
-    | CSR_FLAGS =>
-        let fg0 := read_flag_group st FG0 in
-        let fg1 := read_flag_group st FG1 in
-        fg0 |' (fg1 << 4)
-    end.
-
-  (* Implements a read from the register file, handling all special registers. *)
-  Definition read_reg (st : OtbnState) (r : reg) : Z :=
-    match r with
-    | gpreg r => read_gpr st r
-    | wdreg r => read_wdr st r
-    | csreg r => read_csr st r
-    | wsreg r => read_wsr st r
-    end.
-
-  Definition read_limb (st : OtbnState) (l : limb) : Z :=
-    match l with
-    | limb0 r => (read_wdr st r) &' Z.ones 64
-    | limb1 r => ((read_wdr st r) >> 64) &' Z.ones 64
-    | limb2 r => ((read_wdr st r) >> 128) &' Z.ones 64
-    | limb3 r => ((read_wdr st r) >> 192) &' Z.ones 64
+Ltac get_next_insn :=
+  lazymatch goal with
+  | |- eventually (run1 (fetch:=?fetch)) _ (otbn_busy ?pc _ _ _ _ _ _) =>
+      let i := eval vm_compute in (fetch pc) in
+        i
   end.
 
-  Definition inc_insn_counter (st : OtbnState) : OtbnState :=
-    {| regs := st.(regs);
-      flags := st.(flags);
-      dmem := st.(dmem);
-      callstack := st.(callstack);
-      loopstack := st.(loopstack);
-      insn_counter := st.(insn_counter) + 1;
-      pc := st.(pc);
-    |}.
+(* Debugging tactic, prints the next instruction to be fetched. *)
+Ltac print_next_insn :=
+  let i := ltac:(get_next_insn) in
+  idtac i.
 
-  Definition regfile_set (st : OtbnState) (r : reg) (v : Z) : OtbnState :=
-    {| regs := map.put st.(regs) r v;
-      flags := st.(flags);
-      dmem := st.(dmem);
-      callstack := st.(callstack);
-      loopstack := st.(loopstack);
-      insn_counter := st.(insn_counter);
-      pc := st.(pc);
-    |}.
-
-  Definition flagfile_set (st : OtbnState) (f : flag) (v : bool) : OtbnState :=
-    {| regs := st.(regs);
-      flags := map.put st.(flags) f v;
-      dmem := st.(dmem);
-      callstack := st.(callstack);
-      loopstack := st.(loopstack);
-      insn_counter := st.(insn_counter);
-      pc := st.(pc);
-    |}.
-  
-  Definition jump (st : OtbnState) (pc : addr) : OtbnState :=
-    {| regs := st.(regs);
-      flags := st.(flags);
-      dmem := st.(dmem);
-      callstack := st.(callstack);
-      loopstack := st.(loopstack);
-      insn_counter := st.(insn_counter);
-      pc := pc;
-    |}.
-  
-  Definition callstack_pop (st : OtbnState) : OtbnState :=
-    (pc <- map_err (hd_error st.(callstack)) "Call stack empty" ;
-     Ok ({| regs := st.(regs);
-           flags := st.(flags);
-           dmem := st.(dmem);
-           callstack := tl st.(callstack);
-           loopstack := st.(loopstack);
-           insn_counter := st.(insn_counter);
-           pc := pc;
-         |})).
-
-  Definition callstack_push (st : OtbnState) (new_pc : addr) : maybe OtbnState :=
-    (_ <- assertion (length st.(callstack) <? 8)%nat "Call stack full" ;
-     Ok {| regs := st.(regs);
-          flags := st.(flags);
-          dmem := st.(dmem);
-          callstack := new_pc :: st.(callstack);
-          loopstack := st.(loopstack);
-          insn_counter := st.(insn_counter);
-          pc := st.(pc);
-        |}).
-
-  Definition loopstack_pop (st : OtbnState) : maybe ((addr * addr * nat) * OtbnState) :=
-    (l <- map_err (hd_error st.(loopstack)) "Loop stack empty" ;
-     Ok (l,
-         {| regs := st.(regs);
-           flags := st.(flags);
-           dmem := st.(dmem);
-           callstack := st.(callstack);
-           loopstack := tl st.(loopstack);
-           insn_counter := st.(insn_counter);
-          pc := st.(pc);
-         |})).
-
-  Definition loopstack_push (st : OtbnState) (l : addr * addr * nat) : maybe OtbnState :=
-    (_ <- assertion (length st.(loopstack) <? 8)%nat "Call stack full" ;
-     Ok {| regs := st.(regs);
-          flags := st.(flags);
-          dmem := st.(dmem);
-          callstack := st.(callstack);
-          loopstack := l :: st.(loopstack);
-          insn_counter := st.(insn_counter);
-          pc := st.(pc);
-        |}).
-
-  Fixpoint repeat_advance_pc (pc : addr) (n : nat) : addr :=
-    match n with
-    | O => pc
-    | S n => advance_pc (repeat_advance_pc pc n)
-    end.
-
-
-  (* set the M, L, and Z flags according to the destination register *)
-  Definition set_mlz (st : OtbnState) (fg : flag_group) (v : Z) : OtbnState :=
-    let st := flagfile_set st (flagM fg) (Z.testbit v 255) in
-    let st := flagfile_set st (flagL fg) (Z.testbit v 0) in
-    let st := flagfile_set st (flagZ fg) (v =? 0) in
-    st.
-
-  Definition cast32 (v : Z) : Z := v &' Z.ones 32.
-  Definition cast256 (v : Z) : Z := v &' Z.ones 256.
-
-  Definition write_gpr (st : OtbnState) (r : gpr) (v : Z) : maybe OtbnState :=
-    match r with
-    | x0 => Ok st
-    | x1 =>
-        (* TODO: this should push to the call stack, but is
-           practically never used. For now, don't model this behavior
-           and treat it as an error. *)
-        Err "Attempt to write to call stack. This behavior is not yet modelled."
-    | _ => Ok (regfile_set st (gpreg r) (cast32 v))
-    end.
-
-  Definition write_wdr (st : OtbnState) (r : wdr) (v : Z) : OtbnState :=
-    regfile_set st (wdreg r) (cast256 v).
-  Definition write_wsr (st : OtbnState) (r : wsr) (v : Z) : OtbnState :=
-    match r with
-    | RND => st (* writes to RND are ignored *)
-    | URND => st (* writes to URND are ignored *)
-    | _ => regfile_set st (wsreg r) (cast256 v)
-    end.
-
-  (* mulqacc shifts must be multiples of 64 *)
-  Definition valid_mul_shift (s : Z) : bool :=
-    ((s =? 0) || (s =? 64) || (s =? 128) || (s =? 192)).
-  (* rshi shifts must be in the range [0,255] *)
-  Definition valid_rshi_imm (s : Z) : bool :=
-    (0 <=? s) && (s <? 256).
-  (* other shift immediates must be multiples of 8 and in the range [0,248] *)
-  Definition valid_arith_shift (s : shift) : bool :=
-    let s := match s with
-             | lshift x => x
-             | rshift x => x
-             end in
-    ((s mod 8 =? 0) && (0 <=? s) && (s <=? 248)).
-  (* immediates for addi must be in the range [-2048, 2047] *)
-  Definition valid_addi_imm (imm : Z) : bool :=
-    (-2048 <=? imm) && (imm <=? 2047).
-  (* offsets for loads and stores are in the range [-16384, 16352] in steps of 32 *)
-  Definition valid_mem_offset (offset : Z) : bool :=
-    (-16384 <=? offset) && (offset <=? 16352) && (offset mod 32 =? 0).
-
-  (* returns whether the indirect register should be incremented *)
-  Definition has_inc (x : ind) : bool :=
-    match x with
-    | ind_noinc r => false
-    | ind_inc r => true
-    end.
-  (* gets the gpr corresponding to this indirect value *)
-  Definition ind_to_gpr (x : ind) : gpr :=
-    match x with
-    | ind_noinc r => r
-    | ind_inc r => r
-    end.
-  (* get a wdr by its index value *)
-  Definition index_to_wdr (idx : Z) : maybe wdr :=
-    match idx with
-    | 0 => Ok w0
-    | 1 => Ok w1
-    | 2 => Ok w2
-    | 3 => Ok w3
-    | 4 => Ok w4
-    | 5 => Ok w5
-    | 6 => Ok w6
-    | 7 => Ok w7
-    | 8 => Ok w8
-    | 9 => Ok w9
-    | 10 => Ok w10
-    | 11 => Ok w11
-    | 12 => Ok w12
-    | 13 => Ok w13
-    | 14 => Ok w14
-    | 15 => Ok w15
-    | 16 => Ok w16
-    | 17 => Ok w17
-    | 18 => Ok w18
-    | 19 => Ok w19
-    | 20 => Ok w20
-    | 21 => Ok w21
-    | 22 => Ok w22
-    | 23 => Ok w23
-    | 24 => Ok w24
-    | 25 => Ok w25
-    | 26 => Ok w26
-    | 27 => Ok w27
-    | 28 => Ok w28
-    | 29 => Ok w29
-    | 30 => Ok w30
-    | 31 => Ok w31
-    | _ => Err "Invalid WDR index"
-    end.
-  (* gets the value from the wdr corresponding to this indirect value *)
-  Definition read_ind (st : OtbnState) (x : ind) : maybe Z :=
-    let r := ind_to_gpr x in
-    ptr <- read_gpr st r ;
-    w <- index_to_wdr (ptr &' 32) ;
-    read_wdr st w.
-
-  (* specifications for complex operations (may make proofs a little nicer) *)
-  Definition mulqacc_spec (acc x y s : Z) : Z :=
-    acc + (x * y) << s.
-  Definition addm_spec (x y m : Z) : Z :=
-    let r := x + y in
-    if r >? m then r - m else r.
-  Definition subm_spec (x y m : Z) : Z :=
-    let r := x - y in
-    if r <? 0 then r + m else r.
-  Definition rshi_spec (x y imm : Z) : Z :=
-    let xy := Z.lor (x << 256) y in
-    xy >> imm.
-
-  Definition exec1
-    (st : OtbnState) (i : sinsn) : maybe OtbnState :=
-    let st := inc_insn_counter st in
+(* Finds the PC that matches the end of the loop. *)
+Ltac find_loop_end' fetch pc :=
+  let i := eval vm_compute in (fetch pc) in
     match i with
-    | Addi d x imm =>
-        (_ <- assertion (valid_addi_imm imm) "Invalid immediate for addi";
-         x <- read_gpr st x ;
-         write_gpr st d (x + imm))
-    | Bn_mulqacc z x y s =>
-        let st := if z then write_wsr st ACC 0 else st in
-        (_ <- assertion (valid_mul_shift s) "Invalid shift for bn.mulqacc";
-         x <- read_limb st x ;
-         y <- read_limb st y ;
-         acc <- read_wsr st ACC ;
-         let r := mulqacc_spec acc x y s in
-         Ok (write_wsr st ACC r))
-    | Bn_mulqacc_wo z d x y s =>
-        let st := if z then write_wsr st ACC 0 else st in
-        (_ <- assertion (valid_mul_shift s) "Invalid shift for bn.mulqacc.wo" ;
-         x <- read_limb st x ;
-         y <- read_limb st y ;
-         acc <- read_wsr st ACC ;
-         let r := mulqacc_spec acc x y s in
-         Ok (write_wdr (write_wsr st ACC r) d r))
-    | Bn_mulqacc_so z L d x y s =>
-        let st := if z then write_wsr st ACC 0 else st in
-        (_ <- assertion (valid_mul_shift s) "Invalid shift for bn.mulqacc.so" ;
-         x <- read_limb st x ;
-         y <- read_limb st y ;
-         old <- read_wdr st d ;
-         acc <- read_wsr st ACC ;
-         let r := mulqacc_spec acc x y s in
-         let accL := r &' (Z.ones 128) in
-         let accH := r >> 128 in
-         let dL := old &' (Z.ones 128) in
-         let dH := old >> 128 in
-         let d' := if L
-                   then (accL |' (dH << 128))
-                   else (dL |' (accL << 128)) in
-         Ok (write_wdr (write_wsr st ACC r) d d'))
-    | Bn_addm d x y =>
-         (x <- read_wdr st x ;
-          y <- read_wdr st y ;
-          m <- read_wsr st MOD ;          
-          Ok (write_wdr st d (addm_spec x y m)))
-    | Bn_subm d x y =>
-         (x <- read_wdr st x ;
-          y <- read_wdr st y ;
-          m <- read_wsr st MOD ;
-          Ok (write_wdr st d (subm_spec x y m)))
-    | Bn_add d x y s fg =>
-        (_ <- assertion (valid_arith_shift s) "Invalid shift for bn.add" ;
-         x <- read_wdr st x ;
-         y <- read_wdr st y ;
-         let r := x + y in
-         let st := set_mlz st fg r in
-         let st := flagfile_set st (flagC fg) (2^256 <=? r) in
-         Ok (write_wdr st d r))
-    | Bn_addc d x y s fg =>
-        (_ <- assertion (valid_arith_shift s) "Invalid shift for bn.addc" ;
-         c <- read_flag st (flagC fg);
-         x <- read_wdr st x ;
-         y <- read_wdr st y ;
-         let r := x + y + c in
-         let st := set_mlz st fg r in
-         let st := flagfile_set st (flagC fg) (2^256 <=? r) in
-         Ok (write_wdr st d r))
-    | Bn_sub d x y s fg =>
-        (_ <- assertion (valid_arith_shift s) "Invalid shift for bn.sub" ;
-         x <- read_wdr st x ;
-         y <- read_wdr st y ;
-         let r := x - y in
-         let st := set_mlz st fg r in
-         let st := flagfile_set st (flagC fg) (r <? 0) in
-         Ok (write_wdr st d r))
-    | Bn_subb d x y s fg =>
-        (_ <- assertion (valid_arith_shift s) "Invalid shift for bn.subb" ;
-         b <- read_flag st (flagC fg);
-         x <- read_wdr st x ;
-         y <- read_wdr st y ;
-         let r := x - y - b in
-         let st := set_mlz st fg r in
-         let st := flagfile_set st (flagC fg) (r <? 0) in
-         Ok (write_wdr st d r))
-    | Bn_rshi d x y imm =>
-        (_ <- assertion (valid_rshi_imm imm) "Invalid immediate for bn.rshi" ;
-         x <- read_wdr st x ;
-         y <- read_wdr st y ;
-         let r := rshi_spec x y imm in
-         Ok (write_wdr st d r))
-    | Bn_movr x y =>
-        let xinc := has_inc x in
-        let yinc := has_inc y in
-        let xr := ind_to_gpr x in
-        let yr := ind_to_gpr y in
-        (_ <- assertion (negb(xinc && yinc)) "Cannot increment both indirect registers (bn.movr)";
-         src_ptr <- read_gpr st yr ;
-         src <- index_to_wdr (src_ptr &' 32) ;
-         addr_ptr <- read_gpr st xr ;
-         addr <- index_to_wdr (addr_ptr &' 32) ;
-         v <- read_wdr st src ;
-         st <- (if xinc
-                then write_gpr st xr (src_ptr + 1)
-                else if yinc
-                     then write_gpr st yr (addr_ptr + 1)
-                     else Ok st) ;
-         Ok (write_wdr st addr v))
-    | Bn_lid x offset y =>
-        let xinc := has_inc x in
-        let yinc := has_inc y in
-        let xr := ind_to_gpr x in
-        let yr := ind_to_gpr y in
-        (_ <- assertion (negb(xinc && yinc)) "Cannot increment both indirect registers (bn.lid)";
-         _ <- assertion (valid_mem_offset offset) "Invalid offset for bn.lid";
-         src_ptr <- read_gpr st yr ;
-         src <- index_to_wdr (src_ptr &' 32) ;
-         addr_ptr <- read_gpr st xr ;
-         addr <- index_to_wdr (addr_ptr &' 32) ;
-         v <- read_wdr st src ;
-         st <- (if xinc
-                then write_gpr st xr (src_ptr + 1)
-                else if yinc
-                     then write_gpr st yr (addr_ptr + 1)
-                     else Ok st) ;
-         Ok (write_wdr st addr v))
-          (*
-    | _ => Err "NotImplemented"
-*)
+    | Some (Control LoopEnd) => pc
+    | Some (Control (Loop _)) =>
+        let end_pc := find_loop_end' fetch (advance_pc pc) in
+        find_loop_end' fetch (advance_pc end_pc)
+    | Some (Control (Loopi _)) =>
+        let end_pc := find_loop_end' fetch (advance_pc pc) in
+        find_loop_end' fetch (advance_pc end_pc)
+    | Some _ => find_loop_end' fetch (advance_pc pc)
+    | None => fail "reached end of function without finding loop end"
     end.
+Ltac find_loop_end :=
+  lazymatch goal with
+  | |- context [eventually (run1 (fetch:=?fetch)) _ (otbn_busy ?pc _ _ _ _ _ _)] =>
+      let i := eval vm_compute in (fetch pc) in
+        match i with
+        | Some (Control (Loop _)) => find_loop_end' fetch (advance_pc pc)
+        | Some (Control (Loopi _)) => find_loop_end' fetch (advance_pc pc)
+        | ?x => fail "expected a loop insn at " pc ", got " x
+        end
+  | _ => fail "could not determine fetch and pc from goal"
+  end.
 
-  Definition exec_straightline
-    (st : OtbnState) (insns : list sinsn) : maybe OtbnState :=
-    fold_left (fun st i => (st <- st ;
-                            st <- exec1 st i;
-                            Ok (inc_insn_counter st)))
-      insns (Ok st).
+(* register tracking initialize *)
+Ltac track_registers_init :=
+  let regs := lazymatch goal with
+              | |- context [otbn_busy _ ?regs] => regs end in
+  let regs' := fresh "regs" in
+  let H := fresh in
+  remember regs as regs' eqn:H;
+  assert (clobbers [] regs regs')
+    by (cbv [clobbers]; subst regs'; right; reflexivity);
+  (* rewrite back in postcondition but not state *)
+  rewrite H;
+  lazymatch goal with
+  | |- context [otbn_busy ?pc regs] =>
+      replace (otbn_busy pc regs) with (otbn_busy pc regs')
+      by (rewrite H; reflexivity)
+  end;
+  clear H.
 
-  Definition exec_straightline_cps {A}
-    (st : OtbnState) (insns : list sinsn) (f : maybe OtbnState -> A) : A :=
-    f (exec_straightline st insns).
+Ltac track_registers_update_step :=
+  lazymatch goal with
+  | H : clobbers ?l ?regs ?regs0
+    |- context [otbn_busy _ (map.put ?regs0 ?k ?v)] =>
+      let v' := fresh "v" in
+      set (v':= v);
+      (* try clobbers_step_in first, then more generic clobbers_step *)
+      first [ (let Hin := fresh in
+               assert (In k l) as Hin by (cbv [In]; tauto);
+               pose proof (clobbers_step_in l k v' _ _ H Hin))
+            | pose proof (clobbers_step l k v' _ _ H) ];
+      let regs1 := fresh "regs" in
+      let Hregs1 := fresh in
+      remember (map.put regs0 k v') as regs1 eqn:Hregs1;
+      assert (map.get regs1 k = Some v') by (subst regs1; apply map.get_put_same);
+      repeat lazymatch goal with
+        | H : map.get regs0 k = Some _ |- _ => clear H
+        | H : map.get regs0 ?r = Some ?v |- _ =>
+            assert (map.get regs1 r = Some v)
+            by (subst regs1; rewrite map.get_put_diff by congruence; eauto);
+            clear H
+        end;
+      clear Hregs1 H regs0
+  | H : clobbers ?l ?regs ?regs0
+    |- context [otbn_busy _ ?regs0] => idtac (* registers were not updated *)
+  end.
+Ltac track_registers_update :=
+  track_registers_update_step; repeat progress track_registers_update_step.
 
-  (* Test *)
-  Goal (forall st,
-           map.ok regfile ->
-           read_wdr st w2 = Ok 5 ->
-           (st <- exec_straightline st
-                    ([Addi x2 x0 2;
-                      Bn_add w0 w2 w2 (lshift 0) FG0]);
-            read_wdr st w0) = Ok 10).
+(* use after a jump to combine the postconditions *)
+Ltac track_registers_combine :=
+  lazymatch goal with
+  | H0 : clobbers ?l0 ?regs ?regs0,
+      H1 : clobbers ?l1 ?regs0 ?regs1
+    |- context [otbn_busy _ ?regs1] =>
+      repeat lazymatch goal with
+        | H : map.get regs0 ?r = _ |- _ =>
+            try (let Hnin := fresh in
+                 assert (~ In r l1) as Hnin by (cbv [In]; intuition congruence);
+                 pose proof (clobbers_not_in l1 _ _ _ _ H1 H Hnin);
+                 clear Hnin);
+            clear H
+        end;
+      let l2 := (eval vm_compute in (List.dedup reg_eqb (l0 ++ l1))) in
+      pose proof (clobbers_trans_dedup _ _ l2 _ _ _ H0 H1 ltac:(reflexivity));
+      clear H0 H1; try clear regs0
+  end.
+
+Ltac check_register_tracking :=
+  lazymatch goal with
+  | H : clobbers _ _ ?regs0 |- context [?regs0] => idtac
+  | _ => fail "cannot find register tracking; did you run track_registers_init?"
+  end.
+
+Ltac init_register_tracking_if_missing :=
+  first [ check_register_tracking
+        | track_registers_init ].
+
+Ltac straightline_step :=
+  init_register_tracking_if_missing;
+  let i := get_next_insn in
+  lazymatch i with
+  | Some (Straightline _) =>
+      intros; subst; eapply eventually_step;
+      [ simplify_side_condition; [ .. | try eapply eq_refl]
+      | intros; subst; track_registers_update ]
+  | Some ?i => fail "next instruction is not straightline:" i
+  | None => fail "pc is invalid?"
+  end.
+
+Ltac subst_lets_step :=
+  multimatch goal with
+  | x := _ |- _ => lazymatch goal with |- context [x] => subst x end
+  end.
+Ltac subst_lets := repeat subst_lets_step.
+
+Module Test.
+  Section __.
+  Context {word32 : word.word 32} {word32_ok : word.ok word32}.
+  Context {word256 : word.word 256} {word256_ok : word.ok word256}.
+  Context {regfile : map.map reg word32} {regfile_ok : map.ok regfile}.
+  Context {wregfile : map.map wreg word256} {wregfile_ok : map.ok wregfile}.
+  Context {flagfile : map.map flag bool} {flagfile_ok : map.ok flagfile}.
+  Context {mem : map.map word32 word32} {mem_ok : map.ok mem}.
+  Add Ring wring32: (@word.ring_theory 32 word32 word32_ok).
+  
+  (* Test program 0 : a function that adds two registers.
+
+     start:
+       addi x2, x0, 2
+       addi x3, x0, 3
+       jal  x1, add
+       sw   x5, 0(x0)
+       ecall
+
+     add:
+       add  x5, x2, x3
+       ret
+   *)
+  Definition add_fn : function :=
+    ("add"%string,
+      map.empty,
+      [(Add x5 x2 x3 : insn);
+       (Ret : insn)]).
+  Definition start_fn : function :=
+    ("start",
+      map.empty,
+      [ (Addi x2 x0 2 : insn);
+        (Addi x3 x0 3 : insn);
+        (Jal x1 "add" : insn);
+        (Sw x0 x5 0 : insn) ;
+        (Ecall : insn)])%string.
+
+  Compute (link [start_fn; add_fn]).
+
+  (* Test program 1 : build multiplication out of addition
+
+     mul:
+       addi   x2, x0, x0
+       beq    x4, x0, _mul_end
+       loop   x4, 2
+         jal    x1, add
+         addi   x2, x5, 0
+       _mul_end:
+       ret
+
+     add:
+       add  x5, x2, x3
+       ret
+   *)
+  Definition mul_fn : function :=
+    Eval cbn [List.app length] in (
+        let syms := map.empty in
+        let body : list insn :=
+          [ (Addi x2 x0 0 : insn);
+            (Beq x4 x0 "_mul_end" : insn);
+            (Loop x4 : insn);
+            (Jal x1 "add" : insn);
+            (Addi x2 x5 0 : insn);
+            (LoopEnd : insn)] in
+        let syms := map.put syms "_mul_end" (length body) in
+        let body := (body ++  [(Ret : insn)])%list in
+        ("mul", syms, body))%string.
+
+  Compute (link [mul_fn; add_fn]).
+
+  Definition prog0 : program := ltac:(link_program [start_fn; add_fn]).
+
+  Lemma prog0_correct :
+    eventually
+      (run1 (fetch:=fetch prog0))
+      (fun st =>
+         match st with
+         | otbn_done _ dmem =>
+             map.get dmem (word.of_Z 0) = Some (word.of_Z 5)
+         | _ => False
+         end)
+      start_state.
   Proof.
-    intros; cbn. destruct st.
-    cbv [read_wdr inc_insn_counter regs prefix_err] in *; cbn.
-    rewrite !map.get_put_diff by congruence.
-    lazymatch goal with
-    | H : _ = inl _ |- _ => rewrite H; cbn [bind]
-    end.
-    cbn [write_wdr regfile_set regs].
-    rewrite ?map.get_put_diff by congruence.
-    rewrite ?map.get_put_same by congruence.
+    cbv [prog0 start_state]; intros.
+    eapply eventually_step.
+    { simplify_side_condition. apply eq_refl. }
+    intros; subst. eapply eventually_step.
+    { simplify_side_condition. apply eq_refl. }
+    intros; subst. eapply eventually_step.
+    { simplify_side_condition. apply eq_refl. }
+    intros; subst. eapply eventually_step.
+    { simplify_side_condition. apply eq_refl. }
+    intros; subst. eapply eventually_step.
+    { simplify_side_condition. apply eq_refl. }
+    intros; subst. eapply eventually_step.
+    { simplify_side_condition. apply eq_refl. }
+    intros; subst. eapply eventually_step.
+    { simplify_side_condition. apply eq_refl. }
+    intros; subst. eapply eventually_done.
+    rewrite word.add_0_r.
+    solve_map. apply f_equal.
+    cbv [addi_spec]. repeat destruct_one_match; try lia; [ ].    
+    rewrite !word.add_0_l.
+    apply word.unsigned_inj.
+    rewrite !word.unsigned_add, !word.unsigned_of_Z by lia.
+    cbv [word.wrap]. Z.push_pull_mod. reflexivity.
+  Qed.
+
+  Lemma add_correct :
+    forall regs wregs flags dmem cstack lstack a b,
+      map.get regs (gpreg x2) = Some a ->
+      map.get regs (gpreg x3) = Some b ->
+      returns
+        (fetch:=fetch_ctx [add_fn])
+        "add"%string regs wregs flags dmem cstack lstack
+        (fun regs' wregs' flags' dmem' =>
+           map.get regs' (gpreg x5) = Some (word.add a b)
+           /\ wregs' = wregs
+           (* note: no guarantees about flags *)
+           /\ dmem' = dmem
+           /\ clobbers [gpreg x5] regs regs').
+  Proof.
+    cbv [add_fn returns]. intros; subst.
+    track_registers_init.
+    
+    eapply eventually_step.
+    { simplify_side_condition. apply eq_refl. }
+    intros; subst.    
+    track_registers_update.
+    eapply eventually_ret; [ reflexivity | eassumption | ].
+    ssplit; try reflexivity; [ | ].
+    { solve_map. }
+    { eapply map.only_differ_subset; [ | eassumption ].
+      cbv. tauto. }
+  Qed.
+
+  Lemma mul_correct :
+    forall regs wregs flags dmem cstack lstack a b,
+      map.get regs (gpreg x3) = Some a ->
+      map.get regs (gpreg x4) = Some b ->
+      (length cstack < 8)%nat ->
+      (length lstack < 8)%nat ->
+      returns
+        (fetch:=fetch_ctx [mul_fn; add_fn])
+        "mul"%string regs wregs flags dmem cstack lstack
+        (fun regs' wregs' flags' dmem' =>
+           map.get regs' (gpreg x2) = Some (word.mul a b)
+           /\ wregs' = wregs
+           /\ dmem' = dmem
+           /\ clobbers [gpreg x2; gpreg x5] regs regs').
+  Proof.
+    cbv [mul_fn returns]. intros; subst. 
+    repeat straightline_step.
+ 
+    (* branch; use branch helper lemma *)
+    eapply eventually_beq.
+    { reflexivity. }
+    { simplify_side_condition; reflexivity. }
+    { simplify_side_condition; reflexivity. }
+    { (* case: b = 0, exit early *)
+      intros; subst. eapply eventually_ret; [ reflexivity | eassumption | ].
+      rewrite word.mul_0_r.
+      ssplit; try reflexivity; [ | ].
+      { (* result value *)
+        solve_map; subst_lets. cbv [addi_spec].
+        destruct_one_match; try lia; [ ].
+        apply f_equal. ring. }
+      { eapply clobbers_incl; eauto.
+        cbv [incl In]; tauto. } }
+    (* case: b <> 0, proceed *)
+    intros; subst.
+
+    pose proof (word.unsigned_range b).
+    assert (0 < word.unsigned b).
+    { lazymatch goal with H : b <> word.of_Z 0 |- _ =>
+                            apply word.unsigned_inj' in H end.
+      rewrite word.unsigned_of_Z_0 in *.
+      lia. }
+ 
+    (* loop; use loop invariant lemma *)
+    let loop_end_pc := find_loop_end in
+    eapply loop_invariant
+      with
+      (end_pc:=loop_end_pc)
+      (invariant :=
+         fun i regs' wregs' flags' dmem' =>
+           map.get regs' (gpreg x2) = Some (word.mul a (word.sub b (word.of_Z (Z.of_nat i))))
+           /\ map.get regs' (gpreg x3) = Some a
+           /\ map.get regs' (gpreg x4) = Some b
+           /\ wregs' = wregs
+           /\ dmem' = dmem
+           /\ clobbers [gpreg x2; gpreg x5] regs regs').
+    { reflexivity. }
+    { reflexivity. }
+    { simplify_side_condition; reflexivity. }
+    { apply Z2Nat.id; lia. }
+    { lia. }
+    { lia. }
+    { (* prove invariant holds at start *)
+      ssplit; simplify_side_condition; zsimplify; try reflexivity.
+      { (* accumulator value *)
+        subst_lets. apply f_equal.
+        cbv [addi_spec]. destruct_one_match; try lia; [ ].
+        rewrite word.of_Z_unsigned. ring. }
+      { (* clobbered registers *)
+        eapply clobbers_incl; eauto. cbv [incl In]; tauto. } }
+    { (* invariant step; proceed through loop and prove invariant still holds *)
+      intros; subst. repeat lazymatch goal with H : _ /\ _ |- _ => destruct H end.
+
+      (* helper assertion that mul and add don't share symbols *)
+      assert (function_symbols_disjoint add_fn mul_fn).
+      { cbv [function_symbols_disjoint]; cbn [add_fn mul_fn fst snd].
+        ssplit; solve_map; try congruence; [ ].
+        cbv [map.disjoint]; intros *. rewrite map.get_empty; congruence. }
+
+      (* jump to "add" function *)
+      eapply eventually_jump.
+      { reflexivity. }
+      { lia. }
+      { apply add_correct; eauto. }
+      { intros.
+        rewrite fetch_ctx_weaken_cons_ne; [ eassumption | ].
+        eapply fetch_fn_disjoint; eauto; [ ].
+        eapply fetch_ctx_singleton_iff; eauto. }
+
+      (* post-jump; continue *)
+      cbv beta. intros; subst.
+      repeat lazymatch goal with H : _ /\ _ |- _ => destruct H end.
+      track_registers_combine.
+
+      repeat straightline_step.
+
+      (* end of loop; use loop-end helper lemma *)
+      eapply eventually_loop_end; [ reflexivity .. | ].
+      destruct_one_match.
+      { (* case: i = 0, loop ends *)
+        intros; subst. eapply eventually_done.
+        left. do 4 eexists; ssplit; [ .. | reflexivity ]; solve_map; [ ].
+        simplify_side_condition; subst_lets; zsimplify.
+        cbv [addi_spec]. destruct_one_match; try lia.
+        apply f_equal. ring. }
+      { (* case: 0 < i, loop continues *)
+        intros; subst. eapply eventually_done.
+        left. do 4 eexists; ssplit; [ .. | reflexivity ]; solve_map; [ ].
+        { simplify_side_condition. subst_lets; zsimplify.
+          cbv [addi_spec]. destruct_one_match; try lia.
+          apply f_equal.
+          replace (word.of_Z (Z.of_nat (S (S i))))
+            with (word.add (word:=word32) (word.of_Z (Z.of_nat (S i))) (word.of_Z 1));
+            [ ring | ].
+          apply word.unsigned_inj.
+          rewrite !word.unsigned_add, !word.unsigned_of_Z_nowrap, word.unsigned_of_Z by lia.
+          rewrite Z.add_1_r, <-Nat2Z.inj_succ. reflexivity. } } }
+ 
+    (* invariant implies postcondition (i.e. post-loop code) *)
+    zsimplify. rewrite word.sub_0_r. intros.
+    repeat lazymatch goal with
+           | H : _ /\ _ |- _ => destruct H
+           | H : Some _ = Some _ |- _ => inversion H; clear H; subst
+           end.
+    simplify_side_condition.
+    repeat straightline_step.
+    intros; subst. eapply eventually_ret; [ reflexivity | eassumption | ].
+    ssplit; eauto.
+  Qed.
+
+  Lemma prog0_correct_prelink regs wregs flags dmem :
+    exits
+      (fetch:=fetch_ctx [start_fn; add_fn])
+      "start"%string regs wregs flags dmem [] []
+      (fun dmem' =>
+         map.get dmem' (word.of_Z 0) = Some (word.of_Z 5))
+      (fun errs => False).
+  Proof.
+    cbv [exits start_fn start_state]; intros.
+    repeat straightline_step.
+
+    eapply eventually_jump.
+    { reflexivity. }
+    { cbn [length]; lia. }
+    { eapply add_correct; eauto. }
+    { intros.
+      rewrite fetch_ctx_weaken_cons_ne; [ eassumption | ].
+      eapply fetch_fn_disjoint; eauto; [ | ].
+      { eapply fetch_ctx_singleton_iff; eauto. }
+      { cbv; intuition congruence. } }
+
+    cbv beta. intros; subst.
+    repeat lazymatch goal with H : _ /\ _ |- _ => destruct H end.
+    track_registers_combine.
+
+    repeat straightline_step.
+
+    eapply eventually_ecall; ssplit; [ reflexivity .. | ].
+    subst_lets. cbv [addi_spec]. repeat destruct_one_match; try lia; [ ].
+    rewrite !word.add_0_l. solve_map.
+    apply f_equal. apply word.unsigned_inj.
+    rewrite !word.unsigned_add, !word.unsigned_of_Z_nowrap by lia.
     reflexivity.
   Qed.
 
-  Definition ctrl1_cps (st : OtbnState) (i : cinsn (addr:=addr))
-    {A} (f : maybe OtbnState -> A) : A :=
-    let st := inc_insn_counter st in
-    let next_pc := advance_pc st.(pc) in
-    match i with
-    | Ret => f (callstack_pop st)
-    | Ecall => f (Ok st)
-    | Jal r jump_pc =>
-        if gpr_eqb r x0
-        then f (Ok (jump st jump_pc))
-        else if gpr_eqb r x1
-             then 
-               match callstack_push st next_pc with
-               | Err e => f (Err e)
-               | Ok st => f (Ok (jump st jump_pc))
-               end
-             else f (Err "Jump-and-link for registers other than x1 or x0 is not supported.")
-    | Bne r1 r2 branch_pc =>
-        match read_gpr st r1, read_gpr st r2 with
-        | Err e, _ => f (Err e)
-        | _, Err e => f (Err e)
-        | Ok v1, Ok v2 =>
-            if (v1 =? v2) then f (Ok (jump st next_pc)) else f (Ok (jump st branch_pc))
-        end
-    | Beq r1 r2 branch_pc =>
-        match read_gpr st r1, read_gpr st r2 with
-        | Err e, _ => f (Err e)
-        | _, Err e => f (Err e)
-        | Ok v1, Ok v2 =>
-            if (v1 =? v2) then f (Ok (jump st branch_pc)) else f (Ok (jump st next_pc))
-        end
-    | Loop r len =>
-        match read_gpr st r with
-        | Err e => f (Err e)
-        | Ok v =>
-            if (0 <=? len)%nat
-            then
-              if 0 <=? v
-              then
-                let start_addr := next_pc in
-                let end_addr := repeat_advance_pc st.(pc) len in
-                match loopstack_push st (start_addr, end_addr, len) with
-                | Err e => f (Err e)
-                | Ok st => f (Ok (jump st next_pc))
-                end
-              else f (Err "Loop iteration count must be > 0.")
-            else f (Err "Loop instruction length must be > 0.")
-        end
-    | Loopi iters len =>
-        if (0 <=? len)%nat
-        then
-          if (0 <=? iters)%nat
-          then
-            let start_addr := next_pc in
-            let end_addr := repeat_advance_pc st.(pc) len in
-            match loopstack_push st (start_addr, end_addr, iters) with
-            | Err e => f (Err e)
-            | Ok st => f (Ok (jump st next_pc))
-            end
-          else f (Err "Loop iteration count must be > 0.")
-        else f (Err "Loop instruction length must be > 0.")
-    end.
-
-  Section __.
-    Context (blocks : map.rep (map:=blockmap)).
-
-    Definition exec_cps
-      {A} (st : OtbnState) (f : maybe OtbnState -> A) : A :=
-      match map.get blocks st.(pc) with
-      | None => f (Err "Block not found")
-      | Some (si, ci) =>
-          let end_pc := repeat_advance_pc st.(pc) (length si) in          
-          exec_straightline_cps
-            st si (fun st =>
-                     match st with
-                     | Err e => f (Err e)
-                     | Ok st =>
-                         match ci with
-                         | None =>
-                             (* Not a control-flow instruction; we
-                                must have reached the end of a loop *)
-                             match loopstack_pop st with
-                             | Err e => f (Err e)
-                             | Ok (loop_end_addr, loop_start_addr, iters, st) =>
-                                 if addr_eqb end_pc loop_end_addr
-                                 then
-                                   match iters with
-                                   | 0%nat => f (Ok (jump st (advance_pc loop_end_addr)))
-                                   | S iters =>
-                                       let loop_entry := (loop_end_addr, loop_start_addr, iters) in
-                                       match loopstack_push st loop_entry with
-                                       | Ok st => f (Ok (jump st loop_start_addr))
-                                       | Err e => f (Err e)
-                                       end
-                                   end
-                                 else f (Err "Reached loop end but loop stack did not match PC.")
-                             end
-                         | Some ci => ctrl1_cps (jump st end_pc) ci f
-                         end
-                     end)
+  (* check that link_run1 works by using add_fn proof to prove link_run1 program *)
+  Lemma prog0_correct_postlink :
+    exits
+      (fetch:=fetch prog0)
+      0%nat map.empty map.empty map.empty map.empty [] []
+      (fun dmem' =>
+         map.get dmem' (word.of_Z 0) = Some (word.of_Z 5))
+      (fun errs => False).
+  Proof.
+    set (fns:=[start_fn; add_fn]).
+    assert (link fns = inl prog0) by reflexivity.
+    let x := eval vm_compute in (link_symbols [start_fn; add_fn]) in
+      match x with
+      | inl ?x =>
+          pose (syms:=x)
+      | _ => fail
       end.
+    assert (link_symbols fns = inl syms) by reflexivity.
+    assert (find_global_offset fns "start"%string = Some 0%nat) by reflexivity.
+    eapply link_exits; eauto using prog0_correct_prelink.
+  Qed.
 
-    Definition exec (st : OtbnState) (P : OtbnState -> Prop) : Prop :=
-      exec_cps st (fun x =>
-                     match x with
-                     | Err _ => False
-                     | Ok x => P x
-                     end).
+  (* Test scaling with a large codegen. *)
+  Definition repeat_add (n : nat) : function :=
+    (("add" ++ String.of_nat n)%string,
+      map.empty,
+      (Addi x2 x0 0 : insn) :: repeat (Add x2 x2 x3 : insn) n ++ [(Ret : insn)]).
+  Definition add100_fn : function := Eval vm_compute in (repeat_add 100).
 
-    Check eventually.
-    Check eventually exec.
-    Check (forall (initial_state : OtbnState) (end_addr : addr),
-              eventually exec (fun st =>
-                                 st.(pc) = end_addr /\ read_wdr st w0 = Ok 0)
-                initial_state).
-    
-    (* key thing that makes this work is that in the postcondition P
-    you can specify which address you returned to *)
-    (* eventually doesn't guarantee that you've returned, but you know
-    because of the PC *)
-    (* so for subroutines you specify in the postcondition that the PC
-    is back to the caller *)
+  (* helper lemma *)
+  Lemma mul_by_add_step x (a : word32) n :
+    0 < n ->
+    x = word.mul a (word.of_Z (n - 1)) ->
+    word.add x a = word.mul a (word.of_Z n).
+  Proof.
+    intros; subst. cbv [Z.sub].
+    rewrite word.ring_morph_add, word.ring_morph_opp.
+    ring.
+  Qed.
 
-    (* question: how do you create blocks? *)
-    (* can use Z when processing binaries, since you know PC ahead of time *)
-    (* can use string + offset for correct-by-construction *)
+  Lemma add100_correct :
+    forall regs wregs flags dmem cstack lstack a,
+      map.get regs (gpreg x3) = Some a ->
+      returns
+        (fetch:=fetch_ctx [add100_fn])
+        "add100"%string regs wregs flags dmem cstack lstack
+        (fun regs' wregs' flags' dmem' =>
+           map.get regs' (gpreg x2) = Some (word.mul a (word.of_Z 100))
+           /\ wregs' = wregs
+           /\ dmem' = dmem                
+           /\ clobbers [gpreg x2] regs regs').
+  Proof.
+    cbv [returns]; intros.
+    straightline_step.
+    Time do 10 straightline_step.
+    Time do 10 straightline_step.
+    Time do 10 straightline_step.
+    Time do 10 straightline_step.
+    Time do 10 straightline_step.
+    Time do 10 straightline_step.
+    Time do 10 straightline_step.
+    Time do 10 straightline_step.
+    Time do 10 straightline_step.
+    Time do 10 straightline_step. (* .57s *)
 
-    (* need a definition that parses list of insns into blocks *)
-    (* need a way to construct subroutines as blocks *)
-    (* keep in mind that PCs are relative in binaries *)
-
-
-  End __.
-
-  Section TestProof.
-    Context {start_addr pow32_addr : addr}
-      {addrs_disjoint :
-        NoDup [start_addr; advance_pc (start_addr); advance_pc (advance_pc (start_addr));
-               pow32_addr; advance_pc (pow32_addr); advance_pc (advance_pc (pow32_addr))]}.
-    Import OtbnNotations.
-
-    Definition pow32_program : list (insn (addr:=Z)) :=
-      [
-        (* start: *)
-        jal x1, 8
-        ; ecall
-        (* pow32: *)
-        ; loopi 5, 1
-        ; bn.add w2, w2, w2, FG0
-        ; ret
-      ]%otbn.
-
-    Definition pow32_blocks : map.rep (map:=blockmap) :=
-      let blocks := map.empty in
-      let pc := pow32_addr in
-      let blocks := map.put blocks pc ([], Some (Loopi 5 1)) in
-      let pc := advance_pc pc in
-      let blocks := map.put blocks pc ([Bn_add w2 w2 w2 (lshift 0) FG0], None) in
-      let pc := advance_pc pc in
-      let blocks := map.put blocks pc ([], Some Ret) in
-      blocks.
-    Definition start_blocks : map.rep (map:=blockmap) :=
-      let blocks := map.empty in
-      let pc := start_addr in 
-      let blocks := map.put blocks pc ([], Some (Jal x1 pow32_addr)) in
-      let pc := advance_pc start_addr in 
-      let blocks := map.put blocks pc ([], Some Ecall) in
-      blocks.
-
-    Lemma pow32_disjoint :
-      pow32_addr <> advance_pc (pow32_addr)
-      /\ pow32_addr <> advance_pc (advance_pc (pow32_addr))
-      /\ advance_pc (pow32_addr) <> advance_pc (advance_pc (pow32_addr)).
-    Admitted.
-
-    Ltac mapsimpl :=
-      rewrite ?map.get_put_diff by congruence;
-      multimatch goal with
-      | |- context [map.get (map.put ?m ?k1 ?v) ?k2] =>
-          replace (map.put m k1 v) with (map.put m k2 v) by congruence;
-          rewrite (map.get_put_same m k2 v)
-      end.
-
-    Lemma exec_straightline_cps_empty (st : OtbnState) {A} (f : _ -> A) :
-      exec_straightline_cps st [] f = f (Ok st).
-    Proof. reflexivity. Qed.
-
-    Lemma repeat_advance_pc_0 (pc : addr) : repeat_advance_pc pc 0 = pc.
-    Proof. reflexivity. Qed.
-
-    Lemma jump_noop (st : OtbnState) (dst : addr) :
-      st.(pc) = dst -> jump st dst = st.
-    Proof. intros; subst; destruct st; reflexivity. Qed.
-
-    Lemma ctrl1_loopi (st : OtbnState) iters looplen :
-      (length st.(loopstack) < 8)%nat ->
-      ctrl1_cps st (Loopi iters looplen)
-        (fun st' => match st' with
-                    | inl st' =>
-                        (st'.(regs) = st.(regs)
-                         /\ st'.(flags) = st.(flags)
-                         /\ st'.(dmem) = st.(dmem)
-                         /\ st'.(callstack) = st.(callstack)
-                         /\ st'.(loopstack) =
-                              (advance_pc st.(pc), repeat_advance_pc st.(pc) looplen, iters)
-                                :: st.(loopstack)
-                         /\ st'.(insn_counter) = (st.(insn_counter) + 1)%nat
-                         /\ st'.(pc) = advance_pc (st.(pc)))
-                    | inr _ => False
-                    end).
-    Proof.
-      intros. cbv [ctrl1_cps inc_insn_counter jump loopstack_push assertion bind].
-      cbn [pc insn_counter loopstack callstack regs flags dmem].
-      repeat lazymatch goal with
-             | |- context [(?x <=? ?y)%nat] =>
-                 destruct (Nat.leb_spec x y); try lia
-             | |- context [(?x <? ?y)%nat] =>
-                 destruct (Nat.ltb_spec x y); try lia
-             end.
-      cbn [pc insn_counter loopstack callstack regs flags dmem].
-      ssplit; reflexivity.
-    Qed.
-
-    Lemma exec_straightline_cps_weaken (st : OtbnState) (insns : list sinsn) (P : _ -> Prop) :
-      forall (Q : _ -> Prop),
-        exec_straightline_cps st insns Q ->
-        (forall st', Q st' -> P st') ->
-        exec_straightline_cps st insns P.
-    Proof. cbv [exec_straightline_cps exec_straightline]. intros; eauto. Qed.
-
-    Lemma pow32_correct (st : OtbnState) :
-      map.ok blockmap ->
-      (0 < length st.(callstack))%nat ->
-      (length st.(loopstack) < 8)%nat ->
-      st.(pc) = pow32_addr ->
-      forall v,
-        map.get st.(regs) w2 = Some v ->
-        eventually (exec pow32_blocks)
-          (fun st' =>
-             st'.(pc) = hd pow32_addr st.(callstack)
-             /\ st'.(dmem) = st.(dmem)
-             /\ st'.(loopstack) = st.(loopstack)
-             /\ st'.(callstack) = tl st.(callstack)
-             /\ st'.(regs) = map.put st.(regs) w2 (v ^ 32)
-             /\ st'.(insn_counter) = (st.(insn_counter) + 7)%nat)
-        st.
-    Proof.
-      intros.
-      pose proof pow32_disjoint.
-      repeat lazymatch goal with
-             | H : _ /\ _ |- _ => destruct H
-             end.
-      
-      eapply eventually_step.
-      { cbv [exec exec_cps pow32_blocks]. mapsimpl.
-        rewrite exec_straightline_cps_empty.
-        rewrite repeat_advance_pc_0.
-        rewrite jump_noop by congruence.
-        apply ctrl1_loopi. lia. }
-
-
-      cbv beta; intros.
-      repeat lazymatch goal with
-             | H : _ /\ _ |- _ => destruct H
-             end.
-      eapply eventually_step.
-      { cbv [exec exec_cps pow32_blocks]. mapsimpl.
-        cbv [exec_straightline_cps exec_straightline]. cbn [fold_left].
-        eapply exec_straightline_cps_weaken.
-        
-        
-        (* need weakening lemma for exec_straightline_cps, then lemma for Bn_add *)
-        (* TODO: maybe separate OTBN control state from regs/flags? *)
-        (* TODO: maybe eliminate insn counter? *)
-        (* TODO: eliminate maybes, use err bits -- for imms and shifts do a mod or drop bits *)
-        
-      
-
-    Qed.
-End TestProof.
-
-  Check exec.
-  Fixpoint to_blocks (insns : list (insn (addr:=Z))) : :=
-    
-
-
-  
-End Exec.
+    eapply eventually_ret; [ reflexivity | eassumption | ].
+    ssplit; try reflexivity; [ | ].
+    { solve_map. apply (f_equal Some).
+      repeat (apply mul_by_add_step; [ lia | ];
+              cbn [Z.sub Z.add Z.opp Z.pos_sub Pos.pred_double]).
+      lazymatch goal with |- ?x = word.mul _ (word.of_Z 0) => subst x end.
+      cbv [addi_spec]. destruct_one_match; try lia; [ ].
+      ring. }    
+    { (* only_differ clause *)
+      eapply clobbers_incl; eauto. cbv [incl In]. tauto. }
+  Time Qed. (* 0.64s *)
 End __.
+End Test.
+
+Require Import coqutil.Word.Naive.
+Module SortedListRegs.
+  Definition ltb (r1 r2 : reg) := String.ltb (reg_to_string r1) (reg_to_string r2).
+  Definition Build_parameters (T : Type) : SortedList.parameters.parameters :=
+    {|
+      SortedList.parameters.key := reg;
+      SortedList.parameters.value := T;
+      SortedList.parameters.ltb := ltb;
+    |}.
+  Definition reg_strict_order : SortedList.parameters.strict_order ltb.
+  Proof.
+    cbv [ltb reg_to_string gpr_to_string csr_to_string]; constructor; intros.
+    { abstract (repeat destruct_one_match; apply eq_refl). }
+    { abstract (repeat destruct_one_match; try apply eq_refl;
+                repeat destruct_one_match_hyp; assumption). }
+    { abstract (repeat destruct_one_match_hyp; try reflexivity;
+                exfalso; cbv in *; try congruence). }
+  Defined.
+
+  Global Instance map : map.map reg Naive.word32 :=
+    SortedList.map (Build_parameters _) reg_strict_order.
+End SortedListRegs.
+
+Module ExecTest.
+  (* Check that exec works *)
+  Eval vm_compute in
+    (exec1 (regfile:=SortedListRegs.map) (fetch:=fetch Test.prog0) start_state).
+  Eval vm_compute in
+    (exec (regfile:=SortedListRegs.map) (fetch:=fetch Test.prog0) start_state 100).
+
+  (* scaling factor; create a program with ~n instructions *)
+  Definition n := 10000.
+  Definition add_fn : function := Eval vm_compute in (Test.repeat_add 10000).
+  Definition start_fn : function :=
+    ("start",
+      map.empty,
+      [ (Addi x3 x0 23 : insn);
+        (Jal x1 (fst (fst add_fn)) : insn);
+        (Ecall : insn)])%string.
+
+  (* Check that exec completes in a reasonable amount of time *)
+  Definition prog : program := ltac:(link_program [start_fn; add_fn]).
+  Time
+    Eval vm_compute in
+    (exec (regfile:=SortedListRegs.map) (fetch:=fetch prog) start_state (length prog)).
+
+End ExecTest.
+
+(* Next: try to add more realistic error conditions for e.g. loop errors *)
+(* Next: separation logic for memory *)
+(* Next: add notations back *)
+(* Next: instruction decoding *)
+(* Next: wclobbers, fclobbers *)
